theories/allocator/allocator_free_spec.v
@@ -1,60 +1,703 @@
 From iris.proofmode Require Import proofmode.
 From griotte Require Import rules proofmode memory_region.
 From griotte.allocator Require Import allocator_preamble
-  allocator_macros_spec.
+  allocator_macros_spec allocator_header_spec.
 
 (** Address of an assembled block relative to the entry point. *)
+
 Definition allocator_free_block_addr {MP : MachineParameters}
   (pc_a : Addr) (n : nat) : Addr :=
   (pc_a ^+ length (concat (take n assembled_allocator_free)))%a.
 
-Section AllocatorFreeBlocks.
-  Context {Σ : gFunctors} {ceriseg : ceriseG Σ} {allocatorg : allocatorG Σ}
-    {MP : MachineParameters} {layout : allocatorLayout}.
+Local Instance allocator_free_in_prefix_dec {MP : MachineParameters} next w :
+  Decision (allocator_free_in_prefix next w).
+Proof.
+  unfold allocator_free_in_prefix.
+  destruct w as [z|sb|tag p g b e a|ot sb].
+  - right. intros (? & ? & ? & ? & ? & Heq & _). discriminate.
+  - destruct sb as [tag p g b e a|tag p g b e a].
+    + destruct tag.
+      * destruct (decide (heap_b < b /\ b < e /\ e <= next)%a) as [Hbounds|Hbounds].
+        { left. exists p, g, b, e, a. auto. }
+        right. intros (p' & g' & b' & e' & a' & Heq & Hrange).
+        inversion Heq; subst. contradiction.
+      * right. intros (? & ? & ? & ? & ? & Heq & _). discriminate.
+    + right. intros (? & ? & ? & ? & ? & Heq & _). discriminate.
+  - right. intros (? & ? & ? & ? & ? & Heq & _). discriminate.
+  - right. intros (? & ? & ? & ? & ? & Heq & _). discriminate.
+Defined.
 
-  Lemma allocator_free_success_block_spec
+Section AllocatorFreeTraversal.
+  Context {Σ : gFunctors}
+    {ceriseg : ceriseG Σ}
+    {allocatorg : allocatorG Σ}
+    {allocator_historyg : allocatorHistoryG Σ}
+    {MP : MachineParameters}
+    {layout : allocatorLayout}.
+
+  (** At the search loop, [allocations] is the unvisited suffix. The visited
+      prefix is framed using [allocator_headers_app_spec], so unfolding one
+      list node supplies exactly the header read by block 4. Blocks 3 and 5
+      implement the loop guard and the advance to the tail, respectively. *)
+
+  Local Lemma allocator_free_search_loop_outcomes_aux
+    (E : coPset) (pc_b pc_e pc_a next h b e : Addr)
+    (allocations : list allocator_header_entry) (w3 wa2 : Word)
+    (φ : language.val griotte_lang → iPropI Σ) :
+
+    let start := allocator_free_block_addr pc_a 3 in
+    let code := concat (encodeInstrsW <$> take 3 (drop 3 assembled_allocator_free)) in
+    ContiguousRegion pc_a (length allocator_free_instrs) ->
+    SubBounds pc_b pc_e pc_a (pc_a ^+ length allocator_free_instrs)%a ->
+    disjoint_from_shadow pc_b pc_e ->
+    (heap_b < h /\ h <= next /\ next <= heap_e)%a ->
+
+    allocator_headers h next allocations ∗
+    PC ↦ᵣ WCap true RX Global pc_b pc_e start ∗
+    ct0 ↦ᵣ WCap true RW Global heap_b heap_e next ∗
+    ct1 ↦ᵣ WInt b ∗
+    ct2 ↦ᵣ WInt e ∗
+    ct3 ↦ᵣ w3 ∗
+    ct4 ↦ᵣ WCap true RW Global heap_b heap_e h ∗
+    ca2 ↦ᵣ wa2 ∗
+    codefrag start code ∗
+    ▷ (
+        allocator_headers h next allocations ∗
+        ct0 ↦ᵣ WCap true RW Global heap_b heap_e next ∗
+        ct1 ↦ᵣ WInt b ∗
+        ct2 ↦ᵣ WInt e ∗
+        ct3 ↦ᵣ - ∗
+        ct4 ↦ᵣ - ∗
+        ca2 ↦ᵣ - ∗
+        codefrag start code ∗
+        (
+          (
+            ⌜allocator_has_bounds allocations b e⌝ ∗
+            PC ↦ᵣ WCap true RX Global pc_b pc_e (allocator_free_block_addr pc_a 6)
+          )
+          ∨
+          (
+            ⌜¬ allocator_has_bounds allocations b e⌝ ∗
+            PC ↦ᵣ WCap true RX Global pc_b pc_e (allocator_free_block_addr pc_a 10)
+          )
+        )
+        -∗ WP Seq (Instr Executable) @ E {{ φ }}
+      )
+    ⊢ WP Seq (Instr Executable) @ E {{ φ }}.
+  Proof.
+    intros start code Hcont Hpc Hshadow Hrange; subst start code.
+    revert h w3 wa2 Hrange.
+    induction allocations as [| (base & finish & reserved) allocations IH]; intros h w3 wa2 Hrange.
+    {
+      iIntros "(%Hstop & HPC & Hct0 & Hct1 & Hct2 & Hct3 & Hct4 & Hca2 & Hcode & Hφ)".
+      subst h.
+      codefrag_facts "Hcode".
+      (* GetA ct3 ct4. *)
+      iInstr "Hcode".
+      assert (Hstep : (pc_a ^+ 26)%a = (allocator_free_block_addr pc_a 3 ^+ 1)%a) by (unfold allocator_free_block_addr; solve_addr).
+      iEval (rewrite Hstep) in "HPC".
+      (* GetA ca2 ct0. *)
+      iInstr "Hcode".
+      (* Lt ct3 ct3 ca2. *)
+      iInstr "Hcode".
+      rewrite Z.ltb_irrefl.
+      (* Jnz .free_header ct3. *)
+      iInstr "Hcode".
+      (* Jmp .free_invalid. *)
+      iInstr "Hcode".
+      assert (Hinvalid : (allocator_free_block_addr pc_a 3 ^+ 40)%a = allocator_free_block_addr pc_a 10) by (unfold allocator_free_block_addr; solve_addr).
+      iEval (rewrite Hinvalid) in "HPC".
+      iApply "Hφ".
+      iFrame.
+      iSplit; first done.
+      iRight.
+      iFrame.
+      iPureIntro.
+      unfold allocator_has_bounds.
+      set_solver.
+    }
+    iIntros "((%Hbounds & (%Hbase & Hend & Hreserved) & Htail) & HPC & Hct0 & Hct1 & Hct2 & Hct3 & Hct4 & Hca2 & Hcode & Hφ)".
+    unfold allocator_header_words in Hbase.
+    codefrag_facts "Hcode".
+    (* GetA ct3 ct4. *)
+    iInstr "Hcode".
+    assert (Hstep : (pc_a ^+ 26)%a = (allocator_free_block_addr pc_a 3 ^+ 1)%a) by (unfold allocator_free_block_addr; solve_addr).
+    iEval (rewrite Hstep) in "HPC".
+    (* GetA ca2 ct0. *)
+    iInstr "Hcode".
+    (* Lt ct3 ct3 ca2. *)
+    iInstr "Hcode".
+    replace (h <? next)%Z with true by (symmetry; apply Z.ltb_lt; solve_addr).
+    (* Jnz .free_header ct3. *)
+    iInstr "Hcode".
+    (* Load ca2 ct4. *)
+    iInstr_lookup "Hcode" as "Hi" "Hcode".
+    wp_instr.
+    iApply (wp_load_success_notinstr _ ca2 ct4 with "[$HPC $Hi $Hca2 $Hct4 $Hend]"); try solve_pure.
+    {
+      eapply (disjoint_from_shadow_not_in heap_b heap_e h); first exact heap_shadow_disjoint.
+      apply withinBounds_true_iff.
+      solve_addr.
+    }
+    { reflexivity. }
+    { constructor; [unfold allocator_free_block_addr; solve_addr|done]. }
+    {
+      split; first done.
+      apply withinBounds_true_iff.
+      solve_addr.
+    }
+    iIntros "!> (HPC & Hca2 & Hi & Hct4 & Hend)".
+    wp_pure.
+    iSpecialize ("Hcode" with "Hi").
+    iEval (cbn [load_word]) in "Hca2".
+    (* GetA ct3 ct4. *)
+    iInstr "Hcode".
+    (* Add ct3 ct3 allocator_header_words. *)
+    iInstr "Hcode".
+    (* Sub ct3 ct3 ct1. *)
+    iInstr "Hcode".
+    destruct (decide (base = b)) as [->|Hbase_ne].
+    + replace (h + 2 - b)%Z with 0%Z by solve_addr.
+      (* Jnz .free_next ct3. *)
+      iInstr "Hcode".
+      (* Sub ct3 ca2 ct2. *)
+      iInstr "Hcode".
+      destruct (decide (finish = e)) as [->|Hend_ne].
+      * rewrite Z.sub_diag.
+        (* Jnz .free_invalid ct3. *)
+        iInstr "Hcode".
+        (* Jmp .free_found. *)
+        iInstr "Hcode".
+        assert (Hfound : (allocator_free_block_addr pc_a 3 ^+ 17)%a = allocator_free_block_addr pc_a 6) by (unfold allocator_free_block_addr; solve_addr).
+        iEval (rewrite Hfound) in "HPC".
+        iApply "Hφ".
+        iFrame.
+        iSplit; first done.
+        iLeft.
+        iFrame.
+        iPureIntro.
+        exists reserved.
+        by left.
+      * assert (Hneq : WInt (finish - e) ≠ WInt 0) by (intros Heq; injection Heq as Heq; apply Hend_ne; solve_addr).
+        (* Jnz .free_invalid ct3. *)
+        iInstr "Hcode".
+        iDestruct (allocator_headers_chain_spec with "Htail") as %Hchain.
+        assert (Hmiss : ¬ allocator_has_bounds ((b, (finish, reserved)) :: allocations) b e).
+        {
+          intros (r & Hin).
+          apply elem_of_cons in Hin as [Heq|Hin].
+          - injection Heq as Heq.
+            congruence.
+          - pose proof (allocator_chain_member_bounds _ _ _ _ _ _ Hchain Hin).
+            solve_addr.
+        }
+        assert (Hinvalid : (allocator_free_block_addr pc_a 3 ^+ 40)%a = allocator_free_block_addr pc_a 10) by (unfold allocator_free_block_addr; solve_addr).
+        iEval (rewrite Hinvalid) in "HPC".
+        iApply "Hφ".
+        iFrame.
+        iSplit; first done.
+        iRight.
+        iFrame.
+        done.
+    + assert (Hneq : WInt (h + 2 - b) ≠ WInt 0) by (intros Heq; injection Heq as Heq; apply Hbase_ne; solve_addr).
+      (* Jnz .free_next ct3. *)
+      iInstr "Hcode".
+      (* GetA ct3 ct4. *)
+      iInstr "Hcode".
+      (* Sub ct3 ca2 ct3. *)
+      iInstr "Hcode".
+      (* Lea ct4 ct3. *)
+      iInstr "Hcode".
+      (* Jmp .free_search. *)
+      iInstr "Hcode".
+      iApply (IH finish with "[$Htail $HPC $Hct0 $Hct1 $Hct2 $Hct3 $Hct4 $Hca2 $Hcode Hφ Hend Hreserved]"); first solve_addr.
+      iNext.
+      iIntros "(Htail & Hct0 & Hct1 & Hct2 & Hct3 & Hct4 & Hca2 & Hcode & Hresult)".
+      iApply "Hφ".
+      iFrame.
+      iSplit; first done.
+      iDestruct "Hresult" as "[(%Hfound & HPC)|(%Hmiss & HPC)]".
+      * iLeft.
+        iFrame.
+        iPureIntro.
+        unfold allocator_has_bounds in *.
+        set_solver.
+      * iRight.
+        iFrame.
+        iPureIntro.
+        intros (r & Hin).
+        apply elem_of_cons in Hin as [Heq|Hin].
+        { injection Heq as Heq; congruence. }
+        apply Hmiss.
+        exists r.
+        exact Hin.
+  Qed.
+
+  Local Lemma allocator_free_search_loop_found_spec
+    (E : coPset) (pc_b pc_e pc_a next h b e : Addr)
+    (allocations : list allocator_header_entry) (w3 wa2 : Word)
+    (φ : language.val griotte_lang → iPropI Σ) :
+
+    let start := allocator_free_block_addr pc_a 3 in
+    let code := concat (encodeInstrsW <$> take 3 (drop 3 assembled_allocator_free)) in
+    ContiguousRegion pc_a (length allocator_free_instrs) ->
+    SubBounds pc_b pc_e pc_a (pc_a ^+ length allocator_free_instrs)%a ->
+    disjoint_from_shadow pc_b pc_e ->
+    (heap_b < h /\ h <= next /\ next <= heap_e)%a ->
+
+    allocator_has_bounds allocations b e ->
+
+    allocator_headers h next allocations ∗
+    PC ↦ᵣ WCap true RX Global pc_b pc_e start ∗
+    ct0 ↦ᵣ WCap true RW Global heap_b heap_e next ∗
+    ct1 ↦ᵣ WInt b ∗
+    ct2 ↦ᵣ WInt e ∗
+    ct3 ↦ᵣ w3 ∗
+    ct4 ↦ᵣ WCap true RW Global heap_b heap_e h ∗
+    ca2 ↦ᵣ wa2 ∗
+    codefrag start code ∗
+    ▷ (
+        allocator_headers h next allocations ∗
+        ct0 ↦ᵣ WCap true RW Global heap_b heap_e next ∗
+        ct1 ↦ᵣ WInt b ∗
+        ct2 ↦ᵣ WInt e ∗
+        ct3 ↦ᵣ - ∗
+        ct4 ↦ᵣ - ∗
+        ca2 ↦ᵣ - ∗
+        codefrag start code ∗
+        (
+          ⌜allocator_has_bounds allocations b e⌝ ∗
+          PC ↦ᵣ WCap true RX Global pc_b pc_e (allocator_free_block_addr pc_a 6)
+        )
+        -∗ WP Seq (Instr Executable) @ E {{ φ }}
+      )
+    ⊢ WP Seq (Instr Executable) @ E {{ φ }}.
+  Proof.
+    intros start code Hcont Hpc Hshadow Hrange Hfound; subst start code.
+    iIntros "(Hheaders & HPC & Hct0 & Hct1 & Hct2 & Hct3 & Hct4 & Hca2 & Hcode & Hφ)".
+    iApply (allocator_free_search_loop_outcomes_aux with
+      "[$Hheaders $HPC $Hct0 $Hct1 $Hct2 $Hct3 $Hct4 $Hca2 $Hcode Hφ]"); eauto.
+    iNext.
+    iIntros "(Hheaders & Hct0 & Hct1 & Hct2 & Hct3 & Hct4 & Hca2 & Hcode & Hresult)".
+    iDestruct "Hresult" as "[(%Hhas & HPC)|(%Hmiss & HPC)]".
+    - iApply "Hφ". iFrame. iPureIntro. exact Hhas.
+    - exfalso. apply Hmiss. exact Hfound.
+  Qed.
+
+  Local Lemma allocator_free_search_loop_missing_spec
+    (E : coPset) (pc_b pc_e pc_a next h b e : Addr)
+    (allocations : list allocator_header_entry) (w3 wa2 : Word)
+    (φ : language.val griotte_lang → iPropI Σ) :
+
+    let start := allocator_free_block_addr pc_a 3 in
+    let code := concat (encodeInstrsW <$> take 3 (drop 3 assembled_allocator_free)) in
+    ContiguousRegion pc_a (length allocator_free_instrs) ->
+    SubBounds pc_b pc_e pc_a (pc_a ^+ length allocator_free_instrs)%a ->
+    disjoint_from_shadow pc_b pc_e ->
+    (heap_b < h /\ h <= next /\ next <= heap_e)%a ->
+
+    ¬ allocator_has_bounds allocations b e ->
+
+    allocator_headers h next allocations ∗
+    PC ↦ᵣ WCap true RX Global pc_b pc_e start ∗
+    ct0 ↦ᵣ WCap true RW Global heap_b heap_e next ∗
+    ct1 ↦ᵣ WInt b ∗
+    ct2 ↦ᵣ WInt e ∗
+    ct3 ↦ᵣ w3 ∗
+    ct4 ↦ᵣ WCap true RW Global heap_b heap_e h ∗
+    ca2 ↦ᵣ wa2 ∗
+    codefrag start code ∗
+    ▷ (
+        allocator_headers h next allocations ∗
+        ct0 ↦ᵣ WCap true RW Global heap_b heap_e next ∗
+        ct1 ↦ᵣ WInt b ∗
+        ct2 ↦ᵣ WInt e ∗
+        ct3 ↦ᵣ - ∗
+        ct4 ↦ᵣ - ∗
+        ca2 ↦ᵣ - ∗
+        codefrag start code ∗
+        (
+          ⌜¬ allocator_has_bounds allocations b e⌝ ∗
+          PC ↦ᵣ WCap true RX Global pc_b pc_e (allocator_free_block_addr pc_a 10)
+        )
+        -∗ WP Seq (Instr Executable) @ E {{ φ }}
+      )
+    ⊢ WP Seq (Instr Executable) @ E {{ φ }}.
+  Proof.
+    intros start code Hcont Hpc Hshadow Hrange Hmissing; subst start code.
+    iIntros "(Hheaders & HPC & Hct0 & Hct1 & Hct2 & Hct3 & Hct4 & Hca2 & Hcode & Hφ)".
+    iApply (allocator_free_search_loop_outcomes_aux with
+      "[$Hheaders $HPC $Hct0 $Hct1 $Hct2 $Hct3 $Hct4 $Hca2 $Hcode Hφ]"); eauto.
+    iNext.
+    iIntros "(Hheaders & Hct0 & Hct1 & Hct2 & Hct3 & Hct4 & Hca2 & Hcode & Hresult)".
+    iDestruct "Hresult" as "[(%Hhas & HPC)|(%Hmiss & HPC)]".
+    - exfalso. apply Hmissing. exact Hhas.
+    - iApply "Hφ". iFrame. iPureIntro. exact Hmiss.
+  Qed.
+
+  (** Full traversal also executes block 2, which rederives the first header
+      from the heap root. No payload ownership is needed to identify a block. *)
+
+  Local Lemma allocator_free_search_outcomes_aux
+    (E : coPset) (pc_b pc_e pc_a next b e : Addr)
+    (allocations : list allocator_header_entry) (w3 w4 wa2 : Word)
+    (φ : language.val griotte_lang → iPropI Σ) :
+
+    let start := allocator_free_block_addr pc_a 2 in
+    let code := concat (encodeInstrsW <$> take 4 (drop 2 assembled_allocator_free)) in
+    ContiguousRegion pc_a (length allocator_free_instrs) ->
+    SubBounds pc_b pc_e pc_a (pc_a ^+ length allocator_free_instrs)%a ->
+    disjoint_from_shadow pc_b pc_e ->
+    (heap_b < next /\ next <= heap_e)%a ->
+
+    allocator_headers (heap_b ^+ 1)%a next allocations ∗
+    PC ↦ᵣ WCap true RX Global pc_b pc_e start ∗
+    ct0 ↦ᵣ WCap true RW Global heap_b heap_e next ∗
+    ct1 ↦ᵣ WInt b ∗
+    ct2 ↦ᵣ WInt e ∗
+    ct3 ↦ᵣ w3 ∗
+    ct4 ↦ᵣ w4 ∗
+    ca2 ↦ᵣ wa2 ∗
+    codefrag start code ∗
+    ▷ (
+        allocator_headers (heap_b ^+ 1)%a next allocations ∗
+        ct0 ↦ᵣ WCap true RW Global heap_b heap_e next ∗
+        ct1 ↦ᵣ WInt b ∗
+        ct2 ↦ᵣ WInt e ∗
+        ct3 ↦ᵣ - ∗
+        ct4 ↦ᵣ - ∗
+        ca2 ↦ᵣ - ∗
+        codefrag start code ∗
+        (
+          (
+            ⌜allocator_has_bounds allocations b e⌝ ∗
+             PC ↦ᵣ WCap true RX Global pc_b pc_e (allocator_free_block_addr pc_a 6)
+          )
+          ∨
+          (
+            ⌜¬ allocator_has_bounds allocations b e⌝ ∗
+            PC ↦ᵣ WCap true RX Global pc_b pc_e (allocator_free_block_addr pc_a 10)
+          )
+        )
+        -∗ WP Seq (Instr Executable) @ E {{ φ }})
+    ⊢ WP Seq (Instr Executable) @ E {{ φ }}.
+  Proof.
+    intros start code Hcont Hpc Hshadow Hnext; subst start code.
+    iIntros "(Hheaders & HPC & Hct0 & Hct1 & Hct2 & Hct3 & Hct4 & Hca2 & Hcode & Hφ)".
+    codefrag_facts "Hcode".
+    (* Mov ct4 ct0. *)
+    iInstr "Hcode".
+    assert (Hstep : (pc_a ^+ 20)%a = (allocator_free_block_addr pc_a 2 ^+ 1)%a)
+      by (unfold allocator_free_block_addr; solve_addr).
+    iEval (rewrite Hstep) in "HPC".
+    (* GetB ct3 ct0. *)
+    iInstr "Hcode".
+    (* GetA ca2 ct0. *)
+    iInstr "Hcode".
+    (* Sub ct3 ct3 ca2. *)
+    iInstr "Hcode".
+    (* Add ct3 ct3 1. *)
+    iInstr "Hcode".
+    (* Lea ct4 ct3. *)
+    iInstr "Hcode".
+    assert (Hfirst : (next ^+ (heap_b - next + 1))%a = (heap_b ^+ 1)%a) by solve_addr.
+    iEval (rewrite Hfirst) in "Hct4".
+    assert (Hsearch : (allocator_free_block_addr pc_a 2 ^+ 6)%a = allocator_free_block_addr pc_a 3)
+      by (unfold allocator_free_block_addr; solve_addr).
+    iEval (rewrite Hsearch) in "HPC".
+    assert (Hsplit : concat (encodeInstrsW <$> take 4 (drop 2 assembled_allocator_free)) =
+      allocator_free_instrs_n 2 ++ concat (encodeInstrsW <$> take 3 (drop 3 assembled_allocator_free))) by reflexivity.
+    iEval (rewrite Hsplit) in "Hcode".
+    focus_block_nochangePC 1 "Hcode" as a_search Ha_search "Hsearchcode" "Hcode_cont".
+    assert (Ha_eq : a_search = allocator_free_block_addr pc_a 3)
+      by (unfold allocator_free_block_addr in *; solve_addr).
+    subst a_search.
+    iApply (allocator_free_search_loop_outcomes_aux with
+      "[- $Hheaders $HPC $Hct0 $Hct1 $Hct2 $Hct3 $Hct4 $Hca2 $Hsearchcode]"); try assumption; first solve_addr.
+    iNext. iIntros "(Hheaders & Hct0 & Hct1 & Hct2 & Hct3 & Hct4 & Hca2 & Hsearchcode & Hresult)".
+    iDestruct ("Hcode_cont" with "Hsearchcode") as "Hcode".
+    iEval (rewrite -Hsplit) in "Hcode".
+    iApply "Hφ". iFrame.
+  Qed.
+
+  Local Lemma allocator_free_search_found_spec
+    (E : coPset) (pc_b pc_e pc_a next b e : Addr)
+    (allocations : list allocator_header_entry) (w3 w4 wa2 : Word)
+    (φ : language.val griotte_lang → iPropI Σ) :
+
+    let start := allocator_free_block_addr pc_a 2 in
+    let code := concat (encodeInstrsW <$> take 4 (drop 2 assembled_allocator_free)) in
+    ContiguousRegion pc_a (length allocator_free_instrs) ->
+    SubBounds pc_b pc_e pc_a (pc_a ^+ length allocator_free_instrs)%a ->
+    disjoint_from_shadow pc_b pc_e ->
+    (heap_b < next /\ next <= heap_e)%a ->
+
+    allocator_has_bounds allocations b e ->
+
+    allocator_headers (heap_b ^+ 1)%a next allocations ∗
+    PC ↦ᵣ WCap true RX Global pc_b pc_e start ∗
+    ct0 ↦ᵣ WCap true RW Global heap_b heap_e next ∗
+    ct1 ↦ᵣ WInt b ∗
+    ct2 ↦ᵣ WInt e ∗
+    ct3 ↦ᵣ w3 ∗
+    ct4 ↦ᵣ w4 ∗
+    ca2 ↦ᵣ wa2 ∗
+    codefrag start code ∗
+    ▷ (
+        allocator_headers (heap_b ^+ 1)%a next allocations ∗
+        ct0 ↦ᵣ WCap true RW Global heap_b heap_e next ∗
+        ct1 ↦ᵣ WInt b ∗
+        ct2 ↦ᵣ WInt e ∗
+        ct3 ↦ᵣ - ∗
+        ct4 ↦ᵣ - ∗
+        ca2 ↦ᵣ - ∗
+        codefrag start code ∗
+        (
+          ⌜allocator_has_bounds allocations b e⌝ ∗
+          PC ↦ᵣ WCap true RX Global pc_b pc_e (allocator_free_block_addr pc_a 6)
+        )
+        -∗ WP Seq (Instr Executable) @ E {{ φ }})
+    ⊢ WP Seq (Instr Executable) @ E {{ φ }}.
+  Proof.
+    intros start code Hcont Hpc Hshadow Hnext Hout; subst start code.
+    iIntros "(Hheaders & HPC & Hct0 & Hct1 & Hct2 & Hct3 & Hct4 & Hca2 & Hcode & Hφ)".
+    iApply (allocator_free_search_outcomes_aux with
+      "[$Hheaders $HPC $Hct0 $Hct1 $Hct2 $Hct3 $Hct4 $Hca2 $Hcode Hφ]"); eauto.
+    iNext.
+    iIntros "(Hheaders & Hct0 & Hct1 & Hct2 & Hct3 & Hct4 & Hca2 & Hcode & Hresult)".
+    iDestruct "Hresult" as "[(%Hhas & HPC)|(%Hmiss & HPC)]".
+    - iApply "Hφ". iFrame. iPureIntro. exact Hhas.
+    - exfalso. apply Hmiss. exact Hout.
+  Qed.
+
+  Local Lemma allocator_free_search_missing_spec
+    (E : coPset) (pc_b pc_e pc_a next b e : Addr)
+    (allocations : list allocator_header_entry) (w3 w4 wa2 : Word)
+    (φ : language.val griotte_lang → iPropI Σ) :
+
+    let start := allocator_free_block_addr pc_a 2 in
+    let code := concat (encodeInstrsW <$> take 4 (drop 2 assembled_allocator_free)) in
+    ContiguousRegion pc_a (length allocator_free_instrs) ->
+    SubBounds pc_b pc_e pc_a (pc_a ^+ length allocator_free_instrs)%a ->
+    disjoint_from_shadow pc_b pc_e ->
+    (heap_b < next /\ next <= heap_e)%a ->
+
+    ¬ allocator_has_bounds allocations b e ->
+
+    allocator_headers (heap_b ^+ 1)%a next allocations ∗
+    PC ↦ᵣ WCap true RX Global pc_b pc_e start ∗
+    ct0 ↦ᵣ WCap true RW Global heap_b heap_e next ∗
+    ct1 ↦ᵣ WInt b ∗
+    ct2 ↦ᵣ WInt e ∗
+    ct3 ↦ᵣ w3 ∗
+    ct4 ↦ᵣ w4 ∗
+    ca2 ↦ᵣ wa2 ∗
+    codefrag start code ∗
+    ▷ (
+        allocator_headers (heap_b ^+ 1)%a next allocations ∗
+        ct0 ↦ᵣ WCap true RW Global heap_b heap_e next ∗
+        ct1 ↦ᵣ WInt b ∗
+        ct2 ↦ᵣ WInt e ∗
+        ct3 ↦ᵣ - ∗
+        ct4 ↦ᵣ - ∗
+        ca2 ↦ᵣ - ∗
+        codefrag start code ∗
+        (
+          ⌜¬ allocator_has_bounds allocations b e⌝ ∗
+          PC ↦ᵣ WCap true RX Global pc_b pc_e (allocator_free_block_addr pc_a 10)
+        )
+        -∗ WP Seq (Instr Executable) @ E {{ φ }})
+    ⊢ WP Seq (Instr Executable) @ E {{ φ }}.
+  Proof.
+    intros start code Hcont Hpc Hshadow Hnext Hout; subst start code.
+    iIntros "(Hheaders & HPC & Hct0 & Hct1 & Hct2 & Hct3 & Hct4 & Hca2 & Hcode & Hφ)".
+    iApply (allocator_free_search_outcomes_aux with
+      "[$Hheaders $HPC $Hct0 $Hct1 $Hct2 $Hct3 $Hct4 $Hca2 $Hcode Hφ]"); eauto.
+    iNext.
+    iIntros "(Hheaders & Hct0 & Hct1 & Hct2 & Hct3 & Hct4 & Hca2 & Hcode & Hresult)".
+    iDestruct "Hresult" as "[(%Hhas & HPC)|(%Hmiss & HPC)]".
+    - exfalso. apply Hout. exact Hhas.
+    - iApply "Hφ". iFrame. iPureIntro. exact Hmiss.
+  Qed.
+
+  Definition allocator_free_shadow_resources (s : AllocStatus) (b : Addr) : iProp Σ :=
+    match s with
+    | ShadowLive => b ↦ₐ -
+    | ShadowQuarantined => reclaim_token b
+    end%I.
+
+  (** This block only reads the shadow bit: ownership of a live cell or a
+      reclaim token connects the observation to the shared allocator invariant.
+      All resources survive either branch; painting starts at block 8. *)
+
+  Local Lemma allocator_free_shadow_check_spec
+    (E : coPset) (pc_b pc_e pc_a next b e sb : Addr)
+    (s : AllocStatus) (w3 wa2 : Word)
+    (φ : language.val griotte_lang → iPropI Σ) :
+
+    let start := allocator_free_block_addr pc_a 7 in
+    let code := allocator_free_instrs_n 7 in
+    ↑Nallocator ⊆ E ->
+    ContiguousRegion pc_a (length allocator_free_instrs) ->
+    SubBounds pc_b pc_e pc_a (pc_a ^+ length allocator_free_instrs)%a ->
+    disjoint_from_shadow pc_b pc_e ->
+    (heap_b < b /\ b < e /\ e <= next /\ next <= heap_e)%a ->
+    (shadow_b + (b - heap_b))%a = Some sb ->
+    heap_to_shadow b = Some sb ->
+
+    allocator_ctx ∗
+    allocator_free_shadow_resources s b ∗
+    PC ↦ᵣ WCap true RX Global pc_b pc_e start ∗
+    ct0 ↦ᵣ WCap true RW Global heap_b heap_e next ∗
+    ct1 ↦ᵣ WInt b ∗
+    ct2 ↦ᵣ WInt e ∗
+    ct3 ↦ᵣ w3 ∗
+    ca2 ↦ᵣ wa2 ∗
+    ctp ↦ᵣ WCap true RW Global shadow_b shadow_e shadow_b ∗
+    codefrag start code ∗
+    ▷ (allocator_free_shadow_resources s b ∗
+         ct0 ↦ᵣ WCap true RW Global heap_b heap_e next ∗
+         ct1 ↦ᵣ WInt b ∗
+         ct2 ↦ᵣ WInt e ∗
+         ctp ↦ᵣ WCap true RW Global shadow_b shadow_e sb ∗
+         codefrag start code ∗
+         (match s with
+            | ShadowLive =>
+                PC ↦ᵣ WCap true RX Global pc_b pc_e
+                  (allocator_free_block_addr pc_a 8) ∗
+                ct3 ↦ᵣ WInt 0 ∗
+                ca2 ↦ᵣ WInt (e - b)
+            | ShadowQuarantined =>
+                PC ↦ᵣ WCap true RX Global pc_b pc_e
+                  (allocator_free_block_addr pc_a 10) ∗
+                ct3 ↦ᵣ WInt (encodeAllocStatus ShadowQuarantined -
+                              encodeAllocStatus ShadowLive) ∗
+                              ca2 ↦ᵣ wa2
+            end)
+         -∗ WP Seq (Instr Executable) @ E {{ φ }})
+    ⊢ WP Seq (Instr Executable) @ E {{ φ }}.
+  Proof.
+    intros start code HE Hcont Hpc Hdisjoint Hbounds Hsb Htranslate; subst start code.
+    iIntros "(#Hctx & Hres & HPC & Hct0 & Hct1 & Hct2 & Hct3 & Hca2 & Hctp & Hcode & Hφ)".
+    codefrag_facts "Hcode".
+    (* GetB ct3 ct0. *)
+    iInstr "Hcode".
+    assert (Hstep : (pc_a ^+ 52)%a = (allocator_free_block_addr pc_a 7 ^+ 1)%a) by (unfold allocator_free_block_addr; solve_addr).
+    iEval (rewrite Hstep) in "HPC".
+    (* Sub ct3 ct1 ct3. *)
+    iInstr "Hcode".
+    (* Lea ctp ct3. *)
+    iInstr "Hcode".
+    (* Load ct3 ctp. *)
+    iInstr_lookup "Hcode" as "Hi" "Hcode".
+    wp_instr.
+    iInv Nallocator as ">Hbody" "Hclose".
+    assert (Hb_heap : b ∈ heap_addresses) by (rewrite elem_of_heap_addresses; apply withinBounds_true_iff; solve_addr).
+    iDestruct (allocator_inv_lookup b with "Hbody") as (st) "[Hentry Hput]"; first done.
+    iAssert (⌜shadow_status st = s⌝)%I with "[Hentry Hres]" as %Hstatus.
+    {
+      destruct s.
+      - iDestruct "Hres" as (w) "Hmem".
+        iDestruct (allocator_entry_memory_live with "Hentry Hmem") as %->.
+        done.
+      - iDestruct (allocator_entry_token_quarantined with "Hentry Hres") as %->.
+        done.
+    }
+    iDestruct "Hentry" as "[Hshadow Hstate]".
+    iEval (rewrite Hstatus) in "Hshadow".
+    iApply (wp_load_success_from_shadow _ ct3 ctp with "[$HPC $Hi $Hct3 $Hctp $Hshadow]"); try solve_pure.
+    { exact (proj2 (heap_to_shadow_bounds _ _ Htranslate)). }
+    {
+      apply heap_shadow_inverse.
+      exact Htranslate.
+    }
+    { constructor; [unfold allocator_free_block_addr; solve_addr|done]. }
+    { split; first done. exact (proj2 (heap_to_shadow_bounds _ _ Htranslate)). }
+    iIntros "!> (HPC & Hct3 & Hi & Hctp & Hshadow)".
+    iMod ("Hclose" with "[Hshadow Hstate Hput]") as "_".
+    {
+      iNext.
+      iApply "Hput".
+      instantiate (1 := st).
+      rewrite /allocator_entry Hstatus.
+      iFrame.
+    }
+    iModIntro.
+    wp_pure.
+    iSpecialize ("Hcode" with "Hi").
+    (* Sub ct3 ct3 (encodeAllocStatus ShadowLive). *)
+    iInstr "Hcode".
+    change (match MP with {| encodeAllocStatus := f |} => f end ShadowLive) with (encodeAllocStatus ShadowLive).
+    destruct s.
+    - rewrite Z.sub_diag.
+    (* Jnz .free_invalid ct3. *)
+    iInstr "Hcode".
+    (* Sub ca2 ct2 ct1. *)
+    iInstr "Hcode".
+    assert (Hpaint : (allocator_free_block_addr pc_a 7 ^+ 7)%a = allocator_free_block_addr pc_a 8) by (unfold allocator_free_block_addr; solve_addr).
+    iEval (rewrite Hpaint) in "HPC".
+    iApply "Hφ".
+    iFrame.
+    - assert (Hneq : WInt (encodeAllocStatus ShadowQuarantined - encodeAllocStatus ShadowLive) ≠ WInt 0).
+    {
+      intros Heq.
+      injection Heq as Heq.
+      assert (Henc : encodeAllocStatus ShadowQuarantined = encodeAllocStatus ShadowLive) by lia.
+      apply (f_equal decodeAllocStatus) in Henc.
+      rewrite !decode_encode_alloc_status_inv in Henc.
+      discriminate.
+    }
+    (* Jnz .free_invalid ct3. *)
+    iInstr "Hcode".
+    assert (Hinvalid : (allocator_free_block_addr pc_a 7 ^+ 14)%a = allocator_free_block_addr pc_a 10) by (unfold allocator_free_block_addr; solve_addr).
+    iEval (rewrite Hinvalid) in "HPC".
+    iApply "Hφ".
+    iFrame.
+  Qed.
+
+  Local Lemma allocator_free_success_block_spec
     (E : coPset) (pc_b pc_e pc_a : Addr) (wreq wstatus : Word)
     (φ : language.val griotte_lang → iPropI Σ) :
 
-    let start := allocator_free_block_addr pc_a 5 in
-    let code := allocator_free_instrs_n 5 in
+    let start := allocator_free_block_addr pc_a 9 in
+    let code := allocator_free_instrs_n 9 in
     ContiguousRegion pc_a (length allocator_free_instrs) ->
     SubBounds pc_b pc_e pc_a (pc_a ^+ length allocator_free_instrs)%a ->
     disjoint_from_shadow pc_b pc_e ->
 
-    ▷ PC ↦ᵣ WCap true RX Global pc_b pc_e start
-    ∗ ▷ ca0 ↦ᵣ wreq
-    ∗ ▷ ca1 ↦ᵣ wstatus
-    ∗ ▷ codefrag start code
-    ∗ ▷ (PC ↦ᵣ WCap true RX Global pc_b pc_e
-           (allocator_free_block_addr pc_a 7)
-         ∗ ca0 ↦ᵣ WInt 0
-         ∗ ca1 ↦ᵣ WInt ALLOC_OK
-         ∗ codefrag start code
+    PC ↦ᵣ WCap true RX Global pc_b pc_e start ∗
+    ca0 ↦ᵣ wreq ∗
+    ca1 ↦ᵣ wstatus ∗
+    codefrag start code ∗
+    ▷ (PC ↦ᵣ WCap true RX Global pc_b pc_e
+           (allocator_free_block_addr pc_a 11) ∗
+         ca0 ↦ᵣ WInt 0 ∗
+         ca1 ↦ᵣ WInt ALLOC_OK ∗
+         codefrag start code
          -∗ WP Seq (Instr Executable) @ E {{ φ }})
     ⊢ WP Seq (Instr Executable) @ E {{ φ }}.
   Proof.
     intros start code Hcont Hpc Hshadow; subst start code.
-    iIntros "(>HPC & >Hca0 & >Hca1 & >Hcode & Hφ)".
+    iIntros "(HPC & Hca0 & Hca1 & Hcode & Hφ)".
     codefrag_facts "Hcode".
     (* Mov ca0 0. *)
     iInstr "Hcode".
-    assert (Hstep : (pc_a ^+ 37)%a =
-      ((allocator_free_block_addr pc_a 5) ^+ 1)%a).
+    assert (Hstep : (pc_a ^+ 63)%a =
+      ((allocator_free_block_addr pc_a 9) ^+ 1)%a).
     { unfold allocator_free_block_addr. solve_addr. }
     iEval (rewrite Hstep) in "HPC".
     (* Mov ca1 ALLOC_OK. *)
     iInstr "Hcode".
     (* Jmp .free_return. *)
     iInstr "Hcode".
-    assert (Hret : (allocator_free_block_addr pc_a 5 ^+ 5)%a =
-      allocator_free_block_addr pc_a 7).
+    assert (Hret : (allocator_free_block_addr pc_a 9 ^+ 5)%a =
+      allocator_free_block_addr pc_a 11).
     { unfold allocator_free_block_addr. solve_addr. }
     iEval (rewrite Hret) in "HPC".
     iApply "Hφ". iFrame.
   Qed.
 
-  Lemma allocator_free_prepare_valid_spec
+  Local Lemma allocator_free_prepare_valid_spec
     (E : coPset)
     (pc_b pc_e pc_a next : Addr)
     (wreq w0 w1 w2 w3 : Word)
@@ -66,55 +709,56 @@ Section AllocatorFreeBlocks.
     ContiguousRegion pc_a (length allocator_free_instrs) ->
     SubBounds pc_b pc_e pc_a (pc_a ^+ length allocator_free_instrs)%a ->
     disjoint_from_shadow pc_b pc_e ->
-    allocator_free_valid next wreq ->
+    allocator_free_in_prefix next wreq ->
 
-    allocator_ctx
-    ∗ allocator_service_data next
-    ∗ ▷ PC ↦ᵣ WCap true RX Global pc_b pc_e pc_a
-    ∗ ▷ cgp ↦ᵣ WCap true RW Global
-        allocator_cgp_b allocator_cgp_e allocator_cgp_b
-    ∗ ▷ ca0 ↦ᵣ wreq
-    ∗ ▷ ct0 ↦ᵣ w0
-    ∗ ▷ ct1 ↦ᵣ w1
-    ∗ ▷ ct2 ↦ᵣ w2
-    ∗ ▷ ct3 ↦ᵣ w3
-    ∗ ▷ codefrag pc_a code
-    ∗ ▷ (allocator_service_data next
-         ∗ cgp ↦ᵣ WCap true RW Global
-             allocator_cgp_b allocator_cgp_e allocator_cgp_b
-         ∗ ca0 ↦ᵣ wreq
-         ∗ codefrag pc_a code
-         ∗ (∃ (p : Perm) (g : Locality) (b e a : Addr),
+    allocator_ctx ∗
+    allocator_service_data next ∗
+    PC ↦ᵣ WCap true RX Global pc_b pc_e pc_a ∗
+    cgp ↦ᵣ WCap true RW Global
+        allocator_cgp_b allocator_cgp_e allocator_cgp_b ∗
+    ca0 ↦ᵣ wreq ∗
+    ct0 ↦ᵣ w0 ∗
+    ct1 ↦ᵣ w1 ∗
+    ct2 ↦ᵣ w2 ∗
+    ct3 ↦ᵣ w3 ∗
+    codefrag pc_a code ∗
+    ▷ (allocator_service_data next ∗
+         cgp ↦ᵣ WCap true RW Global
+             allocator_cgp_b allocator_cgp_e allocator_cgp_b ∗
+         ca0 ↦ᵣ wreq ∗
+         codefrag pc_a code ∗
+         (∃ (p : Perm) (g : Locality) (b e a : Addr),
              ⌜wreq = WCap true p g b e a
-               ∧ (heap_b < b /\ b < e /\ e <= next)%a⌝
-             ∗ PC ↦ᵣ WCap true RX Global pc_b pc_e
-                 (allocator_free_block_addr pc_a 2)
-             ∗ ct0 ↦ᵣ WCap true RW Global heap_b heap_e next
-             ∗ ct1 ↦ᵣ WInt b
-             ∗ ct2 ↦ᵣ WInt e
-             ∗ ct3 ↦ᵣ WInt 0)
+               ∧ (heap_b < b /\ b < e /\ e <= next)%a⌝ ∗
+             PC ↦ᵣ WCap true RX Global pc_b pc_e
+                 (allocator_free_block_addr pc_a 2) ∗
+             ct0 ↦ᵣ WCap true RW Global heap_b heap_e next ∗
+             ct1 ↦ᵣ WInt b ∗
+             ct2 ↦ᵣ WInt e ∗
+             ct3 ↦ᵣ WInt 0)
          -∗ WP Seq (Instr Executable) @ E {{ φ }})
     ⊢ WP Seq (Instr Executable) @ E {{ φ }}.
   Proof.
     intros code Hlayout HE Hcont Hpc Hdisjoint (p & g & b & e & a & -> & Hbounds); subst code.
-    iIntros "(#Hctx & Hdata & >HPC & >Hcgp & >Hca0 & >Hct0 & >Hct1 & >Hct2 & >Hct3 & >Hcode & Hφ)".
-    iDestruct "Hdata" as "(%Hnext & Hslot & Hroot & Hfree)".
+    iIntros "(#Hctx & Hdata & HPC & Hcgp & Hca0 & Hct0 & Hct1 & Hct2 & Hct3 & Hcode & Hφ)".
+    iDestruct "Hdata" as (allocations)
+      "(%Hnext & Hslot & Hroot & Hfree & Hheaders & Hhistory)".
     codefrag_facts "Hcode".
     (* GetWType ct3 ca0. *)
     iInstr "Hcode".
     (* Sub ct3 ct3 (encodeWordType wt_cap). *)
     iInstr "Hcode".
     rewrite (encodeWordType_correct_cap true p g b e a true (O LG LM) Global 0%a 0%a 0%a) /wt_cap Z.sub_diag.
-    (* Jnz .free_invalid ct3 falls through for a capability. *)
+    (* Jnz .free_invalid ct3. *)
     iInstr "Hcode".
     (* GetTag ct3 ca0. *)
     iInstr "Hcode".
     (* Sub ct3 ct3 1. *)
     iInstr "Hcode".
     rewrite /Z.b2z Z.sub_diag.
-    (* Jnz .free_invalid ct3 falls through for a tagged capability. *)
+    (* Jnz .free_invalid ct3. *)
     iInstr "Hcode".
-    (* Load ct0 cgp reads the stored bump capability with its clear root shadow bit. *)
+    (* Load ct0 cgp. *)
     iInstr_lookup "Hcode" as "Hi" "Hcode".
     wp_instr.
     iInv Nallocator as ">Hbody" "Hclose".
@@ -166,26 +810,26 @@ Section AllocatorFreeBlocks.
     iInstr "Hcode".
     (* GetB ct3 ct0. *)
     iInstr "Hcode".
-    (* Lt ct3 ct3 ct1 tests heap_b < b. *)
+    (* Lt ct3 ct3 ct1. *)
     iInstr "Hcode".
     replace (heap_b <? b)%Z with true by (symmetry; apply Z.ltb_lt; solve_addr).
-    (* Jnz .free_base_ok ct3 skips the invalid jump. *)
+    (* Jnz .free_base_ok ct3. *)
     iInstr "Hcode".
-    (* Lt ct3 ct1 ct2 tests b < e. *)
+    (* Lt ct3 ct1 ct2. *)
     iInstr "Hcode".
     replace (b <? e)%Z with true by (symmetry; apply Z.ltb_lt; solve_addr).
-    (* Jnz .free_nonempty ct3 skips the invalid jump. *)
+    (* Jnz .free_nonempty ct3. *)
     iInstr "Hcode".
-    (* GetA ct3 ct0 reads the bump cursor. *)
+    (* GetA ct3 ct0. *)
     iInstr "Hcode".
-    (* Lt ct3 ct3 ct2 tests next < e. *)
+    (* Lt ct3 ct3 ct2. *)
     iInstr "Hcode".
     replace (next <? e)%Z with false by (symmetry; apply Z.ltb_ge; solve_addr).
-    (* Jnz .free_invalid ct3 falls through for e <= next. *)
+    (* Jnz .free_invalid ct3. *)
     iInstr "Hcode".
     iApply "Hφ".
-    iSplitL "Hslot Hroot Hfree".
-    { iFrame. done. }
+    iSplitL "Hslot Hroot Hfree Hheaders Hhistory".
+    { iExists allocations. iFrame. done. }
     iFrame "Hcgp Hca0 Hcode".
     iExists p, g, b, e, a.
     iSplit.
@@ -193,7 +837,7 @@ Section AllocatorFreeBlocks.
     iFrame.
   Qed.
 
-  Lemma allocator_free_prepare_invalid_spec
+  Local Lemma allocator_free_prepare_invalid_spec
     (E : coPset)
     (pc_b pc_e pc_a next : Addr)
     (wreq w0 w1 w2 w3 : Word)
@@ -205,36 +849,37 @@ Section AllocatorFreeBlocks.
     ContiguousRegion pc_a (length allocator_free_instrs) ->
     SubBounds pc_b pc_e pc_a (pc_a ^+ length allocator_free_instrs)%a ->
     disjoint_from_shadow pc_b pc_e ->
-    ¬ allocator_free_valid next wreq ->
+    ¬ allocator_free_in_prefix next wreq ->
 
-    allocator_ctx
-    ∗ allocator_service_data next
-    ∗ ▷ PC ↦ᵣ WCap true RX Global pc_b pc_e pc_a
-    ∗ ▷ cgp ↦ᵣ WCap true RW Global
-        allocator_cgp_b allocator_cgp_e allocator_cgp_b
-    ∗ ▷ ca0 ↦ᵣ wreq
-    ∗ ▷ ct0 ↦ᵣ w0
-    ∗ ▷ ct1 ↦ᵣ w1
-    ∗ ▷ ct2 ↦ᵣ w2
-    ∗ ▷ ct3 ↦ᵣ w3
-    ∗ ▷ codefrag pc_a code
-    ∗ ▷ (allocator_service_data next
-         ∗ cgp ↦ᵣ WCap true RW Global
-             allocator_cgp_b allocator_cgp_e allocator_cgp_b
-         ∗ ca0 ↦ᵣ wreq
-         ∗ codefrag pc_a code
-         ∗ PC ↦ᵣ WCap true RX Global pc_b pc_e
-             (allocator_free_block_addr pc_a 6)
-         ∗ ct0 ↦ᵣ -
-         ∗ ct1 ↦ᵣ -
-         ∗ ct2 ↦ᵣ -
-         ∗ ct3 ↦ᵣ -
+    allocator_ctx ∗
+    allocator_service_data next ∗
+    PC ↦ᵣ WCap true RX Global pc_b pc_e pc_a ∗
+    cgp ↦ᵣ WCap true RW Global
+        allocator_cgp_b allocator_cgp_e allocator_cgp_b ∗
+    ca0 ↦ᵣ wreq ∗
+    ct0 ↦ᵣ w0 ∗
+    ct1 ↦ᵣ w1 ∗
+    ct2 ↦ᵣ w2 ∗
+    ct3 ↦ᵣ w3 ∗
+    codefrag pc_a code ∗
+    ▷ (allocator_service_data next ∗
+         cgp ↦ᵣ WCap true RW Global
+             allocator_cgp_b allocator_cgp_e allocator_cgp_b ∗
+         ca0 ↦ᵣ wreq ∗
+         codefrag pc_a code ∗
+         PC ↦ᵣ WCap true RX Global pc_b pc_e
+             (allocator_free_block_addr pc_a 10) ∗
+         ct0 ↦ᵣ - ∗
+         ct1 ↦ᵣ - ∗
+         ct2 ↦ᵣ - ∗
+         ct3 ↦ᵣ -
          -∗ WP Seq (Instr Executable) @ E {{ φ }})
     ⊢ WP Seq (Instr Executable) @ E {{ φ }}.
   Proof.
     intros code Hlayout HE Hcont Hpc Hdisjoint Hrequest; subst code.
-    iIntros "(#Hctx & Hdata & >HPC & >Hcgp & >Hca0 & >Hct0 & >Hct1 & >Hct2 & >Hct3 & >Hcode & Hφ)".
-    iDestruct "Hdata" as "(%Hnext & Hslot & Hroot & Hfree)".
+    iIntros "(#Hctx & Hdata & HPC & Hcgp & Hca0 & Hct0 & Hct1 & Hct2 & Hct3 & Hcode & Hφ)".
+    iDestruct "Hdata" as (allocations)
+      "(%Hnext & Hslot & Hroot & Hfree & Hheaders & Hhistory)".
     codefrag_facts "Hcode".
     (* GetWType ct3 ca0. *)
     iInstr "Hcode".
@@ -244,7 +889,7 @@ Section AllocatorFreeBlocks.
     + destruct wreq; cbn in Hreq_cap; try done.
       destruct sb; cbn in Hreq_cap; try done.
       rewrite (encodeWordType_correct_cap tag p g b e a true (O LG LM) Global 0%a 0%a 0%a) /wt_cap Z.sub_diag.
-      (* Jnz .free_invalid ct3 falls through for a capability. *)
+      (* Jnz .free_invalid ct3. *)
       iInstr "Hcode".
       (* GetTag ct3 ca0. *)
       iInstr "Hcode".
@@ -252,9 +897,9 @@ Section AllocatorFreeBlocks.
       iInstr "Hcode".
       destruct tag.
       * rewrite /Z.b2z Z.sub_diag.
-        (* Jnz .free_invalid ct3 falls through for a tagged capability. *)
+        (* Jnz .free_invalid ct3. *)
         iInstr "Hcode".
-        (* Load ct0 cgp reads the stored bump capability with its clear root shadow bit. *)
+        (* Load ct0 cgp. *)
         iInstr_lookup "Hcode" as "Hi" "Hcode".
         wp_instr.
         iInv Nallocator as ">Hbody" "Hclose".
@@ -306,27 +951,27 @@ Section AllocatorFreeBlocks.
         iInstr "Hcode".
         (* GetB ct3 ct0. *)
         iInstr "Hcode".
-        (* Lt ct3 ct3 ct1 tests heap_b < b. *)
+        (* Lt ct3 ct3 ct1. *)
         iInstr "Hcode".
         destruct (decide (heap_b < b)%a) as [Hbase|Hbase].
         ** replace (heap_b <? b)%Z with true by (symmetry; apply Z.ltb_lt; solve_addr).
-          (* Jnz .free_base_ok ct3 skips the invalid jump. *)
+          (* Jnz .free_base_ok ct3. *)
           iInstr "Hcode".
-          (* Lt ct3 ct1 ct2 tests b < e. *)
+          (* Lt ct3 ct1 ct2. *)
           iInstr "Hcode".
           destruct (decide (b < e)%a) as [Hnonempty|Hempty].
           {
             replace (b <? e)%Z with true by (symmetry; apply Z.ltb_lt; solve_addr).
-            (* Jnz .free_nonempty ct3 skips the invalid jump. *)
+            (* Jnz .free_nonempty ct3. *)
             iInstr "Hcode".
-            (* GetA ct3 ct0 reads the bump cursor. *)
+            (* GetA ct3 ct0. *)
             iInstr "Hcode".
-            (* Lt ct3 ct3 ct2 tests next < e. *)
+            (* Lt ct3 ct3 ct2. *)
             iInstr "Hcode".
             destruct (decide (next < e)%a) as [Hpast|Hwithin].
             {
               replace (next <? e)%Z with true by (symmetry; apply Z.ltb_lt; solve_addr).
-              (* Jnz .free_invalid ct3 rejects e > next. *)
+              (* Jnz .free_invalid ct3. *)
               iInstr "Hcode".
               iApply "Hφ". iFrame. done.
             }
@@ -334,19 +979,19 @@ Section AllocatorFreeBlocks.
               exists p, g, b, e, a. split; first reflexivity. solve_addr. }
           }
           replace (b <? e)%Z with false by (symmetry; apply Z.ltb_ge; solve_addr).
-          (* Jnz .free_nonempty ct3 falls through for an empty interval. *)
+          (* Jnz .free_nonempty ct3. *)
           iInstr "Hcode".
-          (* Jmp .free_invalid rejects an empty interval. *)
+          (* Jmp .free_invalid. *)
           iInstr "Hcode".
           iApply "Hφ". iFrame. done.
         ** replace (heap_b <? b)%Z with false by (symmetry; apply Z.ltb_ge; solve_addr).
-          (* Jnz .free_base_ok ct3 falls through for an invalid base. *)
+          (* Jnz .free_base_ok ct3. *)
           iInstr "Hcode".
-          (* Jmp .free_invalid rejects a base outside the heap prefix. *)
+          (* Jmp .free_invalid. *)
           iInstr "Hcode".
           iApply "Hφ". iFrame. done.
       * cbn.
-        (* Jnz .free_invalid ct3 rejects an untagged capability. *)
+        (* Jnz .free_invalid ct3. *)
         iInstr "Hcode".
         iApply "Hφ". iFrame. done.
     + assert (Hnoncap : WInt (encodeWordType wreq - encodeWordType wt_cap) ≠ WInt 0).
@@ -358,32 +1003,27 @@ Section AllocatorFreeBlocks.
         destruct wreq; cbn in Hreq_cap, Hencode; try discriminate.
         all: try (destruct sb; cbn in Hreq_cap, Hencode; try discriminate); contradiction.
       }
-      (* Jnz .free_invalid ct3 rejects a non-capability word. *)
+      (* Jnz .free_invalid ct3. *)
       iInstr "Hcode".
       iApply "Hφ". iFrame. done.
   Qed.
-End AllocatorFreeBlocks.
 
-Section AllocatorFreeProof.
-  Context
-    {Σ : gFunctors}
-    {ceriseg : ceriseG Σ}
-    {allocatorg : allocatorG Σ}
-    {MP : MachineParameters}
-    {layout : allocatorLayout}
-    {layout_wf : allocatorLayoutWf}
-  .
+  Context {layout_wf : allocatorLayoutWf}.
 
-  (** Since the service invariant hides the bump cursor, this class of requests
-      is invalid for every possible cursor. It includes [WInt 0]. *)
-  Definition allocator_free_always_invalid (wreq : Word) : Prop :=
-    ∀ next : Addr,
-      (heap_b < next /\ next <= heap_e)%a →
-      ¬ allocator_free_valid next wreq.
+  (** Common call boundary for rejection. [P] carries the evidence for the
+      particular rejection and is returned unchanged. Other client resources
+      can be framed. *)
+
+
 
   Lemma allocator_memory_not_free_cell E a w :
-    ↑Nallocator ⊆ E -> a ∈ heap_addresses ->
-    allocator_ctx -∗ a ↦ₐ w -∗ free_cell_token a ={E}=∗ False.
+    ↑Nallocator ⊆ E ->
+    a ∈ heap_addresses ->
+    allocator_ctx -∗
+    a ↦ₐ w -∗
+    free_cell_token a
+    ={E}=∗
+    False.
   Proof.
     iIntros (HE Ha) "#Hctx Hmem Hfree".
     iInv Nallocator as ">Hbody" "Hclose".
@@ -399,7 +1039,11 @@ Section AllocatorFreeProof.
     a ∈ finz.seq_between b e ->
     a ∈ finz.seq_between next heap_e ->
     length ws = length (finz.seq_between b e) ->
-    allocator_ctx -∗ [[b,e]] ↦ₐ [[ws]] -∗ free_cells next heap_e ={E}=∗ False.
+    allocator_ctx -∗
+    [[b,e]] ↦ₐ [[ws]] -∗
+    free_cells next heap_e
+    ={E}=∗
+    False.
   Proof.
     iIntros (HE Ha Hmem_in Hfree_in Hlen) "#Hctx Hmem Hfree".
     destruct (list_elem_of_lookup_1 _ _ Hmem_in) as [i Hi].
@@ -415,8 +1059,13 @@ Section AllocatorFreeProof.
     (heap_b < b /\ b < e /\ e <= heap_e)%a ->
     (heap_b < next /\ next <= heap_e)%a ->
     length ws = length (finz.seq_between b e) ->
-    allocator_ctx -∗ [[b,e]] ↦ₐ [[ws]] -∗ free_cells next heap_e
-      ={E}=∗ ⌜(e <= next)%a⌝ ∗ [[b,e]] ↦ₐ [[ws]] ∗ free_cells next heap_e.
+    allocator_ctx -∗
+    [[b,e]] ↦ₐ [[ws]] -∗
+    free_cells next heap_e
+      ={E}=∗
+      ⌜(e <= next)%a⌝ ∗
+      [[b,e]] ↦ₐ [[ws]] ∗
+      free_cells next heap_e.
   Proof.
     iIntros (HE Hb Hnext Hlen) "#Hctx Hmem Hfree".
     destruct (decide (e <= next)%a) as [Hbound|Hbad].
@@ -434,16 +1083,282 @@ Section AllocatorFreeProof.
     iMod (allocator_range_free_contradiction E b e next a ws HE Ha_heap Ha_mem Ha_free Hlen with "Hctx Hmem Hfree") as %[].
   Qed.
 
+  Local Lemma allocator_free_reject_correct
+    (E : coPset) (wreq wret : Word) (P : iProp Σ)
+    (φ : language.val griotte_lang → iPropI Σ) :
+    (∀ next allocations,
+      (heap_b < next /\ next <= heap_e)%a ->
+      allocator_chain (heap_b ^+ 1)%a next allocations ->
+      allocator_history allocations -∗
+      P -∗
+      ⌜¬ allocator_free_valid next allocations wreq⌝) ->
+    ↑Nallocator ⊆ E ->
+    ↑Nallocator_service ⊆ E ->
+    ⊢ (
+       allocator_ctx ∗
+       allocator_service_ctx ∗
+       na_own cerise_nais E ∗
+       P ∗
+       PC ↦ᵣ WCap true RX Global allocator_pcc_b allocator_pcc_e
+         allocator_free_pcc_addr ∗
+       cgp ↦ᵣ WCap true RW Global
+         allocator_cgp_b allocator_cgp_e allocator_cgp_b ∗
+       cra ↦ᵣ wret ∗
+       ca0 ↦ᵣ wreq ∗
+       ca1 ↦ᵣ - ∗
+       ca2 ↦ᵣ - ∗
+       ct0 ↦ᵣ - ∗
+       ct1 ↦ᵣ - ∗
+       ct2 ↦ᵣ - ∗
+       ct3 ↦ᵣ - ∗
+       ct4 ↦ᵣ - ∗
+       ctp ↦ᵣ - ∗
+       cnull ↦ᵣ - ∗
+       ▷ (na_own cerise_nais E ∗
+       P ∗
+          PC ↦ᵣ updatePcPerm wret ∗
+          cgp ↦ᵣ WCap true RW Global
+            allocator_cgp_b allocator_cgp_e allocator_cgp_b ∗
+          cra ↦ᵣ wret ∗
+          ca0 ↦ᵣ WInt 0 ∗
+          ca1 ↦ᵣ WInt ALLOC_INVALID ∗
+          ca2 ↦ᵣ - ∗
+          ct0 ↦ᵣ - ∗
+          ct1 ↦ᵣ - ∗
+          ct2 ↦ᵣ - ∗
+          ct3 ↦ᵣ - ∗
+          ct4 ↦ᵣ - ∗
+          ctp ↦ᵣ - ∗
+          cnull ↦ᵣ WInt 0
+          -∗ WP Seq (Instr Executable) @ E {{ φ }})
+       -∗ WP Seq (Instr Executable) @ E {{ φ }})%I.
+  Proof.
+    intros Hreject_request HEheap HEservice.
+    iIntros "(#Hctx & #Hservice & Hna & HP & HPC & Hcgp & Hcra & Hca0 & Hca1 & Hca2 & Hct0 & Hct1 & Hct2 & Hct3 & Hct4 & Hctp & Hcnull & Hpost)".
+    (* Open the service invariant and recover the allocator code and state. *)
+    iMod (na_inv_acc with "Hservice Hna") as "(Hinv & Hna & Hclose)"; try exact HEservice.
+    iDestruct "Hinv" as ">[Hstatic Hdata]".
+    iDestruct "Hstatic" as "[Himports Hcode]".
+    iDestruct "Hdata" as (next) "Hdata".
+    iEval (rewrite /allocator_code) in "Hcode".
+    focus_block_nochangePC 1 "Hcode" as a_free Ha_free "Hfreecode" "Hcode_cont".
+    assert (Ha_eq : a_free = allocator_free_pcc_addr).
+    { pose proof allocator_size_imports as Himports_size.
+      unfold allocator_free_pcc_addr, allocator_free_pcc_off in *.
+      solve_addr. }
+    subst a_free.
+    (* Check the capability and its bounds. *)
+    assert (Hsplit : allocator_free_instrs =
+      (allocator_free_instrs_n 0 ++ allocator_free_instrs_n 1) ++
+      concat (encodeInstrsW <$> drop 2 assembled_allocator_free)) by reflexivity.
+    iEval (rewrite Hsplit) in "Hfreecode".
+    focus_block_0 "Hfreecode" as "Hprepare_code" "Hfree_cont".
+    assert (Hpc : SubBounds allocator_pcc_b allocator_pcc_e
+      allocator_free_pcc_addr (allocator_free_pcc_addr ^+ length allocator_free_instrs)%a).
+    { pose proof allocator_size_code as Hsize_code.
+      rewrite /allocator_code length_app in Hsize_code.
+      unfold allocator_free_pcc_addr, allocator_free_pcc_off in *.
+      solve_addr. }
+    assert (Hdisjoint : disjoint_from_shadow allocator_pcc_b allocator_pcc_e).
+    { pose proof allocator_regions_disjoint as Hregions.
+      unfold disjoint_from_shadow.
+      rewrite !disjoint_list_cons in Hregions.
+      cbn [union_list] in Hregions.
+      set_solver. }
+    iDestruct "Hct0" as (w0) "Hct0".
+    iDestruct "Hct1" as (w1) "Hct1".
+    iDestruct "Hct2" as (w2) "Hct2".
+    iDestruct "Hct3" as (w3) "Hct3".
+    iAssert ((P ∗
+      allocator_service_data next ∗
+      PC ↦ᵣ WCap true RX Global allocator_pcc_b allocator_pcc_e
+        (allocator_free_block_addr allocator_free_pcc_addr 10) ∗
+      cgp ↦ᵣ WCap true RW Global allocator_cgp_b allocator_cgp_e allocator_cgp_b ∗
+      ca0 ↦ᵣ wreq ∗
+      ct0 ↦ᵣ - ∗
+      ct1 ↦ᵣ - ∗
+      ct2 ↦ᵣ - ∗
+      ct3 ↦ᵣ - ∗
+      ct4 ↦ᵣ - ∗
+      ca2 ↦ᵣ - ∗
+      codefrag allocator_free_pcc_addr allocator_free_instrs) -∗
+      WP Seq (Instr Executable) @ E {{ φ }})%I
+      with "[- HP Hdata HPC Hcgp Hca0 Hct0 Hct1 Hct2 Hct3 Hct4 Hca2 Hprepare_code Hfree_cont]" as "Hreject".
+    { iIntros "(HP & Hdata & HPC & Hcgp & Hca0 & Hct0 & Hct1 & Hct2 & Hct3 & Hct4 & Hca2 & Hfreecode)".
+      iDestruct "Hct0" as (w0') "Hct0".
+      iDestruct "Hct1" as (w1') "Hct1".
+      iDestruct "Hct2" as (w2') "Hct2".
+      iDestruct "Hct3" as (w3') "Hct3".
+    (* The validity check rejects the request; set ALLOC_INVALID. *)
+    assert (Hsplit6 : allocator_free_instrs =
+      concat (encodeInstrsW <$> take 10 assembled_allocator_free) ++
+      (allocator_free_instrs_n 10 ++ allocator_free_instrs_n 11)) by reflexivity.
+    iEval (rewrite Hsplit6) in "Hfreecode".
+    focus_block_nochangePC 1 "Hfreecode" as a_invalid Ha_invalid "Hinvalid_code" "Hfreecode_cont".
+    assert (Haddr : a_invalid = allocator_free_block_addr allocator_free_pcc_addr 10).
+    { unfold allocator_free_block_addr in *. solve_addr. }
+    subst a_invalid.
+    (* Mov ca0 0. *)
+    iInstr "Hinvalid_code".
+    iDestruct "Hca1" as (wca1) "Hca1".
+    assert (Hstep : (allocator_free_pcc_addr ^+ 66)%a =
+      (allocator_free_block_addr allocator_free_pcc_addr 10 ^+ 1)%a)
+      by (unfold allocator_free_block_addr; solve_addr).
+    iEval (rewrite Hstep) in "HPC".
+    (* Mov ca1 ALLOC_INVALID. *)
+    iInstr_lookup "Hinvalid_code" as "Hi" "Hinvalid_code".
+    wp_instr.
+    iApply (wp_move_success_z with "[$HPC $Hi $Hca1]"); try solve_pure.
+    iIntros "!> (HPC & Hi & Hca1)". wp_pure.
+    iSpecialize ("Hinvalid_code" with "Hi").
+    iDestruct ("Hfreecode_cont" with "Hinvalid_code") as "Hfreecode".
+    iEval (rewrite -Hsplit6) in "Hfreecode".
+    (* Return to the caller and restore the service invariant. *)
+    assert (Hsplit7 : allocator_free_instrs =
+      concat (encodeInstrsW <$> take 11 assembled_allocator_free) ++
+      allocator_free_instrs_n 11) by reflexivity.
+    iEval (rewrite Hsplit7) in "Hfreecode".
+    focus_block_nochangePC 1 "Hfreecode" as a_ret Ha_ret "Hret_code" "Hfreecode_cont".
+    assert (Haddr : a_ret = allocator_free_block_addr allocator_free_pcc_addr 11).
+    { unfold allocator_free_block_addr in *. solve_addr. }
+    subst a_ret.
+    assert (Hret : (allocator_free_block_addr allocator_free_pcc_addr 10 ^+ 2)%a =
+      allocator_free_block_addr allocator_free_pcc_addr 11)
+      by (unfold allocator_free_block_addr; solve_addr).
+    iEval (rewrite Hret) in "HPC".
+    iDestruct "Hcnull" as (wnull) "Hcnull".
+    (* Jalr cnull cra. *)
+    iInstr "Hret_code".
+    iDestruct ("Hfreecode_cont" with "Hret_code") as "Hfreecode".
+    iEval (rewrite -Hsplit7) in "Hfreecode".
+    iDestruct ("Hcode_cont" with "Hfreecode") as "Hcode".
+    iEval (rewrite -/allocator_code) in "Hcode".
+    iMod ("Hclose" with "[Himports Hcode Hdata Hna]") as "Hna".
+    { iSplitR "Hna"; last iFrame.
+      iNext. iSplitL "Himports Hcode"; first iFrame.
+      iExists next. iFrame. }
+    iApply "Hpost". iFrame "∗".
+    }
+    destruct (decide (allocator_free_in_prefix next wreq)) as [Hprefix|Hprefix].
+    - iApply (allocator_free_prepare_valid_spec with
+        "[- $Hctx $Hdata $HPC $Hcgp $Hca0 $Hct0 $Hct1 $Hct2 $Hct3 $Hprepare_code]"); eauto.
+      iNext. iIntros "(Hdata & Hcgp & Hca0 & Hprepare_code & Hvalid)".
+      iDestruct "Hvalid" as (p g b e a) "(%Hvalid & HPC & Hct0 & Hct1 & Hct2 & Hct3)".
+      destruct Hvalid as [Heq Hbounds].
+      iDestruct "Hdata" as (entries) "(%Hcursor & Hslot & Hroot & Hfree & Hheaders & Hhistory)".
+      iDestruct (allocator_headers_chain_spec with "Hheaders") as %Hchain.
+      iDestruct (Hreject_request next entries Hcursor Hchain with "Hhistory HP") as %Hinvalid.
+      assert (Hmissing : ¬ allocator_has_bounds entries b e).
+      { intros Hmember. apply Hinvalid. exists p,g,b,e,a. auto. }
+      iDestruct ("Hfree_cont" with "Hprepare_code") as "Hfreecode".
+      iEval (rewrite -Hsplit) in "Hfreecode".
+      assert (Hsplit_search : allocator_free_instrs =
+        concat (encodeInstrsW <$> take 2 assembled_allocator_free) ++
+        (concat (encodeInstrsW <$> take 4 (drop 2 assembled_allocator_free)) ++
+         concat (encodeInstrsW <$> drop 6 assembled_allocator_free))) by reflexivity.
+      iEval (rewrite Hsplit_search) in "Hfreecode".
+      focus_block_nochangePC 1 "Hfreecode" as a_search Ha_search "Hsearchcode" "Hsearch_cont".
+      assert (Ha_search_eq : a_search = allocator_free_block_addr allocator_free_pcc_addr 2)
+        by (unfold allocator_free_block_addr in *; solve_addr).
+      subst a_search.
+      iDestruct "Hct4" as (w4) "Hct4".
+      iDestruct "Hca2" as (wa2) "Hca2".
+      iApply (allocator_free_search_missing_spec with
+        "[- $Hheaders $HPC $Hct0 $Hct1 $Hct2 $Hct3 $Hct4 $Hca2 $Hsearchcode]"); eauto.
+      iNext. iIntros "(Hheaders & Hct0 & Hct1 & Hct2 & Hct3 & Hct4 & Hca2 & Hsearchcode & Hresult)".
+      iDestruct "Hresult" as "(%Hmiss & HPC)".
+      iAssert (allocator_service_data next) with "[Hslot Hroot Hfree Hheaders Hhistory]" as "Hdata".
+      { iExists entries. iFrame. done. }
+      iDestruct ("Hsearch_cont" with "Hsearchcode") as "Hfreecode".
+      iEval (rewrite -Hsplit_search) in "Hfreecode".
+      iApply "Hreject". iFrame.
+    - iApply (allocator_free_prepare_invalid_spec with
+        "[- $Hctx $Hdata $HPC $Hcgp $Hca0 $Hct0 $Hct1 $Hct2 $Hct3 $Hprepare_code]"); eauto.
+      iNext. iIntros "(Hdata & Hcgp & Hca0 & Hprepare_code & HPC & Hct0 & Hct1 & Hct2 & Hct3)".
+      iDestruct ("Hfree_cont" with "Hprepare_code") as "Hfreecode".
+      iEval (rewrite -Hsplit) in "Hfreecode".
+      iApply "Hreject". iFrame.
+  Qed.
+
+  (** A strict subrange cannot be another allocation in the header chain.
+      The original receipt suffices, whether its payload is live or freed. *)
+
+  Lemma allocator_free_narrowed_spec
+    (E : coPset) (p : Perm) (g : Locality)
+    (b e : Addr) (reserved : Z) (b' e' a : Addr) (wret : Word)
+    (φ : language.val griotte_lang → iPropI Σ) :
+    (b <= b' /\ b' < e' /\ e' <= e)%a ->
+    (b', e') ≠ (b, e) ->
+    ↑Nallocator ⊆ E ->
+    ↑Nallocator_service ⊆ E ->
+    ⊢ (
+       allocator_ctx ∗
+       allocator_service_ctx ∗
+       na_own cerise_nais E ∗
+       (allocator_allocation b e reserved) ∗
+       PC ↦ᵣ WCap true RX Global allocator_pcc_b allocator_pcc_e
+         allocator_free_pcc_addr ∗
+       cgp ↦ᵣ WCap true RW Global
+         allocator_cgp_b allocator_cgp_e allocator_cgp_b ∗
+       cra ↦ᵣ wret ∗
+       ca0 ↦ᵣ (WCap true p g b' e' a) ∗
+       ca1 ↦ᵣ - ∗
+       ca2 ↦ᵣ - ∗
+       ct0 ↦ᵣ - ∗
+       ct1 ↦ᵣ - ∗
+       ct2 ↦ᵣ - ∗
+       ct3 ↦ᵣ - ∗
+       ct4 ↦ᵣ - ∗
+       ctp ↦ᵣ - ∗
+       cnull ↦ᵣ - ∗
+       ▷ (na_own cerise_nais E ∗
+       (allocator_allocation b e reserved) ∗
+          PC ↦ᵣ updatePcPerm wret ∗
+          cgp ↦ᵣ WCap true RW Global
+            allocator_cgp_b allocator_cgp_e allocator_cgp_b ∗
+          cra ↦ᵣ wret ∗
+          ca0 ↦ᵣ WInt 0 ∗
+          ca1 ↦ᵣ WInt ALLOC_INVALID ∗
+          ca2 ↦ᵣ - ∗
+          ct0 ↦ᵣ - ∗
+          ct1 ↦ᵣ - ∗
+          ct2 ↦ᵣ - ∗
+          ct3 ↦ᵣ - ∗
+          ct4 ↦ᵣ - ∗
+          ctp ↦ᵣ - ∗
+          cnull ↦ᵣ WInt 0
+          -∗ WP Seq (Instr Executable) @ E {{ φ }})
+       -∗ WP Seq (Instr Executable) @ E {{ φ }})%I.
+
+  Proof.
+    intros Hbounds Hneq HEheap HEservice.
+    eapply allocator_free_reject_correct; [|exact HEheap|exact HEservice].
+    intros next allocations Hnext Hchain.
+    iIntros "Hhistory #Hreceipt".
+    iDestruct (allocator_history_lookup_spec with "Hhistory Hreceipt") as %Hlookup.
+    assert (Horiginal : allocator_has_bounds allocations b e).
+    { exists reserved. apply elem_of_list_to_map_2. exact Hlookup. }
+    pose proof (allocator_chain_subrange_spec _ _ _ _ _ _ _
+      Hchain Horiginal Hbounds Hneq) as Hmissing.
+    iPureIntro. intros (p0 & g0 & b0 & e0 & a0 & Heq & Hprefix & Hmember).
+    inversion Heq; subst. contradiction.
+  Qed.
+
   (** A call with an invalid request leaves client memory untouched and returns
       [ALLOC_INVALID]. Other registers and resources can be framed. *)
+
   Lemma allocator_free_invalid_correct
     (E : coPset) (wreq wret : Word)
     (φ : language.val griotte_lang → iPropI Σ) :
 
-    ⊢ (⌜↑Nallocator ⊆ E⌝ -∗
-       ⌜↑Nallocator_service ⊆ E⌝ -∗
-       ⌜allocator_free_always_invalid wreq⌝ -∗
+    (∀ (next : Addr) (allocations : list allocator_header_entry),
+      (heap_b < next /\ next <= heap_e)%a ->
+      allocator_chain (heap_b ^+ 1)%a next allocations ->
+      ¬ allocator_free_valid next allocations wreq) ->
+    ↑Nallocator ⊆ E ->
+    ↑Nallocator_service ⊆ E ->
 
+    ⊢ (
        allocator_ctx ∗
        allocator_service_ctx ∗
        na_own cerise_nais E ∗
@@ -484,117 +1399,41 @@ Section AllocatorFreeProof.
           -∗ WP Seq (Instr Executable) @ E {{ φ }})
        -∗ WP Seq (Instr Executable) @ E {{ φ }})%I.
   Proof.
-    iIntros "%HEheap %HEservice %Hinvalid".
-    iIntros "(#Hctx & #Hservice & Hna & HPC & Hcgp & Hcra & Hca0 & Hca1 & Hca2 & Hct0 & Hct1 & Hct2 & Hct3 & Hct4 & Hctp & Hcnull & Hpost)".
-    (* Open the service invariant and recover the allocator code and state. *)
-    iMod (na_inv_acc with "Hservice Hna") as "(Hinv & Hna & Hclose)"; try exact HEservice.
-    iDestruct "Hinv" as ">[Hstatic Hdata]".
-    iDestruct "Hstatic" as "[Himports Hcode]".
-    iDestruct "Hdata" as (next) "Hdata".
-    iEval (rewrite /allocator_code) in "Hcode".
-    focus_block_nochangePC 1 "Hcode" as a_free Ha_free "Hfreecode" "Hcode_cont".
-    assert (Ha_eq : a_free = allocator_free_pcc_addr).
-    { pose proof allocator_size_imports as Himports_size.
-      unfold allocator_free_pcc_addr, allocator_free_pcc_off in *.
-      solve_addr. }
-    subst a_free.
-
-    (* Check the capability and its bounds. *)
-    assert (Hsplit : allocator_free_instrs =
-      (allocator_free_instrs_n 0 ++ allocator_free_instrs_n 1) ++
-      concat (encodeInstrsW <$> drop 2 assembled_allocator_free)) by reflexivity.
-    iEval (rewrite Hsplit) in "Hfreecode".
-    focus_block_0 "Hfreecode" as "Hprepare_code" "Hfree_cont".
-    assert (Hpc : SubBounds allocator_pcc_b allocator_pcc_e
-      allocator_free_pcc_addr (allocator_free_pcc_addr ^+ length allocator_free_instrs)%a).
-    { pose proof allocator_size_code as Hsize_code.
-      rewrite /allocator_code length_app in Hsize_code.
-      unfold allocator_free_pcc_addr, allocator_free_pcc_off in *.
-      solve_addr. }
-    assert (Hdisjoint : disjoint_from_shadow allocator_pcc_b allocator_pcc_e).
-    { pose proof allocator_regions_disjoint as Hregions.
-      unfold disjoint_from_shadow.
-      rewrite !disjoint_list_cons in Hregions.
-      cbn [union_list] in Hregions.
-      set_solver. }
-    iDestruct "Hct0" as (w0) "Hct0".
-    iDestruct "Hct1" as (w1) "Hct1".
-    iDestruct "Hct2" as (w2) "Hct2".
-    iDestruct "Hct3" as (w3) "Hct3".
-    iDestruct "Hdata" as "(%Hnext & Hslot & Hroot & Hfree)".
-    assert (Hrequest : ¬ allocator_free_valid next wreq).
-    { apply Hinvalid. exact Hnext. }
-    iAssert (allocator_service_data next) with "[Hslot Hroot Hfree]" as "Hdata".
-    { iFrame. iPureIntro. exact Hnext. }
-    iApply (allocator_free_prepare_invalid_spec with
-      "[- $Hctx $Hdata $HPC $Hcgp $Hca0 $Hct0 $Hct1 $Hct2 $Hct3 $Hprepare_code]"); eauto.
-    iNext. iIntros
-      "(Hdata & Hcgp & Hca0 & Hprepare_code & HPC & Hct0 & Hct1 & Hct2 & Hct3)".
-    iDestruct ("Hfree_cont" with "Hprepare_code") as "Hfreecode".
-    iEval (rewrite -Hsplit) in "Hfreecode".
-    (* The validity check rejects the request; set ALLOC_INVALID. *)
-    assert (Hsplit6 : allocator_free_instrs =
-      concat (encodeInstrsW <$> take 6 assembled_allocator_free) ++
-      (allocator_free_instrs_n 6 ++ allocator_free_instrs_n 7)) by reflexivity.
-    iEval (rewrite Hsplit6) in "Hfreecode".
-    focus_block_nochangePC 1 "Hfreecode" as a_invalid Ha_invalid "Hinvalid_code" "Hfreecode_cont".
-    assert (Haddr : a_invalid = allocator_free_block_addr allocator_free_pcc_addr 6).
-    { unfold allocator_free_block_addr in *. solve_addr. }
-    subst a_invalid.
-    (* Mov ca0 0. *)
-    iInstr "Hinvalid_code".
-    iDestruct "Hca1" as (wca1) "Hca1".
-    changePCto ((allocator_free_block_addr allocator_free_pcc_addr 6) ^+ 1)%a.
-    (* Mov ca1 ALLOC_INVALID. *)
-    iInstr_lookup "Hinvalid_code" as "Hi" "Hinvalid_code".
-    wp_instr.
-    iApply (wp_move_success_z with "[$HPC $Hi $Hca1]"); try solve_pure.
-    iIntros "!> (HPC & Hi & Hca1)". wp_pure.
-    iSpecialize ("Hinvalid_code" with "Hi").
-    iDestruct ("Hfreecode_cont" with "Hinvalid_code") as "Hfreecode".
-    iEval (rewrite -Hsplit6) in "Hfreecode".
-
-    (* Return to the caller and restore the service invariant. *)
-    assert (Hsplit7 : allocator_free_instrs =
-      concat (encodeInstrsW <$> take 7 assembled_allocator_free) ++
-      allocator_free_instrs_n 7) by reflexivity.
-    iEval (rewrite Hsplit7) in "Hfreecode".
-    focus_block_nochangePC 1 "Hfreecode" as a_ret Ha_ret "Hret_code" "Hfreecode_cont".
-    assert (Haddr : a_ret = allocator_free_block_addr allocator_free_pcc_addr 7).
-    { unfold allocator_free_block_addr in *. solve_addr. }
-    subst a_ret.
-    changePCto (allocator_free_block_addr allocator_free_pcc_addr 7).
-    iDestruct "Hcnull" as (wnull) "Hcnull".
-    (* Jalr cnull cra. *)
-    iInstr "Hret_code".
-    iDestruct ("Hfreecode_cont" with "Hret_code") as "Hfreecode".
-    iEval (rewrite -Hsplit7) in "Hfreecode".
-    iDestruct ("Hcode_cont" with "Hfreecode") as "Hcode".
-    iEval (rewrite -/allocator_code) in "Hcode".
-    iMod ("Hclose" with "[Himports Hcode Hdata Hna]") as "Hna".
-    { iSplitR "Hna"; last iFrame.
-      iNext. iSplitL "Himports Hcode"; first iFrame.
-      iExists next. iFrame. }
-    iApply "Hpost". iFrame "∗".
+    intros Hinvalid HEheap HEservice.
+    assert (Hreject : ∀ next allocations,
+      (heap_b < next /\ next <= heap_e)%a ->
+      allocator_chain (heap_b ^+ 1)%a next allocations ->
+      allocator_history allocations -∗
+      emp -∗
+      ⌜¬ allocator_free_valid next allocations wreq⌝).
+    { intros next allocations Hnext Hchain. iIntros "_ _".
+      iPureIntro. exact (Hinvalid next allocations Hnext Hchain). }
+    pose proof (allocator_free_reject_correct E wreq wret emp φ
+      Hreject HEheap HEservice) as Hcorrect.
+    rewrite !left_id in Hcorrect.
+    iApply Hcorrect.
   Qed.
 
-  (** Ownership of every cell in the capability's bounds witnesses a live
-      range in the allocated prefix. A successful call relinquishes that memory
-      and returns one reclaim token per cell. Permissions and cursor may vary. *)
+  (** The receipt fixes both original bounds; ownership of every payload cell
+      witnesses liveness. A successful call relinquishes that memory and
+      returns one reclaim token per cell. Permissions and cursor may vary. *)
+
   Lemma allocator_free_valid_correct
-    (E : coPset) (p : Perm) (g : Locality) (b e a : Addr)
+    (E : coPset) (p : Perm) (g : Locality) (b e a : Addr) (reserved : Z)
     (ws : list Word) (wret : Word)
     (φ : language.val griotte_lang → iPropI Σ) :
 
-    ⊢ (⌜↑Nallocator ⊆ E⌝ -∗
-       ⌜↑Nallocator_service ⊆ E⌝ -∗
-       ⌜(heap_b < b /\ b < e /\ e <= heap_e)%a⌝ -∗
-       ⌜length ws = length (finz.seq_between b e)⌝ -∗
+    ↑Nallocator ⊆ E ->
+    ↑Nallocator_service ⊆ E ->
+    (heap_b < b /\ b < e /\ e <= heap_e)%a ->
+    length ws = length (finz.seq_between b e) ->
+
+    ⊢ (
 
        allocator_ctx ∗
        allocator_service_ctx ∗
        na_own cerise_nais E ∗
-       [[b, e]] ↦ₐ [[ws]] ∗
+       allocator_allocation b e reserved ∗
 
        (* Initial register file. *)
        PC ↦ᵣ WCap true RX Global allocator_pcc_b allocator_pcc_e
@@ -612,8 +1451,10 @@ Section AllocatorFreeProof.
        ct4 ↦ᵣ - ∗
        ctp ↦ᵣ - ∗
        cnull ↦ᵣ - ∗
+       [[b, e]] ↦ₐ [[ws]] ∗
 
        ▷ (na_own cerise_nais E ∗
+          allocator_allocation b e reserved ∗
           PC ↦ᵣ updatePcPerm wret ∗
           cgp ↦ᵣ WCap true RW Global
             allocator_cgp_b allocator_cgp_e allocator_cgp_b ∗
@@ -633,19 +1474,19 @@ Section AllocatorFreeProof.
           -∗ WP Seq (Instr Executable) @ E {{ φ }})
        -∗ WP Seq (Instr Executable) @ E {{ φ }})%I.
   Proof.
-    iIntros "%HEheap %HEservice %Hbounds %Hlen".
-    iIntros "(#Hctx & #Hservice & Hna & Hmem & HPC & Hcgp & Hcra & Hca0 & Hca1 & Hca2 & Hct0 & Hct1 & Hct2 & Hct3 & Hct4 & Hctp & Hcnull & Hpost)".
+    intros HEheap HEservice Hbounds Hlen.
+    iIntros "(#Hctx & #Hservice & Hna & #Hreceipt & HPC & Hcgp & Hcra & Hca0 & Hca1 & Hca2 & Hct0 & Hct1 & Hct2 & Hct3 & Hct4 & Hctp & Hcnull & Hmem & Hpost)".
     (* Open the service invariant and recover the allocator code and state. *)
     iMod (na_inv_acc with "Hservice Hna") as "(Hinv & Hna & Hclose)"; try exact HEservice.
     iDestruct "Hinv" as ">[Hstatic Hdata]".
     iDestruct "Hstatic" as "[Himports Hcode]".
     iDestruct "Hdata" as (next) "Hdata".
-    iDestruct "Hdata" as "(%Hnext & Hslot & Hroot & Hfree)".
+    iDestruct "Hdata" as (allocations) "(%Hnext & Hslot & Hroot & Hfree & Hheaders & Hhistory)".
     (* Use ownership of the range to show that it lies below the bump cursor. *)
     iMod (allocator_owned_range_below_cursor E b e next ws HEheap Hbounds Hnext Hlen
       with "Hctx Hmem Hfree") as "(%Hend & Hmem & Hfree)".
-    iAssert (allocator_service_data next) with "[Hslot Hroot Hfree]" as "Hdata".
-    { iFrame. iPureIntro. exact Hnext. }
+    iAssert (allocator_service_data next) with "[Hslot Hroot Hfree Hheaders Hhistory]" as "Hdata".
+    { iExists allocations. iFrame. done. }
     iEval (rewrite /allocator_code) in "Hcode".
     focus_block_nochangePC 1 "Hcode" as a_free Ha_free "Hfreecode" "Hcode_cont".
     assert (Ha_eq : a_free = allocator_free_pcc_addr).
@@ -674,7 +1515,7 @@ Section AllocatorFreeProof.
     iDestruct "Hct1" as (w1) "Hct1".
     iDestruct "Hct2" as (w2) "Hct2".
     iDestruct "Hct3" as (w3) "Hct3".
-    assert (Hrequest : allocator_free_valid next (WCap true p g b e a)).
+    assert (Hrequest : allocator_free_in_prefix next (WCap true p g b e a)).
     { exists p, g, b, e, a. split; first reflexivity. solve_addr. }
     iApply (allocator_free_prepare_valid_spec with
       "[- $Hctx $Hdata $HPC $Hcgp $Hca0 $Hct0 $Hct1 $Hct2 $Hct3 $Hprepare_code]"); eauto.
@@ -684,22 +1525,48 @@ Section AllocatorFreeProof.
     destruct Hvalid as [Heq Hvalid]. inversion Heq; subst; clear Heq.
     iDestruct ("Hfree_cont" with "Hprepare_code") as "Hfreecode".
     iEval (rewrite -Hsplit) in "Hfreecode".
+    (* Follow authentic headers until both original bounds match. *)
+    iDestruct "Hdata" as (entries) "(%Hcursor & Hslot & Hroot & Hfree & Hheaders & Hhistory)".
+    iDestruct (allocator_headers_chain_spec with "Hheaders") as %Hchain.
+    iDestruct (allocator_history_lookup_spec with "Hhistory Hreceipt") as %Hlookup.
+    assert (Hmember : allocator_has_bounds entries b0 e0).
+    { exists reserved. apply elem_of_list_to_map_2. exact Hlookup. }
+    assert (Hsplit_search : allocator_free_instrs =
+      concat (encodeInstrsW <$> take 2 assembled_allocator_free) ++
+      (concat (encodeInstrsW <$> take 4 (drop 2 assembled_allocator_free)) ++
+       concat (encodeInstrsW <$> drop 6 assembled_allocator_free))) by reflexivity.
+    iEval (rewrite Hsplit_search) in "Hfreecode".
+    focus_block_nochangePC 1 "Hfreecode" as a_search Ha_search "Hsearchcode" "Hsearch_cont".
+    assert (Ha_search_eq : a_search = allocator_free_block_addr allocator_free_pcc_addr 2)
+      by (unfold allocator_free_block_addr in *; solve_addr).
+    subst a_search.
+    iDestruct "Hct4" as (w4) "Hct4".
+    iDestruct "Hca2" as (wa2) "Hca2".
+    iApply (allocator_free_search_found_spec with
+      "[- $Hheaders $HPC $Hct0 $Hct1 $Hct2 $Hct3 $Hct4 $Hca2 $Hsearchcode]"); eauto.
+    iNext. iIntros "(Hheaders & Hct0 & Hct1 & Hct2 & Hct3 & Hct4 & Hca2 & Hsearchcode & Hresult)".
+    iDestruct "Hresult" as "(%Hfound & HPC)".
+    iAssert (allocator_service_data next) with "[Hslot Hroot Hfree Hheaders Hhistory]" as "Hdata".
+    { iExists entries. iFrame. done. }
+    iDestruct ("Hsearch_cont" with "Hsearchcode") as "Hfreecode".
+    iEval (rewrite -Hsplit_search) in "Hfreecode".
+    iDestruct "Hct3" as (w3') "Hct3".
     (* Fetch the shadow capability and translate the range to free. *)
     assert (Hsplit2 : allocator_free_instrs =
-      concat (encodeInstrsW <$> take 2 assembled_allocator_free) ++
-      (allocator_free_instrs_n 2 ++
-       concat (encodeInstrsW <$> drop 3 assembled_allocator_free))) by reflexivity.
+      concat (encodeInstrsW <$> take 6 assembled_allocator_free) ++
+      (allocator_free_instrs_n 6 ++
+       concat (encodeInstrsW <$> drop 7 assembled_allocator_free))) by reflexivity.
     iEval (rewrite Hsplit2) in "Hfreecode".
     focus_block_nochangePC 1 "Hfreecode" as a_fetch Ha_fetch
       "Hfetch_code" "Hfreecode_cont".
-    assert (Haddr : a_fetch = allocator_free_block_addr allocator_free_pcc_addr 2).
+    assert (Haddr : a_fetch = allocator_free_block_addr allocator_free_pcc_addr 6).
     { unfold allocator_free_block_addr in *. solve_addr. }
     subst a_fetch.
     pose proof allocator_size_imports as Himports_size.
     iDestruct (region_pointsto_single with "Himports") as (v)
       "[Himport %Hentry]"; first exact Himports_size.
     cbn in Hentry. inversion Hentry; subst v.
-    assert (Hfetch_eq : allocator_free_instrs_n 2 =
+    assert (Hfetch_eq : allocator_free_instrs_n 6 =
       fetch.fetch_instrs allocator_shadow_import_off ctp ct3 ca2)
       by reflexivity.
     iEval (rewrite Hfetch_eq) in "Hfetch_code".
@@ -711,7 +1578,7 @@ Section AllocatorFreeProof.
     iApply (allocator_fetch_spec with
       "[- $HPC $Hctp $Hct3 $Hca2 $Hfetch_code $Himport]").
     { reflexivity. }
-    { rewrite -Hfetch_eq; exact H2. }
+    { rewrite -Hfetch_eq; assumption. }
     { apply withinBounds_true_iff; solve_addr. }
     { exact Hdisjoint. }
     { rewrite /is_heap_cap /heap_cap_base /memory_cap_base /=.
@@ -725,7 +1592,7 @@ Section AllocatorFreeProof.
     { discriminate. }
     { discriminate. }
     { discriminate. }
-    iNext. iIntros "(HPC & Hctp & Hct3 & Hca2 & Hfetch_code & Himport)".
+    iNext. iIntros "(HPC & Hctp & Hct3 & Hca2 & Himport & Hfetch_code)".
     iEval (cbn) in "Hctp".
     iEval (rewrite Himpaddr) in "Himport".
     iAssert ([[allocator_pcc_b,allocator_code_b]] ↦ₐ [[allocator_imports]])%I
@@ -737,50 +1604,57 @@ Section AllocatorFreeProof.
     iDestruct ("Hfreecode_cont" with "Hfetch_code") as "Hfreecode".
     iEval (rewrite -Hsplit2) in "Hfreecode".
     assert (Hsplit3 : allocator_free_instrs =
-      concat (encodeInstrsW <$> take 3 assembled_allocator_free) ++
-      (allocator_free_instrs_n 3 ++
-       concat (encodeInstrsW <$> drop 4 assembled_allocator_free))) by reflexivity.
+      concat (encodeInstrsW <$> take 7 assembled_allocator_free) ++
+      (allocator_free_instrs_n 7 ++
+       concat (encodeInstrsW <$> drop 8 assembled_allocator_free))) by reflexivity.
     iEval (rewrite Hsplit3) in "Hfreecode".
     focus_block_nochangePC 1 "Hfreecode" as a_translate Ha_translate
       "Htranslate_code" "Hfreecode_cont".
     assert (Haddr3 : a_translate =
-      allocator_free_block_addr allocator_free_pcc_addr 3).
+      allocator_free_block_addr allocator_free_pcc_addr 7).
     { unfold allocator_free_block_addr. solve_addr. }
     subst a_translate.
-    assert (Hpc3 : (allocator_free_block_addr allocator_free_pcc_addr 2 ^+
+    assert (Hpc3 : (allocator_free_block_addr allocator_free_pcc_addr 6 ^+
       length (fetch.fetch_instrs allocator_shadow_import_off ctp ct3 ca2))%a =
-      allocator_free_block_addr allocator_free_pcc_addr 3).
+      allocator_free_block_addr allocator_free_pcc_addr 7).
     { unfold allocator_free_block_addr. solve_addr. }
     iEval (rewrite Hpc3) in "HPC".
-    assert (Htranslate_eq : allocator_free_instrs_n 3 =
-      allocator_malloc_instrs_n 4) by reflexivity.
-    iEval (rewrite Htranslate_eq) in "Htranslate_code".
-    iApply (allocator_translate_spec with
-      "[- $HPC $Hct0 $Hct1 $Hct2 $Hct3 $Hctp $Hca2 $Htranslate_code]");
-      eauto; try solve_addr.
-    iNext. iIntros
-      "(HPC & Hct0 & Hct1 & Hct2 & Hct3 & Hctp & Hca2 & Htranslate_code)".
-    iEval (rewrite -Htranslate_eq) in "Htranslate_code".
+    pose (sb := (shadow_b ^+ (b0 - heap_b))%a).
+    assert (Hsb : (shadow_b + (b0 - heap_b))%a = Some sb).
+    { unfold sb. pose proof heap_shadow_same_size. solve_addr. }
+    assert (Hbtranslate : heap_to_shadow b0 = Some sb).
+    { rewrite allocator_translation_affine /translate_region.
+      assert (Hbheap : withinBounds heap_b heap_e b0 = true)
+        by (apply withinBounds_true_iff; solve_addr).
+      rewrite Hbheap. exact Hsb. }
+    destruct ws as [|v ws].
+    { exfalso. rewrite finz_seq_between_length /finz.dist /= in Hlen. solve_addr. }
+    assert (Hbnext : (b0 + 1)%a = Some (b0 ^+ 1)%a) by solve_addr.
+    assert (Hbnext_e : (b0 ^+ 1 <= e0)%a) by solve_addr.
+    iEval (rewrite (region_pointsto_cons _ _ _ _ _ Hbnext Hbnext_e)) in "Hmem".
+    iDestruct "Hmem" as "[Hb Hmemtail]".
+    iApply (allocator_free_shadow_check_spec _ _ _ _ _ _ _ sb ShadowLive with
+      "[- $Hctx $HPC $Hct0 $Hct1 $Hct2 $Hct3 $Hctp $Hca2 $Htranslate_code]");
+      try assumption; try solve_addr.
+    iSplitL "Hb". { iExists v. iFrame. }
+    iNext. iIntros "(Hb & Hct0 & Hct1 & Hct2 & Hctp & Htranslate_code & HPC & Hct3 & Hca2)".
+    iDestruct "Hb" as (v') "Hb".
+    iAssert ([[b0,e0]] ↦ₐ [[v' :: ws]])%I with "[Hb Hmemtail]" as "Hmem".
+    { rewrite (region_pointsto_cons _ _ _ _ _ Hbnext Hbnext_e). iFrame. }
     iDestruct ("Hfreecode_cont" with "Htranslate_code") as "Hfreecode".
     iEval (rewrite -Hsplit3) in "Hfreecode".
     (* Set the shadow bits and exchange memory ownership for reclaim tokens. *)
     assert (Hsplit4 : allocator_free_instrs =
-      concat (encodeInstrsW <$> take 4 assembled_allocator_free) ++
-      (allocator_free_instrs_n 4 ++
-       concat (encodeInstrsW <$> drop 5 assembled_allocator_free))) by reflexivity.
+      concat (encodeInstrsW <$> take 8 assembled_allocator_free) ++
+      (allocator_free_instrs_n 8 ++
+       concat (encodeInstrsW <$> drop 9 assembled_allocator_free))) by reflexivity.
     iEval (rewrite Hsplit4) in "Hfreecode".
     focus_block_nochangePC 1 "Hfreecode" as a_paint Ha_paint
       "Hpaint_code" "Hfreecode_cont".
     assert (Haddr4 : a_paint =
-      allocator_free_block_addr allocator_free_pcc_addr 4).
+      allocator_free_block_addr allocator_free_pcc_addr 8).
     { unfold allocator_free_block_addr. solve_addr. }
     subst a_paint.
-    assert (Hpc4 : (allocator_free_block_addr allocator_free_pcc_addr 3 ^+
-      length (allocator_malloc_instrs_n 4))%a =
-      allocator_free_block_addr allocator_free_pcc_addr 4).
-    { unfold allocator_free_block_addr. solve_addr. }
-    iEval (rewrite Hpc4) in "HPC".
-    pose (sb := (shadow_b ^+ (b0 - heap_b))%a).
     pose (se := (shadow_b ^+ (e0 - heap_b))%a).
     assert (Hshadow : (shadow_b <= sb /\ sb < se /\ se <= shadow_e)%a).
     { pose proof heap_shadow_same_size. unfold sb, se. solve_addr. }
@@ -793,15 +1667,15 @@ Section AllocatorFreeProof.
       assert (Hxheap : withinBounds heap_b heap_e x = true).
       { apply withinBounds_true_iff. solve_addr. }
       rewrite Hxheap. unfold sb. pose proof heap_shadow_same_size. solve_addr. }
-    assert (Hpaint_eq : allocator_free_instrs_n 4 =
+    assert (Hpaint_eq : allocator_free_instrs_n 8 =
       allocator_paint_instrs ctp ca2 ShadowQuarantined) by reflexivity.
     iEval (rewrite Hpaint_eq) in "Hpaint_code".
     iApply (allocator_paint_spec ShadowQuarantined ctp ca2 E RX Global
       allocator_pcc_b allocator_pcc_e
-      (allocator_free_block_addr allocator_free_pcc_addr 4) b0 e0 sb se ws
+      (allocator_free_block_addr allocator_free_pcc_addr 8) b0 e0 sb se (v' :: ws)
       with "[- $Hctx $HPC $Hctp $Hca2 $Hpaint_code $Hmem]").
     { reflexivity. }
-    { rewrite -Hpaint_eq; exact H6. }
+    { rewrite -Hpaint_eq; assumption. }
     { exact Hdisjoint. }
     { exact HEheap. }
     { solve_addr. }
@@ -814,35 +1688,35 @@ Section AllocatorFreeProof.
       constructor; [rewrite !elem_of_cons elem_of_nil; intuition congruence|];
       constructor; [apply not_elem_of_nil|];
       constructor. }
-    iNext. iIntros "(HPC & Hctp & Hca2 & Hpaint_code & Hreclaimed)".
+    iNext. iIntros "(HPC & Hctp & Hca2 & Hreclaimed & Hpaint_code)".
     iEval (rewrite -Hpaint_eq) in "Hpaint_code".
     iDestruct ("Hfreecode_cont" with "Hpaint_code") as "Hfreecode".
     iEval (rewrite -Hsplit4) in "Hfreecode".
     (* Set ALLOC_OK, then return and restore the service invariant. *)
     assert (Hsplit5 : allocator_free_instrs =
-      concat (encodeInstrsW <$> take 5 assembled_allocator_free) ++
-      (allocator_free_instrs_n 5 ++
-       concat (encodeInstrsW <$> drop 6 assembled_allocator_free))) by reflexivity.
+      concat (encodeInstrsW <$> take 9 assembled_allocator_free) ++
+      (allocator_free_instrs_n 9 ++
+       concat (encodeInstrsW <$> drop 10 assembled_allocator_free))) by reflexivity.
     iEval (rewrite Hsplit5) in "Hfreecode".
     focus_block_nochangePC 1 "Hfreecode" as a_success Ha_success
       "Hsuccess_code" "Hfreecode_cont".
     assert (Haddr5 : a_success =
-      allocator_free_block_addr allocator_free_pcc_addr 5).
+      allocator_free_block_addr allocator_free_pcc_addr 9).
     { unfold allocator_free_block_addr. solve_addr. }
     subst a_success.
-    assert (Hoff4 : allocator_free_block_addr allocator_free_pcc_addr 4 =
-      (allocator_free_pcc_addr ^+ 32)%a) by reflexivity.
-    assert (Hoff5 : allocator_free_block_addr allocator_free_pcc_addr 5 =
-      (allocator_free_pcc_addr ^+ 36)%a) by reflexivity.
+    assert (Hoff4 : allocator_free_block_addr allocator_free_pcc_addr 8 =
+      (allocator_free_pcc_addr ^+ 58)%a) by reflexivity.
+    assert (Hoff5 : allocator_free_block_addr allocator_free_pcc_addr 9 =
+      (allocator_free_pcc_addr ^+ 62)%a) by reflexivity.
     assert (Hlenpaint : length (allocator_paint_instrs ctp ca2 ShadowQuarantined) = 4)
       by reflexivity.
-    assert (Hpc5 : (allocator_free_block_addr allocator_free_pcc_addr 4 ^+
+    assert (Hpc5 : (allocator_free_block_addr allocator_free_pcc_addr 8 ^+
        length (allocator_paint_instrs ctp ca2 ShadowQuarantined))%a =
-       allocator_free_block_addr allocator_free_pcc_addr 5).
+       allocator_free_block_addr allocator_free_pcc_addr 9).
     { clear -Hoff4 Hoff5 Hlenpaint.
       rewrite Hoff4 Hoff5 Hlenpaint.
       rewrite incr_addr_opt_add_twice.
-      { replace (32 + 4)%Z with 36%Z by lia; reflexivity. }
+      { replace (58 + 4)%Z with 62%Z by lia; reflexivity. }
       all: lia. }
     iEval (rewrite Hpc5) in "HPC".
     iDestruct "Hca1" as (wca1) "Hca1".
@@ -852,17 +1726,17 @@ Section AllocatorFreeProof.
     iDestruct ("Hfreecode_cont" with "Hsuccess_code") as "Hfreecode".
     iEval (rewrite -Hsplit5) in "Hfreecode".
     assert (Hsplit7 : allocator_free_instrs =
-      concat (encodeInstrsW <$> take 7 assembled_allocator_free) ++
-      allocator_free_instrs_n 7) by reflexivity.
+      concat (encodeInstrsW <$> take 11 assembled_allocator_free) ++
+      allocator_free_instrs_n 11) by reflexivity.
     iEval (rewrite Hsplit7) in "Hfreecode".
     focus_block_nochangePC 1 "Hfreecode" as a_ret Ha_ret
       "Hret_code" "Hfreecode_cont".
     assert (Haddr7 : a_ret =
-      allocator_free_block_addr allocator_free_pcc_addr 7).
+      allocator_free_block_addr allocator_free_pcc_addr 11).
     { unfold allocator_free_block_addr. clear -Ha_ret.
       cbn [take concat fmap] in *. solve_addr. }
     subst a_ret.
-    assert (Hret_eq : allocator_free_instrs_n 7 =
+    assert (Hret_eq : allocator_free_instrs_n 11 =
       encodeInstrsW [Jalr cnull cra]) by reflexivity.
     iEval (rewrite Hret_eq) in "Hret_code".
     iDestruct "Hcnull" as (wnull) "Hcnull".
@@ -878,6 +1752,273 @@ Section AllocatorFreeProof.
     { iSplitR "Hna"; last iFrame.
       iNext. iSplitL "Himports Hcode"; first iFrame.
       iExists next. iFrame. }
-    iApply "Hpost". iFrame "∗".
+    iApply "Hpost". iFrame "Hreceipt ∗".
   Qed.
-End AllocatorFreeProof.
+
+  (** A still-tagged alias with exact original bounds reaches the shadow
+      check and is rejected. Only the first payload cell's reclaim token is
+      needed to justify that observation; the remaining tokens can be framed. *)
+
+  Lemma allocator_free_repeated_spec
+    (E : coPset) (p : Perm) (g : Locality)
+    (b e a : Addr) (reserved : Z) (wret : Word)
+    (φ : language.val griotte_lang → iPropI Σ) :
+    ↑Nallocator ⊆ E ->
+    ↑Nallocator_service ⊆ E ->
+    ⊢ (
+       allocator_ctx ∗
+       allocator_service_ctx ∗
+       na_own cerise_nais E ∗
+       allocator_allocation b e reserved ∗
+       PC ↦ᵣ WCap true RX Global allocator_pcc_b allocator_pcc_e
+         allocator_free_pcc_addr ∗
+       cgp ↦ᵣ WCap true RW Global
+         allocator_cgp_b allocator_cgp_e allocator_cgp_b ∗
+       cra ↦ᵣ wret ∗
+       ca0 ↦ᵣ (WCap true p g b e a) ∗
+       ca1 ↦ᵣ - ∗
+       ca2 ↦ᵣ - ∗
+       ct0 ↦ᵣ - ∗
+       ct1 ↦ᵣ - ∗
+       ct2 ↦ᵣ - ∗
+       ct3 ↦ᵣ - ∗
+       ct4 ↦ᵣ - ∗
+       ctp ↦ᵣ - ∗
+       cnull ↦ᵣ - ∗
+       reclaim_token b ∗
+       ▷ (na_own cerise_nais E ∗
+          allocator_allocation b e reserved ∗
+          PC ↦ᵣ updatePcPerm wret ∗
+          cgp ↦ᵣ WCap true RW Global
+            allocator_cgp_b allocator_cgp_e allocator_cgp_b ∗
+          cra ↦ᵣ wret ∗
+          ca0 ↦ᵣ WInt 0 ∗
+          ca1 ↦ᵣ WInt ALLOC_INVALID ∗
+          ca2 ↦ᵣ - ∗
+          ct0 ↦ᵣ - ∗
+          ct1 ↦ᵣ - ∗
+          ct2 ↦ᵣ - ∗
+          ct3 ↦ᵣ - ∗
+          ct4 ↦ᵣ - ∗
+          ctp ↦ᵣ - ∗
+          cnull ↦ᵣ WInt 0 ∗
+          reclaim_token b
+          -∗ WP Seq (Instr Executable) @ E {{ φ }})
+       -∗ WP Seq (Instr Executable) @ E {{ φ }})%I.
+
+  Proof.
+    intros HEheap HEservice.
+    iIntros "(#Hctx & #Hservice & Hna & #Hreceipt & HPC & Hcgp & Hcra & Hca0 & Hca1 & Hca2 & Hct0 & Hct1 & Hct2 & Hct3 & Hct4 & Hctp & Hcnull & Hreclaim & Hpost)".
+    (* Open the service invariant and recover the allocator code and state. *)
+    iMod (na_inv_acc with "Hservice Hna") as "(Hinv & Hna & Hclose)"; try exact HEservice.
+    iDestruct "Hinv" as ">[Hstatic Hdata]".
+    iDestruct "Hstatic" as "[Himports Hcode]".
+    iDestruct "Hdata" as (next) "Hdata".
+    iDestruct "Hdata" as (allocations) "(%Hnext & Hslot & Hroot & Hfree & Hheaders & Hhistory)".
+    iDestruct (allocator_headers_chain_spec with "Hheaders") as %Hinitial_chain.
+    iDestruct (allocator_history_lookup_spec with "Hhistory Hreceipt") as %Hinitial_lookup.
+    assert (Hinitial_member : (b, (e, reserved)) ∈ allocations).
+    { apply elem_of_list_to_map_2. exact Hinitial_lookup. }
+    pose proof (allocator_chain_member_bounds _ _ _ _ _ _ Hinitial_chain Hinitial_member) as Hentry_bounds.
+    assert (Hbounds : (heap_b < b /\ b < e /\ e <= heap_e)%a) by solve_addr.
+    assert (Hend : (e <= next)%a) by solve_addr.
+    iAssert (allocator_service_data next) with "[Hslot Hroot Hfree Hheaders Hhistory]" as "Hdata".
+    { iExists allocations. iFrame. done. }
+    iEval (rewrite /allocator_code) in "Hcode".
+    focus_block_nochangePC 1 "Hcode" as a_free Ha_free "Hfreecode" "Hcode_cont".
+    assert (Ha_eq : a_free = allocator_free_pcc_addr).
+    { pose proof allocator_size_imports as Himports_size.
+      unfold allocator_free_pcc_addr, allocator_free_pcc_off in *. solve_addr. }
+    subst a_free.
+    (* Check the capability and its bounds. *)
+    assert (Hsplit : allocator_free_instrs =
+      (allocator_free_instrs_n 0 ++ allocator_free_instrs_n 1) ++
+      concat (encodeInstrsW <$> drop 2 assembled_allocator_free)) by reflexivity.
+    iEval (rewrite Hsplit) in "Hfreecode".
+    focus_block_0 "Hfreecode" as "Hprepare_code" "Hfree_cont".
+    assert (Hpc : SubBounds allocator_pcc_b allocator_pcc_e
+      allocator_free_pcc_addr (allocator_free_pcc_addr ^+ length allocator_free_instrs)%a).
+    { pose proof allocator_size_code as Hsize_code.
+      rewrite /allocator_code length_app in Hsize_code.
+      unfold allocator_free_pcc_addr, allocator_free_pcc_off in *.
+      solve_addr. }
+    assert (Hdisjoint : disjoint_from_shadow allocator_pcc_b allocator_pcc_e).
+    { pose proof allocator_regions_disjoint as Hregions.
+      unfold disjoint_from_shadow.
+      rewrite !disjoint_list_cons in Hregions.
+      cbn [union_list] in Hregions.
+      set_solver. }
+    iDestruct "Hct0" as (w0) "Hct0".
+    iDestruct "Hct1" as (w1) "Hct1".
+    iDestruct "Hct2" as (w2) "Hct2".
+    iDestruct "Hct3" as (w3) "Hct3".
+    assert (Hrequest : allocator_free_in_prefix next (WCap true p g b e a)).
+    { exists p, g, b, e, a. split; first reflexivity. solve_addr. }
+    iApply (allocator_free_prepare_valid_spec with
+      "[- $Hctx $Hdata $HPC $Hcgp $Hca0 $Hct0 $Hct1 $Hct2 $Hct3 $Hprepare_code]"); eauto.
+    iNext. iIntros "(Hdata & Hcgp & Hca0 & Hprepare_code & Hvalid)".
+    iDestruct "Hvalid" as (p0 g0 b0 e0 a0)
+      "(%Hvalid & HPC & Hct0 & Hct1 & Hct2 & Hct3)".
+    destruct Hvalid as [Heq Hvalid]. inversion Heq; subst; clear Heq.
+    iDestruct ("Hfree_cont" with "Hprepare_code") as "Hfreecode".
+    iEval (rewrite -Hsplit) in "Hfreecode".
+    (* Follow authentic headers until both original bounds match. *)
+    iDestruct "Hdata" as (entries) "(%Hcursor & Hslot & Hroot & Hfree & Hheaders & Hhistory)".
+    iDestruct (allocator_headers_chain_spec with "Hheaders") as %Hchain.
+    iDestruct (allocator_history_lookup_spec with "Hhistory Hreceipt") as %Hlookup.
+    assert (Hmember : allocator_has_bounds entries b0 e0).
+    { exists reserved. apply elem_of_list_to_map_2. exact Hlookup. }
+    assert (Hsplit_search : allocator_free_instrs =
+      concat (encodeInstrsW <$> take 2 assembled_allocator_free) ++
+      (concat (encodeInstrsW <$> take 4 (drop 2 assembled_allocator_free)) ++
+       concat (encodeInstrsW <$> drop 6 assembled_allocator_free))) by reflexivity.
+    iEval (rewrite Hsplit_search) in "Hfreecode".
+    focus_block_nochangePC 1 "Hfreecode" as a_search Ha_search "Hsearchcode" "Hsearch_cont".
+    assert (Ha_search_eq : a_search = allocator_free_block_addr allocator_free_pcc_addr 2)
+      by (unfold allocator_free_block_addr in *; solve_addr).
+    subst a_search.
+    iDestruct "Hct4" as (w4) "Hct4".
+    iDestruct "Hca2" as (wa2) "Hca2".
+    iApply (allocator_free_search_found_spec with
+      "[- $Hheaders $HPC $Hct0 $Hct1 $Hct2 $Hct3 $Hct4 $Hca2 $Hsearchcode]"); eauto.
+    iNext. iIntros "(Hheaders & Hct0 & Hct1 & Hct2 & Hct3 & Hct4 & Hca2 & Hsearchcode & Hresult)".
+    iDestruct "Hresult" as "(%Hfound & HPC)".
+    iAssert (allocator_service_data next) with "[Hslot Hroot Hfree Hheaders Hhistory]" as "Hdata".
+    { iExists entries. iFrame. done. }
+    iDestruct ("Hsearch_cont" with "Hsearchcode") as "Hfreecode".
+    iEval (rewrite -Hsplit_search) in "Hfreecode".
+    iDestruct "Hct3" as (w3') "Hct3".
+    (* Fetch the shadow capability and translate the range to free. *)
+    assert (Hsplit2 : allocator_free_instrs =
+      concat (encodeInstrsW <$> take 6 assembled_allocator_free) ++
+      (allocator_free_instrs_n 6 ++
+       concat (encodeInstrsW <$> drop 7 assembled_allocator_free))) by reflexivity.
+    iEval (rewrite Hsplit2) in "Hfreecode".
+    focus_block_nochangePC 1 "Hfreecode" as a_fetch Ha_fetch
+      "Hfetch_code" "Hfreecode_cont".
+    assert (Haddr : a_fetch = allocator_free_block_addr allocator_free_pcc_addr 6).
+    { unfold allocator_free_block_addr in *. solve_addr. }
+    subst a_fetch.
+    pose proof allocator_size_imports as Himports_size.
+    iDestruct (region_pointsto_single with "Himports") as (v)
+      "[Himport %Hentry]"; first exact Himports_size.
+    cbn in Hentry. inversion Hentry; subst v.
+    assert (Hfetch_eq : allocator_free_instrs_n 6 =
+      fetch.fetch_instrs allocator_shadow_import_off ctp ct3 ca2)
+      by reflexivity.
+    iEval (rewrite Hfetch_eq) in "Hfetch_code".
+    iDestruct "Hctp" as (wctp) "Hctp".
+    iDestruct "Hca2" as (wca2) "Hca2".
+    assert (Himpaddr : (allocator_pcc_b ^+ allocator_shadow_import_off)%a =
+      allocator_pcc_b) by (unfold allocator_shadow_import_off; solve_addr).
+    iEval (rewrite -Himpaddr) in "Himport".
+    iApply (allocator_fetch_spec with
+      "[- $HPC $Hctp $Hct3 $Hca2 $Hfetch_code $Himport]").
+    { reflexivity. }
+    { rewrite -Hfetch_eq; assumption. }
+    { apply withinBounds_true_iff; solve_addr. }
+    { exact Hdisjoint. }
+    { rewrite /is_heap_cap /heap_cap_base /memory_cap_base /=.
+      destruct (is_heap_address shadow_b) eqn:Hheap; last reflexivity.
+      exfalso. unfold is_heap_address in Hheap.
+      apply withinBounds_true_iff in Hheap;
+      pose proof heap_shadow_disjoint as Hd;
+      rewrite /disjoint_from_shadow elem_of_disjoint in Hd;
+      apply (Hd shadow_b); apply elem_of_finz_seq_between; try exact Hheap;
+      pose proof shadow_valid; solve_addr. }
+    { discriminate. }
+    { discriminate. }
+    { discriminate. }
+    iNext. iIntros "(HPC & Hctp & Hct3 & Hca2 & Himport & Hfetch_code)".
+    iEval (cbn) in "Hctp".
+    iEval (rewrite Himpaddr) in "Himport".
+    iAssert ([[allocator_pcc_b,allocator_code_b]] ↦ₐ [[allocator_imports]])%I
+      with "[Himport]" as "Himports".
+    { rewrite /allocator_imports /region_pointsto
+        (finz_seq_between_singleton allocator_pcc_b allocator_code_b Himports_size) /=.
+      iFrame. }
+    iEval (rewrite -Hfetch_eq) in "Hfetch_code".
+    iDestruct ("Hfreecode_cont" with "Hfetch_code") as "Hfreecode".
+    iEval (rewrite -Hsplit2) in "Hfreecode".
+    assert (Hsplit3 : allocator_free_instrs =
+      concat (encodeInstrsW <$> take 7 assembled_allocator_free) ++
+      (allocator_free_instrs_n 7 ++
+       concat (encodeInstrsW <$> drop 8 assembled_allocator_free))) by reflexivity.
+    iEval (rewrite Hsplit3) in "Hfreecode".
+    focus_block_nochangePC 1 "Hfreecode" as a_translate Ha_translate
+      "Htranslate_code" "Hfreecode_cont".
+    assert (Haddr3 : a_translate =
+      allocator_free_block_addr allocator_free_pcc_addr 7).
+    { unfold allocator_free_block_addr. solve_addr. }
+    subst a_translate.
+    assert (Hpc3 : (allocator_free_block_addr allocator_free_pcc_addr 6 ^+
+      length (fetch.fetch_instrs allocator_shadow_import_off ctp ct3 ca2))%a =
+      allocator_free_block_addr allocator_free_pcc_addr 7).
+    { unfold allocator_free_block_addr. solve_addr. }
+    iEval (rewrite Hpc3) in "HPC".
+    pose (sb := (shadow_b ^+ (b0 - heap_b))%a).
+    assert (Hsb : (shadow_b + (b0 - heap_b))%a = Some sb).
+    { unfold sb. pose proof heap_shadow_same_size. solve_addr. }
+    assert (Hbtranslate : heap_to_shadow b0 = Some sb).
+    { rewrite allocator_translation_affine /translate_region.
+      assert (Hbheap : withinBounds heap_b heap_e b0 = true)
+        by (apply withinBounds_true_iff; solve_addr).
+      rewrite Hbheap. exact Hsb. }
+    iApply (allocator_free_shadow_check_spec _ _ _ _ _ _ _ sb ShadowQuarantined with
+      "[- $Hctx $HPC $Hct0 $Hct1 $Hct2 $Hct3 $Hctp $Hca2 $Htranslate_code $Hreclaim]");
+      try assumption; try solve_addr.
+    iNext. iIntros "(Hreclaim & Hct0 & Hct1 & Hct2 & Hctp & Htranslate_code & HPC & Hct3 & Hca2)".
+    iDestruct ("Hfreecode_cont" with "Htranslate_code") as "Hfreecode".
+    iEval (rewrite -Hsplit3) in "Hfreecode".
+    (* The validity check rejects the request; set ALLOC_INVALID. *)
+    assert (Hsplit6 : allocator_free_instrs =
+      concat (encodeInstrsW <$> take 10 assembled_allocator_free) ++
+      (allocator_free_instrs_n 10 ++ allocator_free_instrs_n 11)) by reflexivity.
+    iEval (rewrite Hsplit6) in "Hfreecode".
+    focus_block_nochangePC 1 "Hfreecode" as a_invalid Ha_invalid "Hinvalid_code" "Hfreecode_cont".
+    assert (Haddr : a_invalid = allocator_free_block_addr allocator_free_pcc_addr 10).
+    { unfold allocator_free_block_addr in *. solve_addr. }
+    subst a_invalid.
+    (* Mov ca0 0. *)
+    iInstr "Hinvalid_code".
+    iDestruct "Hca1" as (wca1) "Hca1".
+    assert (Hstep : (allocator_free_pcc_addr ^+ 66)%a =
+      (allocator_free_block_addr allocator_free_pcc_addr 10 ^+ 1)%a)
+      by (unfold allocator_free_block_addr; solve_addr).
+    iEval (rewrite Hstep) in "HPC".
+    (* Mov ca1 ALLOC_INVALID. *)
+    iInstr_lookup "Hinvalid_code" as "Hi" "Hinvalid_code".
+    wp_instr.
+    iApply (wp_move_success_z with "[$HPC $Hi $Hca1]"); try solve_pure.
+    iIntros "!> (HPC & Hi & Hca1)". wp_pure.
+    iSpecialize ("Hinvalid_code" with "Hi").
+    iDestruct ("Hfreecode_cont" with "Hinvalid_code") as "Hfreecode".
+    iEval (rewrite -Hsplit6) in "Hfreecode".
+    (* Return to the caller and restore the service invariant. *)
+    assert (Hsplit7 : allocator_free_instrs =
+      concat (encodeInstrsW <$> take 11 assembled_allocator_free) ++
+      allocator_free_instrs_n 11) by reflexivity.
+    iEval (rewrite Hsplit7) in "Hfreecode".
+    focus_block_nochangePC 1 "Hfreecode" as a_ret Ha_ret "Hret_code" "Hfreecode_cont".
+    assert (Haddr : a_ret = allocator_free_block_addr allocator_free_pcc_addr 11).
+    { unfold allocator_free_block_addr in *. solve_addr. }
+    subst a_ret.
+    assert (Hret : (allocator_free_block_addr allocator_free_pcc_addr 10 ^+ 2)%a =
+      allocator_free_block_addr allocator_free_pcc_addr 11)
+      by (clear -H Hpc; unfold allocator_free_block_addr; solve_addr).
+    iEval (rewrite Hret) in "HPC".
+    iDestruct "Hcnull" as (wnull) "Hcnull".
+    (* Jalr cnull cra. *)
+    iInstr "Hret_code".
+    iDestruct ("Hfreecode_cont" with "Hret_code") as "Hfreecode".
+    iEval (rewrite -Hsplit7) in "Hfreecode".
+    iDestruct ("Hcode_cont" with "Hfreecode") as "Hcode".
+    iEval (rewrite -/allocator_code) in "Hcode".
+    iMod ("Hclose" with "[Himports Hcode Hdata Hna]") as "Hna".
+    { iSplitR "Hna"; last iFrame.
+      iNext. iSplitL "Himports Hcode"; first iFrame.
+      iExists next. iFrame. }
+    iApply "Hpost". iFrame "Hreceipt ∗".
+  Qed.
+
+End AllocatorFreeTraversal.
