theories/allocator/allocator_header_spec.v
@@ -1,0 +1,218 @@
+From iris.proofmode Require Import proofmode.
+From griotte.allocator Require Import allocator_preamble.
+
+From griotte Require Import proofmode.
+
+Lemma allocator_chain_bounds h stop allocations :
+  allocator_chain h stop allocations -> (h <= stop)%a.
+Proof.
+  destruct allocations as [| (b & e & reserved) rest]; simpl.
+  - intros ->. solve_addr.
+  - intros ((Hbase & Hbe & Hstop) & _).
+    unfold allocator_header_words in Hbase. solve_addr.
+Qed.
+
+Lemma allocator_chain_member_bounds h stop allocations b e reserved :
+  allocator_chain h stop allocations ->
+  (b, (e, reserved)) ∈ allocations ->
+  (h < b /\ b < e /\ e <= stop)%a.
+Proof.
+  revert h. induction allocations as [| (b0 & e0 & r0) rest IH]; intros h Hchain Hin.
+  - set_solver.
+  - destruct Hchain as ((Hbase & Hbe & Hstop) & Htail).
+    unfold allocator_header_words in Hbase.
+    rewrite elem_of_cons in Hin. destruct Hin as [Heq|Hin].
+    + injection Heq as -> -> ->. solve_addr.
+    + specialize (IH e0 Htail Hin). solve_addr.
+Qed.
+
+Lemma allocator_chain_nodup_spec :
+  ∀ h stop allocations,
+    allocator_chain h stop allocations ->
+    NoDup allocations.*1.
+Proof.
+  intros h stop allocations. revert h.
+  induction allocations as [| (b & e & reserved) rest IH]; intros h Hchain; simpl.
+  - constructor.
+  - destruct Hchain as ((Hbase & Hbe & He) & Htail).
+    constructor; last by apply (IH e).
+    intros Hin. apply list_elem_of_fmap in Hin.
+    destruct Hin as ((b' & e' & r') & Heq & Hin). simpl in Heq. subst b'.
+    pose proof (allocator_chain_member_bounds e stop rest b e' r' Htail Hin).
+    solve_addr.
+Qed.
+
+Lemma allocator_chain_lookup_spec :
+  ∀ h stop allocations b e reserved,
+    allocator_chain h stop allocations ->
+    ((list_to_map allocations : gmap Addr (Addr * Z)) !! b = Some (e, reserved) <->
+     (b, (e, reserved)) ∈ allocations).
+Proof.
+  intros h stop allocations b e reserved Hchain. split.
+  - apply elem_of_list_to_map_2.
+  - apply elem_of_list_to_map_1. eapply allocator_chain_nodup_spec; eauto.
+Qed.
+
+Lemma allocator_chain_subrange_spec :
+  ∀ h stop allocations b e b' e',
+    allocator_chain h stop allocations ->
+    allocator_has_bounds allocations b e ->
+    (b <= b' /\ b' < e' /\ e' <= e)%a ->
+    (b', e') ≠ (b, e) ->
+    ¬ allocator_has_bounds allocations b' e'.
+Proof.
+  intros h stop allocations. revert h.
+  induction allocations as [| (b0 & e0 & r0) rest IH];
+    intros h b e b' e' Hchain [r Hin] Hbounds Hneq [r' Hin'].
+  - set_solver.
+  - destruct Hchain as [Hhead Htail].
+    rewrite elem_of_cons in Hin. rewrite elem_of_cons in Hin'.
+    destruct Hin as [Heq|Hin]; destruct Hin' as [Heq'|Hin'].
+    + injection Heq as -> -> ->. injection Heq' as -> -> ->. done.
+    + injection Heq as -> -> ->.
+      pose proof (allocator_chain_member_bounds e0 stop rest b' e' r' Htail Hin').
+      solve_addr.
+    + injection Heq' as -> -> ->.
+      pose proof (allocator_chain_member_bounds e0 stop rest b e r Htail Hin).
+      solve_addr.
+    + eapply (IH e0 b e b' e' Htail); eauto; eexists; eassumption.
+Qed.
+
+Section AllocatorHeaderContracts.
+  Context {Σ : gFunctors} {ceriseg : ceriseG Σ}.
+
+  Lemma allocator_headers_chain_spec :
+    ∀ h stop allocations,
+      allocator_headers h stop allocations ⊢
+      ⌜allocator_chain h stop allocations⌝.
+  Proof.
+    intros h stop allocations. revert h.
+    induction allocations as [| (b & e & reserved) rest IH]; intros h; simpl.
+    - done.
+    - iIntros "(%Hbounds & (%Hbase & Hfirst & Hreserved) & Htail)".
+      iDestruct (IH with "Htail") as %Htail.
+      iPureIntro. split; [split|]; done.
+  Qed.
+
+  (** The split point is a header address or the terminal bump pointer.
+      This is the prefix/suffix decomposition used by the traversal loop. *)
+
+  Lemma allocator_headers_app_spec :
+    ∀ h stop prefix suffix,
+      allocator_headers h stop (prefix ++ suffix) ⊣⊢
+      ∃ middle : Addr,
+        allocator_headers h middle prefix ∗
+        allocator_headers middle stop suffix.
+  Proof.
+    intros h stop prefix. revert h.
+    induction prefix as [| (b & e & reserved) prefix IH]; intros h suffix; simpl.
+    - iSplit.
+      + iIntros "Htail". iExists h. iFrame. done.
+      + iIntros "(%middle & %Heq & Htail)". by subst middle.
+    - iSplit.
+      + iIntros "(%Hbounds & Hhead & Htail)".
+        iDestruct (IH with "Htail") as (middle) "[Hprefix Hsuffix]".
+        iDestruct (allocator_headers_chain_spec with "Hprefix") as %Hchain.
+        pose proof (allocator_chain_bounds e middle prefix Hchain) as Hmiddle.
+        iExists middle. iFrame "Hsuffix". simpl. iFrame "Hhead Hprefix".
+        iPureIntro. solve_addr.
+      + iIntros "(%middle & (%Hbounds & Hhead & Hprefix) & Hsuffix)".
+        iDestruct (allocator_headers_chain_spec with "Hsuffix") as %Hchain.
+        pose proof (allocator_chain_bounds middle stop suffix Hchain) as Hmiddle.
+        iSplit; first (iPureIntro; solve_addr). iFrame "Hhead".
+        iApply IH. iExists middle. iFrame.
+  Qed.
+
+  Lemma allocator_headers_snoc_spec :
+    ∀ first h b e reserved allocations,
+      allocator_header_bounds h e b e ->
+      allocator_headers first h allocations -∗
+      allocator_header h b e reserved -∗
+      allocator_headers first e (allocations ++ [(b, (e, reserved))]).
+  Proof.
+    intros first h b e reserved allocations [Hbase Hbounds].
+    iIntros "Hprefix Hhead". iApply allocator_headers_app_spec.
+    iExists h. iFrame "Hprefix". simpl. iFrame "Hhead". done.
+  Qed.
+
+End AllocatorHeaderContracts.
+
+Section AllocatorHistoryContracts.
+  Context {Σ : gFunctors} {allocator_historyg : allocatorHistoryG Σ}.
+
+  Lemma allocator_allocation_persistent_spec :
+    ∀ b e reserved, Persistent (allocator_allocation b e reserved).
+  Proof.
+    intros b e reserved. apply _.
+  Qed.
+
+  Lemma allocator_history_lookup_spec :
+    ∀ allocations b e reserved,
+      allocator_history allocations -∗
+      allocator_allocation b e reserved -∗
+      ⌜(list_to_map allocations : gmap Addr (Addr * Z)) !! b = Some (e, reserved)⌝.
+  Proof.
+    intros allocations b e reserved. apply ghost_map_lookup.
+  Qed.
+
+  Lemma allocator_history_insert_spec :
+    ∀ allocations b e reserved,
+      (list_to_map allocations : gmap Addr (Addr * Z)) !! b = None ->
+      allocator_history allocations
+      ==∗
+      allocator_history (allocations ++ [(b, (e, reserved))]) ∗
+      allocator_allocation b e reserved.
+  Proof.
+    intros allocations b e reserved Hfresh.
+    iIntros "Hhistory".
+    iMod (ghost_map_insert_persist b (e, reserved) with "Hhistory") as "[Hhistory Hreceipt]";
+      first exact Hfresh.
+    iModIntro. iFrame "Hreceipt".
+    rewrite /allocator_history list_to_map_app /= -insert_union_r; last exact Hfresh.
+    rewrite right_id. iExact "Hhistory".
+  Qed.
+
+End AllocatorHistoryContracts.
+
+Section AllocatorServiceContracts.
+  Context {Σ : gFunctors} {ceriseg : ceriseG Σ} {allocatorg : allocatorG Σ}
+    {allocator_historyg : allocatorHistoryG Σ}
+    {MP : MachineParameters} {layout : allocatorLayout}.
+
+  (** The bump slot already contains [e]: the executable store must precede
+      this logical publication. This update neither writes memory nor paints. *)
+
+  Lemma allocator_service_commit_spec :
+    ∀ next b e reserved allocations,
+      (heap_b < next)%a ->
+      allocator_header_bounds next heap_e b e ->
+      allocator_cgp_b ↦ₐ WCap true RW Global heap_b heap_e e -∗
+      free_cell_token heap_b -∗
+      free_cells e heap_e -∗
+      allocator_headers (heap_b ^+ 1)%a next allocations -∗
+      allocator_history allocations -∗
+      allocator_header next b e reserved
+      ==∗
+      allocator_service_data e ∗
+      allocator_allocation b e reserved.
+  Proof.
+    intros next b e reserved allocations Hnext [Hbase Hbounds].
+    iIntros "Hslot Hroot Hfree Hheaders Hhistory Hhead".
+    iDestruct (allocator_headers_chain_spec with "Hheaders") as %Hchain.
+    assert (Hfresh : (list_to_map allocations : gmap Addr (Addr * Z)) !! b = None).
+    { apply eq_None_not_Some. intros ((e' & r') & Hlookup).
+      apply elem_of_list_to_map_2 in Hlookup.
+      pose proof (allocator_chain_member_bounds (heap_b ^+ 1)%a next
+        allocations b e' r' Hchain Hlookup).
+      unfold allocator_header_words in Hbase. solve_addr. }
+    iMod (allocator_history_insert_spec with "Hhistory") as "[Hhistory Hreceipt]";
+      first exact Hfresh.
+    iModIntro. iFrame "Hreceipt".
+    iExists (allocations ++ [(b, (e, reserved))]).
+    iFrame "Hslot Hroot Hfree Hhistory".
+    iSplit; first (iPureIntro; unfold allocator_header_words in Hbase; solve_addr).
+    iApply (allocator_headers_snoc_spec with "Hheaders Hhead").
+    split; [exact Hbase|solve_addr].
+  Qed.
+
+End AllocatorServiceContracts.
