theories/allocator/allocator_macros_spec.v
@@ -5,6 +5,7 @@ From griotte.allocator Require Import allocator_preamble.
 (** Loop specifications. Fetch and return use the existing instruction/macro rules.
     Every loop requires a nonempty range because it stores before testing.
     Registers not mentioned in the contracts can be framed. *)
+
 Section AllocatorMacros.
   Context
     {Σ : gFunctors}
@@ -15,6 +16,7 @@ Section AllocatorMacros.
 
   (** The existing fetch macro proof specialized to an arbitrary WP mask, so
       allocator calls can keep the non-atomic service invariant open. *)
+
   Lemma allocator_fetch_spec
     (n : Z) (rdst rscratch1 rscratch2 : RegName) (E : coPset)
     (pc_p : Perm) (pc_g : Locality) (pc_b pc_e pc_a : Addr)
@@ -32,24 +34,24 @@ Section AllocatorMacros.
     rscratch1 ≠ cnull ->
     rscratch2 ≠ cnull ->
 
-    ▷ PC ↦ᵣ WCap true pc_p pc_g pc_b pc_e pc_a
-    ∗ ▷ rdst ↦ᵣ wdst
-    ∗ ▷ rscratch1 ↦ᵣ w1
-    ∗ ▷ rscratch2 ↦ᵣ w2
-    ∗ ▷ codefrag pc_a code
-    ∗ ▷ (pc_b ^+ n)%a ↦ₐ wentry
-    ∗ ▷ (PC ↦ᵣ WCap true pc_p pc_g pc_b pc_e pc_end
-         ∗ rdst ↦ᵣ load_word pc_p wentry
-         ∗ rscratch1 ↦ᵣ WInt 0
-         ∗ rscratch2 ↦ᵣ WInt 0
-         ∗ codefrag pc_a code
-         ∗ (pc_b ^+ n)%a ↦ₐ wentry
+    PC ↦ᵣ WCap true pc_p pc_g pc_b pc_e pc_a ∗
+    rdst ↦ᵣ wdst ∗
+    rscratch1 ↦ᵣ w1 ∗
+    rscratch2 ↦ᵣ w2 ∗
+    (pc_b ^+ n)%a ↦ₐ wentry ∗
+    codefrag pc_a code ∗
+    ▷ (PC ↦ᵣ WCap true pc_p pc_g pc_b pc_e pc_end ∗
+         rdst ↦ᵣ load_word pc_p wentry ∗
+         rscratch1 ↦ᵣ WInt 0 ∗
+         rscratch2 ↦ᵣ WInt 0 ∗
+         (pc_b ^+ n)%a ↦ₐ wentry ∗
+         codefrag pc_a code
          -∗ WP Seq (Instr Executable) @ E {{ φ }})
     ⊢ WP Seq (Instr Executable) @ E {{ φ }}.
   Proof.
     intros code pc_end Hvpc Hcont Hpc_n Hdisjoint Hnonheap Hrdst Hr1 Hr2;
       subst code pc_end.
-    iIntros "(>HPC & >Hrdst & >Hscratch1 & >Hscratch2 & >Hcode & >Hentry & Hφ)".
+    iIntros "(HPC & Hrdst & Hscratch1 & Hscratch2 & Hentry & Hcode & Hφ)".
     codefrag_facts "Hcode".
     assert ((pc_a + (pc_b - pc_a))%a = Some pc_b) as Hlea by solve_addr.
     assert ((pc_b + n)%a = Some (pc_b ^+ n)%a) as Hpc_bn by solve_addr.
@@ -67,19 +69,19 @@ Section AllocatorMacros.
     SubBounds pc_b pc_e pc_a (pc_a ^+ length code)%a ->
     disjoint_from_shadow pc_b pc_e ->
 
-    ▷ PC ↦ᵣ WCap true RX Global pc_b pc_e pc_a
-    ∗ ▷ cra ↦ᵣ wret
-    ∗ ▷ cnull ↦ᵣ wnull
-    ∗ ▷ codefrag pc_a code
-    ∗ ▷ (PC ↦ᵣ updatePcPerm wret
-         ∗ cra ↦ᵣ wret
-         ∗ cnull ↦ᵣ WInt 0
-         ∗ codefrag pc_a code
+    PC ↦ᵣ WCap true RX Global pc_b pc_e pc_a ∗
+    cra ↦ᵣ wret ∗
+    cnull ↦ᵣ wnull ∗
+    codefrag pc_a code ∗
+    ▷ (PC ↦ᵣ updatePcPerm wret ∗
+         cra ↦ᵣ wret ∗
+         cnull ↦ᵣ WInt 0 ∗
+         codefrag pc_a code
          -∗ WP Seq (Instr Executable) @ E {{ φ }})
     ⊢ WP Seq (Instr Executable) @ E {{ φ }}.
   Proof.
     intros code Hpc Hdisjoint; subst code.
-    iIntros "(>HPC & >Hcra & >Hcnull & >Hcode & Hφ)".
+    iIntros "(HPC & Hcra & Hcnull & Hcode & Hφ)".
     codefrag_facts "Hcode".
     (* Jalr cnull cra. *)
     iInstr "Hcode".
@@ -101,25 +103,25 @@ Section AllocatorMacros.
     (heap_b <= b /\ b < e /\ e <= heap_e)%a ->
     NoDup [PC; cnull; rptr; rend; rtmp] ->
 
-    ▷ PC ↦ᵣ WCap true pc_p pc_g pc_b pc_e pc_a
-    ∗ ▷ rptr ↦ᵣ WCap true p g b e b
-    ∗ ▷ rend ↦ᵣ WInt (finz.to_z e)
-    ∗ ▷ rtmp ↦ᵣ wtmp
-    ∗ ▷ codefrag pc_a code
-    ∗ ▷ allocator_range_memory b e
-    ∗ ▷ (PC ↦ᵣ WCap true pc_p pc_g pc_b pc_e pc_end
-         ∗ rptr ↦ᵣ WCap true p g b e e
-         ∗ rend ↦ᵣ WInt (finz.to_z e)
-         ∗ rtmp ↦ᵣ WInt 0
-         ∗ codefrag pc_a code
-         ∗ ([∗ list] a ∈ finz.seq_between b e, a ↦ₐ WInt 0)
+    PC ↦ᵣ WCap true pc_p pc_g pc_b pc_e pc_a ∗
+    rptr ↦ᵣ WCap true p g b e b ∗
+    rend ↦ᵣ WInt (finz.to_z e) ∗
+    rtmp ↦ᵣ wtmp ∗
+    allocator_range_memory b e ∗
+    codefrag pc_a code ∗
+    ▷ (PC ↦ᵣ WCap true pc_p pc_g pc_b pc_e pc_end ∗
+         rptr ↦ᵣ WCap true p g b e e ∗
+         rend ↦ᵣ WInt (finz.to_z e) ∗
+         rtmp ↦ᵣ WInt 0 ∗
+         ([∗ list] a ∈ finz.seq_between b e, a ↦ₐ WInt 0) ∗
+         codefrag pc_a code
          -∗ WP Seq (Instr Executable) @ E {{ φ }})
     ⊢ WP Seq (Instr Executable) @ E {{ φ }}.
 
   Proof.
     intros code pc_end; subst code pc_end.
     iIntros (Hexec Hpc Hpc_shadow Hwrite Hheap Hregs)
-      "(>HPC & >Hptr & >Hend & >Htmp & >Hcode & >Hmem & Hφ)".
+      "(HPC & Hptr & Hend & Htmp & Hmem & Hcode & Hφ)".
     assert (Hrptr : rptr ≠ cnull) by (repeat rewrite NoDup_cons in Hregs; set_solver).
     assert (Hrend : rend ≠ cnull) by (repeat rewrite NoDup_cons in Hregs; set_solver).
     assert (Hrtmp : rtmp ≠ cnull) by (repeat rewrite NoDup_cons in Hregs; set_solver).
@@ -163,8 +165,7 @@ Section AllocatorMacros.
       rewrite (finz_seq_between_cons b e (proj1 (proj2 Hheap)))
         Hlast finz_seq_between_empty; last solve_addr.
       rewrite big_sepL_cons big_sepL_nil. iFrame.
-    - (* Jnz .allocator_zero rtmp repeats the loop. *)
-      iInstr_lookup "Hcode" as "Hi" "Hcode".
+    - (* Jnz .allocator_zero rtmp repeats the loop. *) iInstr_lookup "Hcode" as "Hi" "Hcode".
       wp_instr.
       iApply (wp_jnz_success_jmp_z with "[$HPC $Hi $Htmp]"); try solve_pure.
       { intros Hzero; inversion Hzero; solve_addr. }
@@ -173,10 +174,10 @@ Section AllocatorMacros.
       wp_pure.
       iSpecialize ("Hcode" with "Hi").
       iApply ("IH" $! (b ^+ 1)%a with
-        "[] [] HPC Hptr Hend Htmp Hcode Hmem [Ha Hφ]").
+        "[] [] HPC Hptr Hend Htmp Hmem Hcode [Ha Hφ]").
       { iPureIntro; solve_addr. }
       { iPureIntro; solve_addr. }
-      iNext. iIntros "(HPC & Hptr & Hend & Htmp & Hcode & Hzero)".
+      iNext. iIntros "(HPC & Hptr & Hend & Htmp & Hzero & Hcode)".
       iApply "Hφ"; iFrame.
       rewrite (finz_seq_between_cons b e (proj1 (proj2 Hheap))) big_sepL_cons.
       iFrame.
@@ -190,6 +191,7 @@ Section AllocatorMacros.
       The translation and length premises identify the shadow interval, including
       the one-past-end pointer reached by the final LEA but never dereferenced.
       The service layout supplies them when composing the allocator operations. *)
+
   Lemma allocator_paint_spec
     (status : AllocStatus) (rptr rcount : RegName) (E : coPset)
     (pc_p : Perm) (pc_g : Locality) (pc_b pc_e pc_a : Addr)
@@ -209,26 +211,26 @@ Section AllocatorMacros.
        heap_to_shadow a = Some (sb ^+ (finz.to_z a - finz.to_z b))%a) ->
     NoDup [PC; cnull; rptr; rcount] ->
 
-    allocator_ctx
-    ∗ ▷ PC ↦ᵣ WCap true pc_p pc_g pc_b pc_e pc_a
-    ∗ ▷ rptr ↦ᵣ WCap true RW Global shadow_b shadow_e sb
-    ∗ ▷ rcount ↦ᵣ WInt (finz.to_z e - finz.to_z b)
-    ∗ ▷ codefrag pc_a code
-    ∗ ▷ ([[b, e]] ↦ₐ [[ws]])
-    ∗ ▷ (PC ↦ᵣ WCap true pc_p pc_g pc_b pc_e pc_end
-         ∗ rptr ↦ᵣ WCap true RW Global shadow_b shadow_e se
-         ∗ rcount ↦ᵣ WInt 0
-         ∗ codefrag pc_a code
-         ∗ (match status with
+    allocator_ctx ∗
+    PC ↦ᵣ WCap true pc_p pc_g pc_b pc_e pc_a ∗
+    rptr ↦ᵣ WCap true RW Global shadow_b shadow_e sb ∗
+    rcount ↦ᵣ WInt (finz.to_z e - finz.to_z b) ∗
+    ([[b, e]] ↦ₐ [[ws]]) ∗
+    codefrag pc_a code ∗
+    ▷ (PC ↦ᵣ WCap true pc_p pc_g pc_b pc_e pc_end ∗
+         rptr ↦ᵣ WCap true RW Global shadow_b shadow_e se ∗
+         rcount ↦ᵣ WInt 0 ∗
+         (match status with
             | ShadowQuarantined => [∗ list] a ∈ finz.seq_between b e, reclaim_token a
             | ShadowLive => [[b, e]] ↦ₐ [[ws]]
-            end)
+            end) ∗
+         codefrag pc_a code
          -∗ WP Seq (Instr Executable) @ E {{ φ }})
     ⊢ WP Seq (Instr Executable) @ E {{ φ }}.
   Proof.
     intros code pc_end; subst code pc_end.
     iIntros (Hexec Hpc Hpc_shadow HE Hheap Hshadow Hlen Htranslate Hregs)
-      "(#Halloc & >HPC & >Hptr & >Hcount & >Hcode & >Hmem & Hφ)".
+      "(#Halloc & HPC & Hptr & Hcount & Hmem & Hcode & Hφ)".
     assert (Hrptr : rptr ≠ cnull) by
       (clear -Hregs; repeat rewrite NoDup_cons in Hregs; set_solver).
     assert (Hrcount : rcount ≠ cnull) by
@@ -308,8 +310,7 @@ Section AllocatorMacros.
       + rewrite (finz_seq_between_cons b e (proj1 (proj2 Hheap)))
           Hlast finz_seq_between_empty; last solve_addr.
         rewrite big_sepL_cons big_sepL_nil. iFrame.
-    - (* Jnz .allocator_paint rcount repeats the loop. *)
-      iInstr_lookup "Hcode" as "Hi" "Hcode".
+    - (* Jnz .allocator_paint rcount repeats the loop. *) iInstr_lookup "Hcode" as "Hi" "Hcode".
       wp_instr.
       iApply (wp_jnz_success_jmp_z with "[$HPC $Hi $Hcount]"); try solve_pure.
       { intros Hzero; inversion Hzero; solve_addr. }
@@ -319,14 +320,14 @@ Section AllocatorMacros.
       iSpecialize ("Hcode" with "Hi").
       replace (e - b - 1)%Z with (e - (b ^+ 1)%a)%Z by solve_addr.
       iApply ("IH" $! (b ^+ 1)%a (sb ^+ 1)%a ws with
-        "[] [] [] [] HPC Hptr Hcount Hcode Hmem [Ha Hφ]").
+        "[] [] [] [] HPC Hptr Hcount Hmem Hcode [Ha Hφ]").
       { iPureIntro; solve_addr. }
       { iPureIntro; solve_addr. }
       { iPureIntro; solve_addr. }
       { iPureIntro. intros a Ha_bounds.
         rewrite (Htranslate a); last solve_addr.
         f_equal. clear -Hheap Hshadow Hlen Hbnext Ha_bounds. solve_addr. }
-      iNext. iIntros "(HPC & Hptr & Hcount & Hcode & Hpainted)".
+      iNext. iIntros "(HPC & Hptr & Hcount & Hpainted & Hcode)".
       iApply "Hφ"; iFrame.
       destruct status.
       + rewrite (region_pointsto_cons b (b ^+ 1)%a e w ws Hbnext Hbnext_e).
@@ -334,8 +335,10 @@ Section AllocatorMacros.
       + rewrite (finz_seq_between_cons b e (proj1 (proj2 Hheap))) big_sepL_cons.
         iFrame.
   Qed.
+
   (** Translate a heap interval to its shadow interval. The instruction list
       is shared by malloc block 4 and free block 3. *)
+
   Lemma allocator_translate_spec
     (E : coPset)
     (pc_b pc_e pc_a next b e : Addr) (w3 wa2 : Word)
@@ -347,28 +350,28 @@ Section AllocatorMacros.
     disjoint_from_shadow pc_b pc_e ->
     (heap_b <= b /\ b < e /\ e <= heap_e)%a ->
 
-    ▷ PC ↦ᵣ WCap true RX Global pc_b pc_e pc_a
-    ∗ ▷ ct0 ↦ᵣ WCap true RW Global heap_b heap_e next
-    ∗ ▷ ct1 ↦ᵣ WInt b
-    ∗ ▷ ct2 ↦ᵣ WInt e
-    ∗ ▷ ct3 ↦ᵣ w3
-    ∗ ▷ ctp ↦ᵣ WCap true RW Global shadow_b shadow_e shadow_b
-    ∗ ▷ ca2 ↦ᵣ wa2
-    ∗ ▷ codefrag pc_a code
-    ∗ ▷ (PC ↦ᵣ WCap true RX Global pc_b pc_e (pc_a ^+ length code)%a
-         ∗ ct0 ↦ᵣ WCap true RW Global heap_b heap_e next
-         ∗ ct1 ↦ᵣ WInt b
-         ∗ ct2 ↦ᵣ WInt e
-         ∗ ct3 ↦ᵣ WInt (b - heap_b)
-         ∗ ctp ↦ᵣ WCap true RW Global shadow_b shadow_e sb
-         ∗ ca2 ↦ᵣ WInt (e - b)
-         ∗ codefrag pc_a code
+    PC ↦ᵣ WCap true RX Global pc_b pc_e pc_a ∗
+    ct0 ↦ᵣ WCap true RW Global heap_b heap_e next ∗
+    ct1 ↦ᵣ WInt b ∗
+    ct2 ↦ᵣ WInt e ∗
+    ct3 ↦ᵣ w3 ∗
+    ctp ↦ᵣ WCap true RW Global shadow_b shadow_e shadow_b ∗
+    ca2 ↦ᵣ wa2 ∗
+    codefrag pc_a code ∗
+    ▷ (PC ↦ᵣ WCap true RX Global pc_b pc_e (pc_a ^+ length code)%a ∗
+         ct0 ↦ᵣ WCap true RW Global heap_b heap_e next ∗
+         ct1 ↦ᵣ WInt b ∗
+         ct2 ↦ᵣ WInt e ∗
+         ct3 ↦ᵣ WInt (b - heap_b) ∗
+         ctp ↦ᵣ WCap true RW Global shadow_b shadow_e sb ∗
+         ca2 ↦ᵣ WInt (e - b) ∗
+         codefrag pc_a code
          -∗ WP Seq (Instr Executable) @ E {{ φ }})
     ⊢ WP Seq (Instr Executable) @ E {{ φ }}.
 
   Proof.
     intros code sb Hpc Hdisjoint Hheap; subst code sb.
-    iIntros "(>HPC & >Hct0 & >Hct1 & >Hct2 & >Hct3 & >Hctp & >Hca2 & >Hcode & Hφ)".
+    iIntros "(HPC & Hct0 & Hct1 & Hct2 & Hct3 & Hctp & Hca2 & Hcode & Hφ)".
     codefrag_facts "Hcode".
     (* GetB ct3 ct0. *)
     iInstr "Hcode".
@@ -383,4 +386,5 @@ Section AllocatorMacros.
     iInstr "Hcode".
     iApply "Hφ". iFrame.
   Qed.
+
 End AllocatorMacros.
