theories/allocator/allocator_malloc_spec.v
@@ -1,18 +1,20 @@
 From iris.proofmode Require Import proofmode.
 From griotte Require Import rules proofmode memory_region.
 From griotte.allocator Require Import allocator_preamble
-  allocator_macros_spec allocator_resource_spec.
+  allocator_macros_spec allocator_resource_spec allocator_header_spec.
 
 (** Address of an assembled block relative to the entry point. *)
+
 Definition allocator_malloc_block_addr {MP : MachineParameters}
   (pc_a : Addr) (n : nat) : Addr :=
   (pc_a ^+ length (concat (take n assembled_allocator_malloc)))%a.
 
 Section AllocatorMallocBlocks.
   Context {Σ : gFunctors} {ceriseg : ceriseG Σ} {allocatorg : allocatorG Σ}
+    {allocator_historyg : allocatorHistoryG Σ}
     {MP : MachineParameters} {layout : allocatorLayout}.
 
-  Lemma allocator_malloc_size_check_valid_spec
+  Local Lemma allocator_malloc_size_check_valid_spec
     (E : coPset)
     (pc_b pc_e pc_a : Addr) (wreq wtmp : Word)
     (φ : language.val griotte_lang → iPropI Σ) :
@@ -23,27 +25,27 @@ Section AllocatorMallocBlocks.
     disjoint_from_shadow pc_b pc_e ->
     allocator_positive_size wreq ->
 
-    ▷ PC ↦ᵣ WCap true RX Global pc_b pc_e pc_a
-    ∗ ▷ ca0 ↦ᵣ wreq
-    ∗ ▷ ct3 ↦ᵣ wtmp
-    ∗ ▷ codefrag pc_a code
-    ∗ ▷ (ca0 ↦ᵣ wreq
-         ∗ ct3 ↦ᵣ -
-         ∗ codefrag pc_a code
-         ∗ PC ↦ᵣ WCap true RX Global pc_b pc_e
+    PC ↦ᵣ WCap true RX Global pc_b pc_e pc_a ∗
+    ca0 ↦ᵣ wreq ∗
+    ct3 ↦ᵣ wtmp ∗
+    codefrag pc_a code ∗
+    ▷ (ca0 ↦ᵣ wreq ∗
+         ct3 ↦ᵣ - ∗
+         codefrag pc_a code ∗
+         PC ↦ᵣ WCap true RX Global pc_b pc_e
              (allocator_malloc_block_addr pc_a 1)
          -∗ WP Seq (Instr Executable) @ E {{ φ }})
     ⊢ WP Seq (Instr Executable) @ E {{ φ }}.
   Proof.
     intros code Hcont Hpc Hdisjoint (n & -> & Hpositive); subst code.
-    iIntros "(>HPC & >Hca0 & >Hct3 & >Hcode & Hφ)".
+    iIntros "(HPC & Hca0 & Hct3 & Hcode & Hφ)".
     codefrag_facts "Hcode".
     (* GetWType ct3 ca0. *)
     iInstr "Hcode".
     (* Sub ct3 ct3 (encodeWordType wt_int). *)
     iInstr "Hcode".
     rewrite (encodeWordType_correct_int n 0) /wt_int Z.sub_diag.
-    (* Jnz .malloc_invalid ct3 falls through for an integer. *)
+    (* Jnz .malloc_invalid ct3. *)
     iInstr "Hcode".
     (* Lt ct3 0 ca0. *)
     iInstr "Hcode".
@@ -53,7 +55,7 @@ Section AllocatorMallocBlocks.
     iApply "Hφ". iFrame.
   Qed.
 
-  Lemma allocator_malloc_size_check_invalid_spec
+  Local Lemma allocator_malloc_size_check_invalid_spec
     (E : coPset)
     (pc_b pc_e pc_a : Addr) (wreq wtmp : Word)
     (φ : language.val griotte_lang → iPropI Σ) :
@@ -64,20 +66,20 @@ Section AllocatorMallocBlocks.
     disjoint_from_shadow pc_b pc_e ->
     ¬ allocator_positive_size wreq ->
 
-    ▷ PC ↦ᵣ WCap true RX Global pc_b pc_e pc_a
-    ∗ ▷ ca0 ↦ᵣ wreq
-    ∗ ▷ ct3 ↦ᵣ wtmp
-    ∗ ▷ codefrag pc_a code
-    ∗ ▷ (ca0 ↦ᵣ wreq
-         ∗ ct3 ↦ᵣ -
-         ∗ codefrag pc_a code
-         ∗ PC ↦ᵣ WCap true RX Global pc_b pc_e
+    PC ↦ᵣ WCap true RX Global pc_b pc_e pc_a ∗
+    ca0 ↦ᵣ wreq ∗
+    ct3 ↦ᵣ wtmp ∗
+    codefrag pc_a code ∗
+    ▷ (ca0 ↦ᵣ wreq ∗
+         ct3 ↦ᵣ - ∗
+         codefrag pc_a code ∗
+         PC ↦ᵣ WCap true RX Global pc_b pc_e
              (allocator_malloc_block_addr pc_a 7)
          -∗ WP Seq (Instr Executable) @ E {{ φ }})
     ⊢ WP Seq (Instr Executable) @ E {{ φ }}.
   Proof.
     intros code Hcont Hpc Hdisjoint Hinvalid; subst code.
-    iIntros "(>HPC & >Hca0 & >Hct3 & >Hcode & Hφ)".
+    iIntros "(HPC & Hca0 & Hct3 & Hcode & Hφ)".
     codefrag_facts "Hcode".
     (* GetWType ct3 ca0. *)
     iInstr "Hcode".
@@ -86,16 +88,16 @@ Section AllocatorMallocBlocks.
     destruct (is_z wreq) eqn:Hreq_z.
     - destruct wreq; cbn in *; try done.
       rewrite (encodeWordType_correct_int z 0) /wt_int Z.sub_diag.
-      (* Jnz .malloc_invalid ct3 falls through for an integer. *)
+      (* Jnz .malloc_invalid ct3. *)
       iInstr "Hcode".
       (* Lt ct3 0 ca0. *)
       iInstr "Hcode".
       destruct (decide (0 < z)%Z) as [Hzpos|Hznonpos].
       { exfalso. apply Hinvalid. exists z. split; [reflexivity|exact Hzpos]. }
       replace (0 <? z)%Z with false by (symmetry; apply Z.ltb_ge; lia).
-      (* Jnz .malloc_size_ok ct3 falls through. *)
+      (* Jnz .malloc_size_ok ct3. *)
       iInstr "Hcode".
-      (* Jmp .malloc_invalid leaves this block's code fragment. *)
+      (* Jmp .malloc_invalid. *)
       iInstr "Hcode".
       iApply "Hφ". iFrame.
     - assert (Hnonzero : WInt (encodeWordType wreq - encodeWordType (WInt 0)) ≠ WInt 0).
@@ -104,12 +106,12 @@ Section AllocatorMallocBlocks.
         assert (Heq : encodeWordType wreq = encodeWordType (WInt 0)) by lia.
         destruct wreq; cbn in Hreq_z, Hencode; try discriminate.
         all: try (destruct sb; cbn in Hencode); contradiction. }
-      (* Jnz .malloc_invalid ct3 leaves this block's code fragment. *)
+      (* Jnz .malloc_invalid ct3. *)
       iInstr "Hcode".
       iApply "Hφ". iFrame.
   Qed.
 
-  Lemma allocator_malloc_reject_block_spec
+  Local Lemma allocator_malloc_reject_block_spec
     (E : coPset) (pc_b pc_e pc_a : Addr) (wreq wstatus : Word)
     (φ : language.val griotte_lang → iPropI Σ) :
 
@@ -119,24 +121,24 @@ Section AllocatorMallocBlocks.
     SubBounds pc_b pc_e pc_a (pc_a ^+ length allocator_malloc_instrs)%a ->
     disjoint_from_shadow pc_b pc_e ->
 
-    ▷ PC ↦ᵣ WCap true RX Global pc_b pc_e start
-    ∗ ▷ ca0 ↦ᵣ wreq
-    ∗ ▷ ca1 ↦ᵣ wstatus
-    ∗ ▷ codefrag start code
-    ∗ ▷ (PC ↦ᵣ WCap true RX Global pc_b pc_e
-           (allocator_malloc_block_addr pc_a 9)
-         ∗ ca0 ↦ᵣ WInt 0
-         ∗ ca1 ↦ᵣ WInt ALLOC_INVALID
-         ∗ codefrag start code
+    PC ↦ᵣ WCap true RX Global pc_b pc_e start ∗
+    ca0 ↦ᵣ wreq ∗
+    ca1 ↦ᵣ wstatus ∗
+    codefrag start code ∗
+    ▷ (PC ↦ᵣ WCap true RX Global pc_b pc_e
+           (allocator_malloc_block_addr pc_a 9) ∗
+         ca0 ↦ᵣ WInt 0 ∗
+         ca1 ↦ᵣ WInt ALLOC_INVALID ∗
+         codefrag start code
          -∗ WP Seq (Instr Executable) @ E {{ φ }})
     ⊢ WP Seq (Instr Executable) @ E {{ φ }}.
   Proof.
     intros start code Hcont Hpc Hshadow; subst start code.
-    iIntros "(>HPC & >Hca0 & >Hca1 & >Hcode & Hφ)".
+    iIntros "(HPC & Hca0 & Hca1 & Hcode & Hφ)".
     codefrag_facts "Hcode".
     (* Mov ca0 0. *)
     iInstr "Hcode".
-    assert (Hstep : (pc_a ^+ 44)%a =
+    assert (Hstep : (pc_a ^+ 50)%a =
       ((allocator_malloc_block_addr pc_a 7) ^+ 1)%a).
     { unfold allocator_malloc_block_addr. solve_addr. }
     iEval (rewrite Hstep) in "HPC".
@@ -157,7 +159,7 @@ Section AllocatorMallocBlocks.
     iApply "Hφ". iFrame.
   Qed.
 
-  Lemma allocator_malloc_oom_block_spec
+  Local Lemma allocator_malloc_oom_block_spec
     (E : coPset) (pc_b pc_e pc_a : Addr) (wreq wstatus : Word)
     (φ : language.val griotte_lang → iPropI Σ) :
 
@@ -167,24 +169,24 @@ Section AllocatorMallocBlocks.
     SubBounds pc_b pc_e pc_a (pc_a ^+ length allocator_malloc_instrs)%a ->
     disjoint_from_shadow pc_b pc_e ->
 
-    ▷ PC ↦ᵣ WCap true RX Global pc_b pc_e start
-    ∗ ▷ ca0 ↦ᵣ wreq
-    ∗ ▷ ca1 ↦ᵣ wstatus
-    ∗ ▷ codefrag start code
-    ∗ ▷ (PC ↦ᵣ WCap true RX Global pc_b pc_e
-           (allocator_malloc_block_addr pc_a 9)
-         ∗ ca0 ↦ᵣ WInt 0
-         ∗ ca1 ↦ᵣ WInt ALLOC_NO_MEMORY
-         ∗ codefrag start code
+    PC ↦ᵣ WCap true RX Global pc_b pc_e start ∗
+    ca0 ↦ᵣ wreq ∗
+    ca1 ↦ᵣ wstatus ∗
+    codefrag start code ∗
+    ▷ (PC ↦ᵣ WCap true RX Global pc_b pc_e
+           (allocator_malloc_block_addr pc_a 9) ∗
+         ca0 ↦ᵣ WInt 0 ∗
+         ca1 ↦ᵣ WInt ALLOC_NO_MEMORY ∗
+         codefrag start code
          -∗ WP Seq (Instr Executable) @ E {{ φ }})
     ⊢ WP Seq (Instr Executable) @ E {{ φ }}.
   Proof.
     intros start code Hcont Hpc Hshadow; subst start code.
-    iIntros "(>HPC & >Hca0 & >Hca1 & >Hcode & Hφ)".
+    iIntros "(HPC & Hca0 & Hca1 & Hcode & Hφ)".
     codefrag_facts "Hcode".
     (* Mov ca0 0. *)
     iInstr "Hcode".
-    assert (Hstep : (pc_a ^+ 47)%a =
+    assert (Hstep : (pc_a ^+ 53)%a =
       ((allocator_malloc_block_addr pc_a 8) ^+ 1)%a).
     { unfold allocator_malloc_block_addr. solve_addr. }
     iEval (rewrite Hstep) in "HPC".
@@ -202,7 +204,7 @@ Section AllocatorMallocBlocks.
     iApply "Hφ". iFrame.
   Qed.
 
-  Lemma allocator_malloc_prepare_success_spec
+  Local Lemma allocator_malloc_prepare_success_spec
     (E : coPset)
     (pc_b pc_e pc_a next : Addr) (n : Z)
     (w0 w1 w2 w3 w4 wa2 : Word)
@@ -216,43 +218,46 @@ Section AllocatorMallocBlocks.
     SubBounds pc_b pc_e pc_a (pc_a ^+ length allocator_malloc_instrs)%a ->
     disjoint_from_shadow pc_b pc_e ->
     (0 < n)%Z ->
-    (n <= heap_e - next)%Z ->
+    (n + allocator_header_words <= heap_e - next)%Z ->
 
-    allocator_ctx
-    ∗ allocator_service_data next
-    ∗ ▷ PC ↦ᵣ WCap true RX Global pc_b pc_e start
-    ∗ ▷ cgp ↦ᵣ WCap true RW Global
-        allocator_cgp_b allocator_cgp_e allocator_cgp_b
-    ∗ ▷ ca0 ↦ᵣ WInt n
-    ∗ ▷ ct0 ↦ᵣ w0
-    ∗ ▷ ct1 ↦ᵣ w1
-    ∗ ▷ ct2 ↦ᵣ w2
-    ∗ ▷ ct3 ↦ᵣ w3
-    ∗ ▷ ct4 ↦ᵣ w4
-    ∗ ▷ ca2 ↦ᵣ wa2
-    ∗ ▷ codefrag start code
-    ∗ ▷ (allocator_service_data next
-         ∗ cgp ↦ᵣ WCap true RW Global
-             allocator_cgp_b allocator_cgp_e allocator_cgp_b
-         ∗ ca0 ↦ᵣ WInt n
-         ∗ ct0 ↦ᵣ WCap true RW Global heap_b heap_e next
-         ∗ ct1 ↦ᵣ WInt next
-         ∗ codefrag start code
-         ∗ (∃ finish : Addr,
-             ⌜(next + n)%a = Some finish
-               ∧ (next < finish /\ finish <= heap_e)%a⌝
-             ∗ PC ↦ᵣ WCap true RX Global pc_b pc_e
-                 (allocator_malloc_block_addr pc_a 2)
-             ∗ ct2 ↦ᵣ WInt finish
-             ∗ ct3 ↦ᵣ WInt 0
-             ∗ ct4 ↦ᵣ WCap true RW Global next finish next
-             ∗ ca2 ↦ᵣ WCap true RW Global next finish next)
+    allocator_ctx ∗
+    allocator_service_data next ∗
+    PC ↦ᵣ WCap true RX Global pc_b pc_e start ∗
+    cgp ↦ᵣ WCap true RW Global
+        allocator_cgp_b allocator_cgp_e allocator_cgp_b ∗
+    ca0 ↦ᵣ WInt n ∗
+    ct0 ↦ᵣ w0 ∗
+    ct1 ↦ᵣ w1 ∗
+    ct2 ↦ᵣ w2 ∗
+    ct3 ↦ᵣ w3 ∗
+    ct4 ↦ᵣ w4 ∗
+    ca2 ↦ᵣ wa2 ∗
+    codefrag start code ∗
+    ▷ ((∃ b finish : Addr,
+         ⌜(next + allocator_header_words)%a = Some b ∧
+           (b + n)%a = Some finish ∧
+           (b < finish /\ finish <= heap_e)%a⌝ ∗
+         allocator_service_pending next b finish ∗
+         allocator_range_memory b finish ∗
+         cgp ↦ᵣ WCap true RW Global
+             allocator_cgp_b allocator_cgp_e allocator_cgp_b ∗
+         ca0 ↦ᵣ WInt n ∗
+         ct0 ↦ᵣ WCap true RW Global heap_b heap_e next ∗
+         ct1 ↦ᵣ WInt b ∗
+         codefrag start code ∗
+         PC ↦ᵣ WCap true RX Global pc_b pc_e
+             (allocator_malloc_block_addr pc_a 2) ∗
+         ct2 ↦ᵣ WInt finish ∗
+         ct3 ↦ᵣ WInt 0 ∗
+         ct4 ↦ᵣ WCap true RW Global b finish b ∗
+         ca2 ↦ᵣ WCap true RW Global b finish b)
          -∗ WP Seq (Instr Executable) @ E {{ φ }})
     ⊢ WP Seq (Instr Executable) @ E {{ φ }}.
   Proof.
     intros start code Hlayout HE Hcont Hpc Hdisjoint Hpositive Hroom; subst start code.
-    iIntros "(#Hctx & Hdata & >HPC & >Hcgp & >Hca0 & >Hct0 & >Hct1 & >Hct2 & >Hct3 & >Hct4 & >Hca2 & >Hcode & Hφ)".
-    iDestruct "Hdata" as "(%Hnext & Hslot & Hroot & Hfree)".
+    iIntros "(#Hctx & Hdata & HPC & Hcgp & Hca0 & Hct0 & Hct1 & Hct2 & Hct3 & Hct4 & Hca2 & Hcode & Hφ)".
+    iDestruct "Hdata" as (allocations)
+      "(%Hnext & Hslot & Hroot & Hfree & Hheaders & Hhistory)".
     codefrag_facts "Hcode".
     assert (Hstart : allocator_malloc_block_addr pc_a 1 = (pc_a ^+ 6)%a) by reflexivity.
     iEval (rewrite Hstart) in "Hcode".
@@ -261,6 +266,7 @@ Section AllocatorMallocBlocks.
 
     (* Load ct0 cgp: the reserved root token proves the stored heap
        capability's shadow bit is clear, so the load preserves its tag. *)
+    (* Load ct0 cgp. *)
     iInstr_lookup "Hcode" as "Hi" "Hcode".
     wp_instr.
     iInv Nallocator as ">Hbody" "Hclose".
@@ -290,45 +296,115 @@ Section AllocatorMallocBlocks.
     codefrag_facts "Hcode".
     assert (Hstep : (pc_a ^+ 7)%a = ((pc_a ^+ 6)%a ^+ 1)%a) by solve_addr.
     iEval (rewrite Hstep) in "HPC".
-    iEval (simpl) in "Hct0".
+    iEval (cbn [load_word]) in "Hct0".
+    unfold allocator_header_words in Hroom.
+    pose (b := (next ^+ 2)%a).
+    pose (finish := (b ^+ n)%a).
+    assert (Hbase : (next + 2)%a = Some b) by (unfold b; solve_addr).
+    assert (Hfinish : (b + n)%a = Some finish) by (unfold b, finish; solve_addr).
+    assert (Hrange : (next < b /\ b < finish /\ finish <= heap_e)%a)
+      by (unfold b, finish; solve_addr).
+    (* Read the bump bounds and reserve space for the header. *)
 
     (* GetA ct1 ct0. *)
     iInstr "Hcode".
     (* GetE ct2 ct0. *)
     iInstr "Hcode".
-    (* Sub ct3 ct2 ct1 computes remaining capacity. *)
+    (* Sub ct3 ct2 ct1. *)
     iInstr "Hcode".
-    (* Lt ct3 ct3 ca0 tests whether the request exceeds capacity. *)
+    (* Sub ct3 ct3 allocator_header_words. *)
     iInstr "Hcode".
-    replace (heap_e - next <? n)%Z with false by (symmetry; apply Z.ltb_ge; lia).
-    (* Jnz .malloc_no_memory ct3 falls through. *)
+    (* Lt ct3 ct3 ca0. *)
     iInstr "Hcode".
-    (* Add ct2 ct1 ca0 computes the end. *)
+    replace (heap_e - next - 2 <? n)%Z with false
+      by (symmetry; apply Z.ltb_ge; lia).
+    (* Jnz .malloc_no_memory ct3. *)
     iInstr "Hcode".
-    (* Mov ct4 ct0 copies the heap capability. *)
+    (* Compute the payload bounds and restrict its capability. *)
+    (* Add ct1 ct1 allocator_header_words. *)
     iInstr "Hcode".
-    (* Subseg ct4 ct1 ct2 narrows it to the requested interval. *)
+    assert (Hbword : WInt (next + 2) = WInt b) by (f_equal; solve_addr).
+    iEval (rewrite Hbword) in "Hct1".
+    (* Add ct2 ct1 ca0. *)
     iInstr "Hcode".
-    (* Mov ca2 ct4 copies the bounded capability for zeroing. *)
+    assert (Heword : WInt (b + n) = WInt finish) by (f_equal; solve_addr).
+    iEval (rewrite Heword) in "Hct2".
+    (* Mov ct4 ct0. *)
     iInstr "Hcode".
-    assert (Hfinish : (next + n)%a = Some (next ^+ n)%a) by solve_addr.
-    assert (Hnew : (next < (next ^+ n)%a /\ (next ^+ n)%a <= heap_e)%a) by solve_addr.
-    iApply "Hφ".
-    iSplitL "Hslot Hroot Hfree".
-    { iFrame. done. }
-    iFrame "Hcgp Hca0 Hct0 Hct1 Hcode".
-    iExists (next ^+ n)%a.
-    iSplit; first (iPureIntro; split; [exact Hfinish|exact Hnew]).
-    replace (allocator_malloc_block_addr pc_a 2) with (pc_a ^+ 16)%a by reflexivity.
-    assert (Hnextpc : ((pc_a ^+ 6)%a ^+ 10)%a = (pc_a ^+ 16)%a) by solve_addr.
-    iEval (rewrite Hnextpc) in "HPC".
-    replace (next ^+ (0 + n))%a with (next ^+ n)%a by solve_addr.
-    iFrame.
-    assert (Hword : WInt (next + n) = WInt (next ^+ n)%a) by (f_equal; solve_addr).
-    iEval (rewrite Hword) in "Hct2". iFrame.
+    (* Lea ct4 allocator_header_words. *)
+    iInstr "Hcode".
+    (* Subseg ct4 ct1 ct2. *)
+    iInstr "Hcode".
+    (* Take the header and payload from the free suffix before writing. *)
+    assert (Hsplit_range : (next <= finish /\ finish <= heap_e)%a) by solve_addr.
+    iEval (rewrite /free_cells
+      (finz_seq_between_split next finish heap_e Hsplit_range)
+      big_sepL_app) in "Hfree".
+    iDestruct "Hfree" as "[Hchunk Hfree]".
+    assert (Htake : (heap_b <= next /\ next <= finish /\ finish <= heap_e)%a)
+      by solve_addr.
+    iMod (allocator_take_range_correct E next finish HE Htake with "Hctx Hchunk")
+      as "Hchunk".
+    assert (Hnextfinish : (next < finish)%a) by solve_addr.
+    assert (Hsecondfinish : (next ^+ 1 < finish)%a) by solve_addr.
+    iEval (rewrite /allocator_range_memory
+      (finz_seq_between_cons next finish Hnextfinish) big_sepL_cons
+      (finz_seq_between_cons (next ^+ 1)%a finish Hsecondfinish) big_sepL_cons)
+      in "Hchunk".
+    iDestruct "Hchunk" as "(Hend & Hreserved & Hpayload)".
+    iDestruct "Hend" as (wend) "Hend".
+    iDestruct "Hreserved" as (wreserved) "Hreserved".
+    (* Write the end field. *)
+    (* Store ct0 ct2. *)
+    iInstr_lookup "Hcode" as "Hi" "Hcode".
+     wp_instr.
+    iApply (wp_store_success_reg _ _ _ _ _ _ _ _ ct0 ct2 wend
+      with "[$HPC $Hi $Hct2 $Hct0 $Hend]"); try solve_pure.
+    { eapply (disjoint_from_shadow_not_in heap_b heap_e next);
+        first exact heap_shadow_disjoint.
+      apply withinBounds_true_iff. solve_addr. }
+    { apply withinBounds_true_iff. solve_addr. }
+    iIntros "!> (HPC & Hi & Hct2 & Hct0 & Hend)". wp_pure.
+    iSpecialize ("Hcode" with "Hi").
+    (* Initialize the reserved field at offset one. *)
+    assert (Hsecond_shadow : is_shadow_address (next ^+ 1)%a = false).
+    { eapply (disjoint_from_shadow_not_in heap_b heap_e);
+        first exact heap_shadow_disjoint.
+      apply withinBounds_true_iff. solve_addr. }
+    assert (Hsecond_bounds : withinBounds heap_b heap_e (next ^+ 1)%a = true)
+      by (apply withinBounds_true_iff; solve_addr).
+    (* Store ct0 0 1. *)
+    iInstr_lookup "Hcode" as "Hi" "Hcode".
+     wp_instr.
+    iApply (wp_store_success_z_imm _ _ _ _ _ _ _ _ ct0 0 wreserved
+      _ _ _ _ _ (next ^+ 1)%a 1 with "[$HPC $Hi $Hct0 $Hreserved]"); try solve_pure.
+    { solve_addr. }
+    iIntros "!> (HPC & Hi & Hct0 & Hreserved)". wp_pure.
+    iSpecialize ("Hcode" with "Hi").
+    (* Copy the bounded payload capability for the zeroing loop. *)
+    (* Mov ca2 ct4. *)
+    iInstr_lookup "Hcode" as "Hi" "Hcode".
+     wp_instr.
+    iApply (wp_move_success_reg with "[$HPC $Hi $Hca2 $Hct4]"); try solve_pure.
+    iIntros "!> (HPC & Hi & Hca2 & Hct4)". wp_pure.
+    iSpecialize ("Hcode" with "Hi").
+    iApply "Hφ". iExists b, finish.
+    iSplit; first (iPureIntro; unfold allocator_header_words; naive_solver).
+    iSplitL "Hslot Hroot Hfree Hheaders Hhistory Hend Hreserved".
+    { iExists allocations. iFrame "Hslot Hroot Hfree Hheaders Hhistory".
+      iSplit; first done. iSplit.
+      { iPureIntro. unfold allocator_header_bounds, allocator_header_words. naive_solver. }
+      rewrite /allocator_header. iFrame "Hend Hreserved". done. }
+    iFrame "Hcgp Hca0 Hct0 Hct1 Hct2 Hct3 Hcode".
+    replace (allocator_malloc_block_addr pc_a 2) with (pc_a ^+ 21)%a by reflexivity.
+    assert (Hnextpc : ((pc_a ^+ 6)%a ^+ 15)%a = (pc_a ^+ 21)%a) by solve_addr.
+    iEval (rewrite Hnextpc) in "HPC". iFrame "HPC".
+    iFrame "Hct4 Hca2".
+    assert (Hbmem : ((next ^+ 1)%a ^+ 1)%a = b) by solve_addr.
+    iEval (rewrite Hbmem) in "Hpayload". iExact "Hpayload".
   Qed.
 
-  Lemma allocator_malloc_prepare_oom_spec
+  Local Lemma allocator_malloc_prepare_oom_spec
     (E : coPset)
     (pc_b pc_e pc_a next : Addr) (n : Z)
     (w0 w1 w2 w3 w4 wa2 : Word)
@@ -342,40 +418,41 @@ Section AllocatorMallocBlocks.
     SubBounds pc_b pc_e pc_a (pc_a ^+ length allocator_malloc_instrs)%a ->
     disjoint_from_shadow pc_b pc_e ->
     (0 < n)%Z ->
-    (heap_e - next < n)%Z ->
+    (heap_e - next - allocator_header_words < n)%Z ->
 
-    allocator_ctx
-    ∗ allocator_service_data next
-    ∗ ▷ PC ↦ᵣ WCap true RX Global pc_b pc_e start
-    ∗ ▷ cgp ↦ᵣ WCap true RW Global
-        allocator_cgp_b allocator_cgp_e allocator_cgp_b
-    ∗ ▷ ca0 ↦ᵣ WInt n
-    ∗ ▷ ct0 ↦ᵣ w0
-    ∗ ▷ ct1 ↦ᵣ w1
-    ∗ ▷ ct2 ↦ᵣ w2
-    ∗ ▷ ct3 ↦ᵣ w3
-    ∗ ▷ ct4 ↦ᵣ w4
-    ∗ ▷ ca2 ↦ᵣ wa2
-    ∗ ▷ codefrag start code
-    ∗ ▷ (allocator_service_data next
-         ∗ cgp ↦ᵣ WCap true RW Global
-             allocator_cgp_b allocator_cgp_e allocator_cgp_b
-         ∗ ca0 ↦ᵣ WInt n
-         ∗ ct0 ↦ᵣ WCap true RW Global heap_b heap_e next
-         ∗ ct1 ↦ᵣ WInt next
-         ∗ codefrag start code
-         ∗ PC ↦ᵣ WCap true RX Global pc_b pc_e
-             (allocator_malloc_block_addr pc_a 8)
-         ∗ ct2 ↦ᵣ WInt heap_e
-         ∗ ct3 ↦ᵣ WInt 1
-         ∗ ct4 ↦ᵣ w4
-         ∗ ca2 ↦ᵣ wa2
+    allocator_ctx ∗
+    allocator_service_data next ∗
+    PC ↦ᵣ WCap true RX Global pc_b pc_e start ∗
+    cgp ↦ᵣ WCap true RW Global
+        allocator_cgp_b allocator_cgp_e allocator_cgp_b ∗
+    ca0 ↦ᵣ WInt n ∗
+    ct0 ↦ᵣ w0 ∗
+    ct1 ↦ᵣ w1 ∗
+    ct2 ↦ᵣ w2 ∗
+    ct3 ↦ᵣ w3 ∗
+    ct4 ↦ᵣ w4 ∗
+    ca2 ↦ᵣ wa2 ∗
+    codefrag start code ∗
+    ▷ (allocator_service_data next ∗
+         cgp ↦ᵣ WCap true RW Global
+             allocator_cgp_b allocator_cgp_e allocator_cgp_b ∗
+         ca0 ↦ᵣ WInt n ∗
+         ct0 ↦ᵣ WCap true RW Global heap_b heap_e next ∗
+         ct1 ↦ᵣ WInt next ∗
+         codefrag start code ∗
+         PC ↦ᵣ WCap true RX Global pc_b pc_e
+             (allocator_malloc_block_addr pc_a 8) ∗
+         ct2 ↦ᵣ WInt heap_e ∗
+         ct3 ↦ᵣ WInt 1 ∗
+         ct4 ↦ᵣ w4 ∗
+         ca2 ↦ᵣ wa2
          -∗ WP Seq (Instr Executable) @ E {{ φ }})
     ⊢ WP Seq (Instr Executable) @ E {{ φ }}.
   Proof.
     intros start code Hlayout HE Hcont Hpc Hdisjoint Hpositive Hoom; subst start code.
-    iIntros "(#Hctx & Hdata & >HPC & >Hcgp & >Hca0 & >Hct0 & >Hct1 & >Hct2 & >Hct3 & >Hct4 & >Hca2 & >Hcode & Hφ)".
-    iDestruct "Hdata" as "(%Hnext & Hslot & Hroot & Hfree)".
+    iIntros "(#Hctx & Hdata & HPC & Hcgp & Hca0 & Hct0 & Hct1 & Hct2 & Hct3 & Hct4 & Hca2 & Hcode & Hφ)".
+    iDestruct "Hdata" as (allocations)
+      "(%Hnext & Hslot & Hroot & Hfree & Hheaders & Hhistory)".
     codefrag_facts "Hcode".
     assert (Hstart : allocator_malloc_block_addr pc_a 1 = (pc_a ^+ 6)%a) by reflexivity.
     iEval (rewrite Hstart) in "Hcode".
@@ -384,6 +461,7 @@ Section AllocatorMallocBlocks.
 
     (* Load ct0 cgp: the reserved root token proves the stored heap
        capability's shadow bit is clear, so the load preserves its tag. *)
+    (* Load ct0 cgp. *)
     iInstr_lookup "Hcode" as "Hi" "Hcode".
     wp_instr.
     iInv Nallocator as ">Hbody" "Hclose".
@@ -413,31 +491,34 @@ Section AllocatorMallocBlocks.
     codefrag_facts "Hcode".
     assert (Hstep : (pc_a ^+ 7)%a = ((pc_a ^+ 6)%a ^+ 1)%a) by solve_addr.
     iEval (rewrite Hstep) in "HPC".
-    iEval (simpl) in "Hct0".
-
+    iEval (cbn [load_word]) in "Hct0".
     (* GetA ct1 ct0. *)
     iInstr "Hcode".
     (* GetE ct2 ct0. *)
     iInstr "Hcode".
-    (* Sub ct3 ct2 ct1 computes remaining capacity. *)
+    (* Sub ct3 ct2 ct1. *)
     iInstr "Hcode".
-    (* Lt ct3 ct3 ca0 tests whether the request exceeds capacity. *)
+    (* Reserve the two header cells. *)
+    (* Sub ct3 ct3 allocator_header_words. *)
     iInstr "Hcode".
-    replace (heap_e - next <? n)%Z with true by (symmetry; apply Z.ltb_lt; lia).
+    unfold allocator_header_words in Hoom.
+    (* Lt ct3 ct3 ca0. *)
+    iInstr "Hcode".
+    replace (heap_e - next - 2 <? n)%Z with true by (symmetry; apply Z.ltb_lt; lia).
     (* Jnz to the out-of-memory block. *)
+    (* Jnz .malloc_no_memory ct3. *)
     iInstr_lookup "Hcode" as "Hi" "Hcode".
     wp_instr.
     iApply (wp_jnz_success_jmp_z with "[$HPC $Hi $Hct3]"); try solve_pure.
-    { instantiate (1 := (pc_a ^+ 46)%a). solve_addr. }
+    { instantiate (1 := (pc_a ^+ 52)%a). solve_addr. }
     iIntros "!> (HPC & Hi & Hct3)". wp_pure.
     iSpecialize ("Hcode" with "Hi").
-    iApply "Hφ". iFrame.
-    done.
+    iApply "Hφ". iFrame. done.
   Qed.
 
-  Lemma allocator_malloc_publish_spec
+  Local Lemma allocator_malloc_publish_spec
     (E : coPset)
-    (pc_b pc_e pc_a next finish : Addr) (n : Z) (wstatus : Word)
+    (pc_b pc_e pc_a next b finish : Addr) (n : Z) (wstatus : Word)
     (φ : language.val griotte_lang → iPropI Σ) :
 
     let start := allocator_malloc_block_addr pc_a 6 in
@@ -446,42 +527,48 @@ Section AllocatorMallocBlocks.
     ContiguousRegion pc_a (length allocator_malloc_instrs) ->
     SubBounds pc_b pc_e pc_a (pc_a ^+ length allocator_malloc_instrs)%a ->
     disjoint_from_shadow pc_b pc_e ->
-    (next + n)%a = Some finish ->
-    (heap_b < next /\ next < finish /\ finish <= heap_e)%a ->
+    (next + allocator_header_words)%a = Some b ->
+    (b + n)%a = Some finish ->
+    (heap_b < next /\ b < finish /\ finish <= heap_e)%a ->
 
-    ▷ PC ↦ᵣ WCap true RX Global pc_b pc_e start
-    ∗ ▷ cgp ↦ᵣ WCap true RW Global
-        allocator_cgp_b allocator_cgp_e allocator_cgp_b
-    ∗ ▷ ct0 ↦ᵣ WCap true RW Global heap_b heap_e next
-    ∗ ▷ ct4 ↦ᵣ WCap true RW Global next finish next
-    ∗ ▷ ca0 ↦ᵣ WInt n
-    ∗ ▷ ca1 ↦ᵣ wstatus
-    ∗ ▷ allocator_cgp_b ↦ₐ WCap true RW Global heap_b heap_e next
-    ∗ ▷ codefrag start code
-    ∗ ▷ (PC ↦ᵣ WCap true RX Global pc_b pc_e
-           (allocator_malloc_block_addr pc_a 9)
-         ∗ cgp ↦ᵣ WCap true RW Global
-             allocator_cgp_b allocator_cgp_e allocator_cgp_b
-         ∗ ct0 ↦ᵣ WCap true RW Global heap_b heap_e finish
-         ∗ ct4 ↦ᵣ WCap true RW Global next finish next
-         ∗ ca0 ↦ᵣ WCap true RW Global next finish next
-         ∗ ca1 ↦ᵣ WInt ALLOC_OK
-         ∗ allocator_cgp_b ↦ₐ WCap true RW Global heap_b heap_e finish
-         ∗ codefrag start code
+    PC ↦ᵣ WCap true RX Global pc_b pc_e start ∗
+    cgp ↦ᵣ WCap true RW Global
+        allocator_cgp_b allocator_cgp_e allocator_cgp_b ∗
+    ct0 ↦ᵣ WCap true RW Global heap_b heap_e next ∗
+    ct4 ↦ᵣ WCap true RW Global b finish b ∗
+    ca0 ↦ᵣ WInt n ∗
+    ca1 ↦ᵣ wstatus ∗
+    allocator_cgp_b ↦ₐ WCap true RW Global heap_b heap_e next ∗
+    codefrag start code ∗
+    ▷ (PC ↦ᵣ WCap true RX Global pc_b pc_e
+           (allocator_malloc_block_addr pc_a 9) ∗
+         cgp ↦ᵣ WCap true RW Global
+             allocator_cgp_b allocator_cgp_e allocator_cgp_b ∗
+         ct0 ↦ᵣ WCap true RW Global heap_b heap_e finish ∗
+         ct4 ↦ᵣ WCap true RW Global b finish b ∗
+         ca0 ↦ᵣ WCap true RW Global b finish b ∗
+         ca1 ↦ᵣ WInt ALLOC_OK ∗
+         allocator_cgp_b ↦ₐ WCap true RW Global heap_b heap_e finish ∗
+         codefrag start code
          -∗ WP Seq (Instr Executable) @ E {{ φ }})
     ⊢ WP Seq (Instr Executable) @ E {{ φ }}.
   Proof.
-    intros start code Hlayout Hcont Hpc Hdisjoint Hfinish Hrange; subst start code.
-    iIntros "(>HPC & >Hcgp & >Hct0 & >Hct4 & >Hca0 & >Hca1 & >Hslot & >Hcode & Hφ)".
+    intros start code Hlayout Hcont Hpc Hdisjoint Hbase Hfinish Hrange; subst start code.
+    iIntros "(HPC & Hcgp & Hct0 & Hct4 & Hca0 & Hca1 & Hslot & Hcode & Hφ)".
     codefrag_facts "Hcode".
-    (* Lea ct0 ca0 computes the new bump cursor. *)
+    unfold allocator_header_words in Hbase.
+    assert (Hstart : allocator_malloc_block_addr pc_a 6 = (pc_a ^+ 43)%a) by reflexivity.
+    iEval (rewrite Hstart) in "Hcode HPC". rewrite Hstart in H.
+    (* Skip the header, then advance over the payload. *)
+    (* Lea ct0 allocator_header_words. *)
     iInstr "Hcode".
-    assert (Hstart : allocator_malloc_block_addr pc_a 6 = (pc_a ^+ 38)%a) by reflexivity.
-    iEval (rewrite Hstart) in "Hcode".
-    rewrite Hstart in H.
-    assert (Hstep : (pc_a ^+ 39)%a = ((pc_a ^+ 38)%a ^+ 1)%a) by solve_addr.
-    iEval (rewrite Hstep) in "HPC".
+    assert (Hstep1 : (pc_a ^+ 44)%a = ((pc_a ^+ 43)%a ^+ 1)%a) by solve_addr.
+    iEval (rewrite Hstep1) in "HPC".
+    (* Lea ct0 ca0. *)
+    iInstr "Hcode".
+    assert (Hstep : (pc_a ^+ 45)%a = ((pc_a ^+ 43)%a ^+ 2)%a) by solve_addr.
     (* Store cgp ct0 publishes the new cursor. *)
+    (* Store cgp ct0. *)
     iInstr_lookup "Hcode" as "Hi" "Hcode".
     wp_instr.
     iApply (wp_store_success_reg _ _ _ _ _ _ _ _ _ _
@@ -507,31 +594,25 @@ Section AllocatorMallocBlocks.
     (* Jmp .malloc_return. *)
     iInstr "Hcode".
     iApply "Hφ". iFrame.
-    replace (allocator_malloc_block_addr pc_a 9) with (pc_a ^+ 48)%a by reflexivity.
-    assert (Hret : ((pc_a ^+ 38)%a ^+ 10)%a = (pc_a ^+ 48)%a) by solve_addr.
+    replace (allocator_malloc_block_addr pc_a 9) with (pc_a ^+ 54)%a by reflexivity.
+    assert (Hret : ((pc_a ^+ 43)%a ^+ 11)%a = (pc_a ^+ 54)%a) by solve_addr.
     iEval (rewrite Hret) in "HPC". iFrame.
   Qed.
-End AllocatorMallocBlocks.
 
-Section AllocatorMallocProof.
-  Context
-    {Σ : gFunctors}
-    {ceriseg : ceriseG Σ}
-    {allocatorg : allocatorG Σ}
-    {MP : MachineParameters}
-    {layout : allocatorLayout}
-    {layout_wf : allocatorLayoutWf}
-  .
+  Context {layout_wf : allocatorLayoutWf}.
 
   (** A noninteger or nonpositive size is rejected before the heap is read.
       Other registers and resources can be framed. *)
+
   Lemma allocator_malloc_invalid_correct
     (E : coPset) (wreq wret : Word)
     (φ : language.val griotte_lang → iPropI Σ) :
 
-    ⊢ (⌜↑Nallocator ⊆ E⌝ -∗
-       ⌜↑Nallocator_service ⊆ E⌝ -∗
-       ⌜¬ allocator_positive_size wreq⌝ -∗
+    ↑Nallocator ⊆ E ->
+    ↑Nallocator_service ⊆ E ->
+    ¬ allocator_positive_size wreq ->
+
+    ⊢ (
 
        allocator_ctx ∗
        allocator_service_ctx ∗
@@ -573,7 +654,7 @@ Section AllocatorMallocProof.
           -∗ WP Seq (Instr Executable) @ E {{ φ }})
        -∗ WP Seq (Instr Executable) @ E {{ φ }})%I.
   Proof.
-    iIntros "%HEheap %HEservice %Hinvalid".
+    intros HEheap HEservice Hinvalid.
     iIntros "(#Hctx & #Hservice & Hna & HPC & Hcgp & Hcra & Hca0 & Hca1 & Hca2 & Hct0 & Hct1 & Hct2 & Hct3 & Hct4 & Hctp & Hcnull & Hpost)".
     (* Open the service invariant and recover the allocator code and state. *)
     iMod (na_inv_acc with "Hservice Hna") as "(Hinv & Hna & Hclose)"; try exact HEservice.
@@ -669,13 +750,16 @@ Section AllocatorMallocProof.
   (** A positive integer size either exceeds the remaining suffix or obtains
       a fresh, exactly bounded, zeroed range. The bump cursor stays hidden in
       the service invariant. *)
+
   Lemma allocator_malloc_valid_correct
     (E : coPset) (n : Z) (wret : Word)
     (φ : language.val griotte_lang → iPropI Σ) :
 
-    ⊢ (⌜↑Nallocator ⊆ E⌝ -∗
-       ⌜↑Nallocator_service ⊆ E⌝ -∗
-       ⌜(0 < n)%Z⌝ -∗
+    ↑Nallocator ⊆ E ->
+    ↑Nallocator_service ⊆ E ->
+    (0 < n)%Z ->
+
+    ⊢ (
 
        allocator_ctx ∗
        allocator_service_ctx ∗
@@ -719,12 +803,13 @@ Section AllocatorMallocProof.
                   (e - b = n)%Z⌝ ∗
                 ca0 ↦ᵣ WCap true RW Global b e b ∗
                 ca1 ↦ᵣ WInt ALLOC_OK ∗
+                allocator_allocation b e 0 ∗
                 allocator_zeroed b e))
 
           -∗ WP Seq (Instr Executable) @ E {{ φ }})
        -∗ WP Seq (Instr Executable) @ E {{ φ }})%I.
   Proof.
-    iIntros "%HEheap %HEservice %Hpositive".
+    intros HEheap HEservice Hpositive.
     iIntros "(#Hctx & #Hservice & Hna & HPC & Hcgp & Hcra & Hca0 & Hca1 & Hca2 & Hct0 & Hct1 & Hct2 & Hct3 & Hct4 & Hctp & Hcnull & Hpost)".
     (* Open the service invariant and recover the allocator code and state. *)
     iMod (na_inv_acc with "Hservice Hna") as "(Hinv & Hna & Hclose)"; try exact HEservice.
@@ -788,31 +873,18 @@ Section AllocatorMallocProof.
     iDestruct "Hct3" as (w3b) "Hct3".
     iDestruct "Hct4" as (w4) "Hct4".
     iDestruct "Hca2" as (wa2) "Hca2".
-    destruct (decide (n <= heap_e - next)%Z) as [Hroom|Hoom].
+    destruct (decide (n + allocator_header_words <= heap_e - next)%Z) as [Hroom|Hoom].
     - iApply (allocator_malloc_prepare_success_spec with
         "[- $Hctx $Hdata $HPC $Hcgp $Hca0 $Hct0 $Hct1 $Hct2 $Hct3 $Hct4 $Hca2 $Hprepare_code]"); eauto.
       { rewrite -Hstart. exact H. }
-      iNext. iIntros
-        "(Hdata & Hcgp & Hca0 & Hct0 & Hct1 & Hprepare_code & Hroom)".
-      iDestruct "Hroom" as (finish)
-        "(%Hfinish & HPC & Hct2 & Hct3 & Hct4 & Hca2)".
-      destruct Hfinish as [Hfinish Hrange].
+      iNext. iIntros "(%b & %finish & %Hbounds & Hpending & Hrange_mem &
+        Hcgp & Hca0 & Hct0 & Hct1 & Hprepare_code & HPC & Hct2 & Hct3 & Hct4 & Hca2)".
+      destruct Hbounds as (Hbase & Hfinish & Hrange).
+      unfold allocator_header_words in Hbase.
       iDestruct ("Hmalloc_cont" with "Hprepare_code") as "Hmalloc_code".
       iEval (rewrite -Hsplit1) in "Hmalloc_code".
-      iDestruct "Hdata" as "(%Hnext & Hslot & Hroot & Hfree)".
-      (* Take ownership of the requested range from the free suffix. *)
-      assert (Hsplit_range : (next <= finish /\ finish <= heap_e)%a)
-        by solve_addr.
-      iEval (rewrite /free_cells
-        (finz_seq_between_split next finish heap_e Hsplit_range)
-        big_sepL_app) in "Hfree".
-      iDestruct "Hfree" as "[Hrange_free Hfree]".
-      iPoseProof (allocator_take_range_correct E next finish) as "Htake".
-      iSpecialize ("Htake" with
-        "[] [] Hctx Hrange_free").
-      { iPureIntro. exact HEheap. }
-      { iPureIntro. solve_addr. }
-      iMod "Htake" as "Hrange_mem".
+      iDestruct "Hpending" as (allocations)
+        "(%Hnext & %Hchunk & Hslot & Hroot & Hfree & Hheaders & Hhistory & Hhead)".
       (* Zero the newly allocated cells. *)
       assert (Hsplit2 : allocator_malloc_instrs =
         concat (encodeInstrsW <$> take 2 assembled_allocator_malloc) ++
@@ -833,7 +905,7 @@ Section AllocatorMallocProof.
       iApply (allocator_zero_spec ca2 ct2 ct3 E RX Global
         allocator_pcc_b allocator_pcc_e
         (allocator_malloc_block_addr allocator_malloc_pcc_addr 2)
-        RW Global next finish (WInt 0)
+        RW Global b finish (WInt 0)
         with "[- $HPC $Hca2 $Hct2 $Hct3 $Hzero_code $Hrange_mem]").
       { reflexivity. }
       { unfold allocator_malloc_block_addr; cbn; solve_addr. }
@@ -846,7 +918,7 @@ Section AllocatorMallocProof.
         constructor.
         { apply not_elem_of_nil. }
         { constructor. } }
-      iNext. iIntros "(HPC & Hca2 & Hct2 & Hct3 & Hzero_code & Hzeros)".
+      iNext. iIntros "(HPC & Hca2 & Hct2 & Hct3 & Hzeros & Hzero_code)".
       iEval (rewrite -Hzero_eq) in "Hzero_code".
       iDestruct ("Hmalloc_cont" with "Hzero_code") as "Hmalloc_code".
       iEval (rewrite -Hsplit2) in "Hmalloc_code".
@@ -901,7 +973,7 @@ Section AllocatorMallocProof.
       { discriminate. }
       { discriminate. }
       { discriminate. }
-      iNext. iIntros "(HPC & Hctp & Hct3 & Hca2 & Hfetch_code & Himport)".
+      iNext. iIntros "(HPC & Hctp & Hct3 & Hca2 & Himport & Hfetch_code)".
       iEval (cbn) in "Hctp".
       iEval (rewrite Himpaddr) in "Himport".
       iAssert ([[allocator_pcc_b,allocator_code_b]] ↦ₐ [[allocator_imports]])%I
@@ -937,8 +1009,8 @@ Section AllocatorMallocProof.
         "(HPC & Hct0 & Hct1 & Hct2 & Hct3 & Hctp & Hca2 & Htranslate_code)".
       iDestruct ("Hmalloc_cont" with "Htranslate_code") as "Hmalloc_code".
       iEval (rewrite -Hsplit4) in "Hmalloc_code".
-      iAssert ([[next, finish]] ↦ₐ
-        [[replicate (length (finz.seq_between next finish)) (WInt 0)]])%I
+      iAssert ([[b, finish]] ↦ₐ
+        [[replicate (length (finz.seq_between b finish)) (WInt 0)]])%I
         with "[Hzeros]" as "Hzeros".
       { rewrite /region_pointsto big_sepL2_replicate_r; last reflexivity.
         iFrame. }
@@ -961,14 +1033,14 @@ Section AllocatorMallocProof.
         allocator_malloc_block_addr allocator_malloc_pcc_addr 5).
       { unfold allocator_malloc_block_addr. solve_addr. }
       iEval (rewrite Hpc5) in "HPC".
-      pose (sb := (shadow_b ^+ (next - heap_b))%a).
+      pose (sb := (shadow_b ^+ (b - heap_b))%a).
       pose (se := (shadow_b ^+ (finish - heap_b))%a).
       assert (Hshadow : (shadow_b <= sb /\ sb < se /\ se <= shadow_e)%a).
       { pose proof heap_shadow_same_size. unfold sb, se. solve_addr. }
-      assert (Hlen_shadow : (se - sb = finish - next)%Z).
+      assert (Hlen_shadow : (se - sb = finish - b)%Z).
       { unfold sb, se. pose proof heap_shadow_same_size. solve_addr. }
-      assert (Htranslation : ∀ x, (next <= x /\ x < finish)%a ->
-        heap_to_shadow x = Some (sb ^+ (x - next))%a).
+      assert (Htranslation : ∀ x, (b <= x /\ x < finish)%a ->
+        heap_to_shadow x = Some (sb ^+ (x - b))%a).
       { intros x Hx. rewrite allocator_translation_affine.
         unfold translate_region.
         assert (Hxheap : withinBounds heap_b heap_e x = true).
@@ -981,8 +1053,8 @@ Section AllocatorMallocProof.
       iApply (allocator_paint_spec ShadowLive ctp ca2 E RX Global
         allocator_pcc_b allocator_pcc_e
         (allocator_malloc_block_addr allocator_malloc_pcc_addr 5)
-        next finish sb se
-        (replicate (length (finz.seq_between next finish)) (WInt 0))
+        b finish sb se
+        (replicate (length (finz.seq_between b finish)) (WInt 0))
         with "[- $Hctx $HPC $Hctp $Hca2 $Hpaint_code $Hzeros]").
       { reflexivity. }
       { rewrite -Hpaint_eq;
@@ -999,7 +1071,7 @@ Section AllocatorMallocProof.
         try apply not_elem_of_nil; constructor.
         { apply not_elem_of_nil. }
         { constructor. } }
-      iNext. iIntros "(HPC & Hctp & Hca2 & Hpaint_code & Hzeros)".
+      iNext. iIntros "(HPC & Hctp & Hca2 & Hzeros & Hpaint_code)".
       iEval (rewrite -Hpaint_eq) in "Hpaint_code".
       iDestruct ("Hmalloc_cont" with "Hpaint_code") as "Hmalloc_code".
       iEval (rewrite -Hsplit5) in "Hmalloc_code".
@@ -1018,9 +1090,9 @@ Section AllocatorMallocProof.
         clear -Ha_publish. cbn [take concat fmap] in *. solve_addr. }
       subst a_publish.
       assert (Hoff5 : allocator_malloc_block_addr allocator_malloc_pcc_addr 5 =
-        (allocator_malloc_pcc_addr ^+ 34)%a) by reflexivity.
+        (allocator_malloc_pcc_addr ^+ 39)%a) by reflexivity.
       assert (Hoff6 : allocator_malloc_block_addr allocator_malloc_pcc_addr 6 =
-        (allocator_malloc_pcc_addr ^+ 38)%a) by reflexivity.
+        (allocator_malloc_pcc_addr ^+ 43)%a) by reflexivity.
       assert (Hlenpaint : length (allocator_paint_instrs ctp ca2 ShadowLive) = 4)
         by reflexivity.
       assert (Hpc6 : (allocator_malloc_block_addr allocator_malloc_pcc_addr 5 ^+
@@ -1029,7 +1101,7 @@ Section AllocatorMallocProof.
       { clear -Hoff5 Hoff6 Hlenpaint.
         rewrite Hoff5 Hoff6 Hlenpaint.
         rewrite incr_addr_opt_add_twice.
-        { replace (34 + 4)%Z with 38%Z by lia; reflexivity. }
+        { replace (39 + 4)%Z with 43%Z by lia; reflexivity. }
         all: lia. }
       iEval (rewrite Hpc6) in "HPC".
       iDestruct "Hca1" as (wca1) "Hca1".
@@ -1038,6 +1110,7 @@ Section AllocatorMallocProof.
       { rewrite -Hstart; exact H. }
       { exact Hpc. }
       { exact Hdisjoint. }
+      { exact Hbase. }
       { exact Hfinish. }
       { split; [exact (proj1 Hnext)|exact Hrange]. }
       iNext. iIntros
@@ -1070,22 +1143,24 @@ Section AllocatorMallocProof.
       iEval (rewrite -Hsplit9) in "Hmalloc_code".
       iDestruct ("Hcode_cont" with "Hmalloc_code") as "Hcode".
       iEval (rewrite -/allocator_code) in "Hcode".
-      iMod ("Hclose" with "[Himports Hcode Hslot Hroot Hfree Hna]") as "Hna".
+      iMod (allocator_service_commit_spec next b finish 0 allocations
+        (proj1 Hnext) Hchunk with "Hslot Hroot Hfree Hheaders Hhistory Hhead")
+        as "[Hdata Hreceipt]".
+      iMod ("Hclose" with "[Himports Hcode Hdata Hna]") as "Hna".
       { iSplitR "Hna"; last iFrame.
         iNext. iSplitL "Himports Hcode"; first iFrame.
-        iExists finish. iFrame. iPureIntro.
-        clear -Hnext Hrange. solve_addr. }
+        iExists finish. iExact "Hdata". }
       iApply "Hpost". iFrame "∗".
-      iRight. iExists next, finish.
+      iRight. iExists b, finish.
       iSplit.
       { iPureIntro. split.
-        { split; [exact (proj1 Hnext)|exact Hrange]. }
+        { solve_addr. }
         { clear -Hfinish. solve_addr. } }
       iFrame.
       rewrite /allocator_zeroed /region_pointsto big_sepL2_replicate_r;
         last reflexivity.
       iFrame.
-    - assert (Hcapacity : (heap_e - next < n)%Z) by lia.
+    - assert (Hcapacity : (heap_e - next - allocator_header_words < n)%Z) by lia.
       iApply (allocator_malloc_prepare_oom_spec with
         "[- $Hctx $Hdata $HPC $Hcgp $Hca0 $Hct0 $Hct1 $Hct2 $Hct3 $Hct4 $Hca2 $Hprepare_code]"); eauto.
       { rewrite -Hstart. exact H. }
@@ -1146,4 +1221,5 @@ Section AllocatorMallocProof.
         iExists next. iFrame. }
       iApply "Hpost". iFrame "∗". iLeft. iFrame.
   Qed.
-End AllocatorMallocProof.
+
+End AllocatorMallocBlocks.
