theories/case_studies/heap_temporal_safety/heap_temporal_safety_spec.v
@@ -14,6 +14,7 @@ Section Heap_Temporal_Safety_Main.
     {Cname : CmptNameG}
     {stsg : STSG Addr region_type OType Word Σ} {relg : relGS Σ}
     {cstackg : CSTACKG Σ} {allocatorg : allocatorG Σ}
+    {allocator_historyg : allocatorHistoryG Σ}
     `{MP: MachineParameters}
     {alloclayout : allocatorLayout} {allocwf : allocatorLayoutWf}
     {swlayout : switcherLayout} {swlayoutWf : switcherLayoutWf} {assertlayout : assertLayout}
